decidablity with several holes

proof/uni/algo_worklist/prop_decidability.v
@@ -6,359 +6,160 @@ Require Import Coq.micromega.Lia.
 
 Require Import uni.notations.
 Require Import uni.prop_basic.
+Require Import uni.decl_worklist.prop_equiv.
 Require Import uni.algo_worklist.def_extra.
 Require Import uni.algo_worklist.prop_basic.
 Require Import uni.algo_worklist.prop_rename.
+Require Import uni.algo_worklist.prop_soundness.
+Require Import uni.algo_worklist.prop_completeness.
+Require Import uni.algo_worklist.transfer.
 Require Import ltac_utils.
 
-Fixpoint iu_size (A : typ) : nat :=
-  match A with
-  | typ_unit => 0
-  | typ_bot => 0
-  | typ_top => 0
-  | typ_var_f _ => 0
-  | typ_var_b _ => 0
-  | typ_arrow A1 A2 => iu_size A1 + iu_size A2
-  | typ_all A => iu_size A
-  | typ_union A1 A2 => 2 + iu_size A1 + iu_size A2
-  | typ_intersection A1 A2 => 2 + iu_size A1 + iu_size A2
-  end.
-
-Fixpoint exp_size (e : exp) : nat :=
+Fixpoint exp_size (Γ : aworklist) (e : exp) : nat :=
   match e with
   | exp_unit => 1
   | exp_var_b _ => 1
   | exp_var_f _ => 1
-  | exp_abs e => 1 + exp_size e
-  | exp_app e1 e2 => 1 + exp_size e1 + exp_size e2
-  | exp_tabs b => 1 + body_size b
-  | exp_tapp e _ => 1 + exp_size e
-  | exp_anno e A => 1 + exp_size e * (1 + iu_size A)
+  | exp_abs e => 1 + exp_size Γ e
+  | exp_app e1 e2 => 1 + exp_size Γ e1 + exp_size Γ e2 * (1 + exp_split_size (awl_to_aenv Γ) e1)
+  | exp_tabs b => 1 + body_size Γ b
+  | exp_tapp e _ => 1 + exp_size Γ e
+  | exp_anno e A => 1 + exp_size Γ e * (1 + iu_size A)
   end
-with body_size (b : body) : nat :=
+with body_size (Γ : aworklist) (b : body) : nat :=
   match b with 
-  | body_anno e A => exp_size e * (1 + iu_size A)
+  | body_anno e A => exp_size Γ e * (1 + iu_size A)
   end.
 
-Lemma exp_size_gt_0 : forall e,
-  exp_size e > 0.
+Lemma exp_size_gt_0 : forall Γ e,
+  exp_size Γ e > 0.
 Proof.
   induction e; simpl; try lia.
 Qed.
 
-Fixpoint exp_size_cont (c : cont) : nat :=
-  match c with
-  | cont_infabs c => exp_size_cont c
-  | cont_infabsunion _ c => exp_size_cont c
-  | cont_infapp e c => exp_size e + exp_size_cont c
-  | cont_inftapp _ c => exp_size_cont c
-  | cont_inftappunion _ _ c => exp_size_cont c
-  | cont_unioninftapp _ c => exp_size_cont c
-  | cont_unioninfabs _ c => exp_size_cont c
-  | cont_sub A => 0
+Fixpoint exp_size_conts (Γ : aworklist) (cs : conts) : nat :=
+  match cs with
+  | conts_infabs cd => exp_size_contd Γ cd
+  | conts_inftapp _ cs => exp_size_conts Γ cs
+  | conts_inftappunion _ _ cs => exp_size_conts Γ cs
+  | conts_unioninftapp _ cs => exp_size_conts Γ cs
+  | conts_sub A => 0
+  end
+with exp_size_contd (Γ : aworklist) (cd : contd) : nat :=
+  match cd with
+  | contd_infabsunion _ cd => exp_size_contd Γ cd
+  | contd_infapp n e cs => exp_size Γ e * (1 + n) + exp_size_conts Γ cs
+  | contd_unioninfabs _ _ cd => exp_size_contd Γ cd
   end.
 
-Definition exp_size_work (w : work) : nat :=
+Definition exp_size_work (Γ : aworklist) (w : work) : nat :=
   match w with
-  | work_infer e c => exp_size e + exp_size_cont c
-  | work_check e A => exp_size e * (1 + iu_size A)
-  | work_infabs _ c => exp_size_cont c
-  | work_infabsunion _ _ c => exp_size_cont c
-  | work_infapp _ e c => exp_size e + exp_size_cont c
-  | work_inftapp _ _ c => exp_size_cont c
+  | work_infer e cs => exp_size Γ e + exp_size_conts Γ cs
+  | work_check e A => exp_size Γ e * (1 + iu_size A)
+  | work_infabs _ cd => exp_size_contd Γ cd
+  | work_infabsunion _ _ _ cd => exp_size_contd Γ cd
+  | work_infapp A _ e cs => exp_size Γ e * (1 + iu_size A) + exp_size_conts Γ cs
+  | work_inftapp _ _ cs => exp_size_conts Γ cs
   | work_sub _ _ => 0
-  | work_inftappunion _ _ _ c => exp_size_cont c
-  | work_unioninftapp _ _ c => exp_size_cont c
-  | work_unioninfabs _ _ c => exp_size_cont c
-  | work_apply c _ => exp_size_cont c
+  | work_inftappunion _ _ _ cs => exp_size_conts Γ cs
+  | work_unioninftapp _ _ cs => exp_size_conts Γ cs
+  | work_unioninfabs _ _ _ _ cd => exp_size_contd Γ cd
+  | work_applys cs _ => exp_size_conts Γ cs
+  | work_applyd cd _ _ => exp_size_contd Γ cd
   end.
 
 Fixpoint exp_size_wl (Γ : aworklist) : nat :=
   match Γ with
   | aworklist_empty => 0 
-  | aworklist_constvar Γ' _ _ => exp_size_wl Γ'
-  | aworklist_consvar Γ' _ _ => exp_size_wl Γ'
-  | aworklist_conswork Γ' w => exp_size_work w + exp_size_wl Γ'
+  | aworklist_cons_var Γ' _ _ => exp_size_wl Γ'
+  | aworklist_cons_work Γ' w => exp_size_work Γ' w + exp_size_wl Γ'
   end.
 
-Fixpoint judge_size_cont (c : cont) : nat :=
-  match c with
-  | cont_infabs c => judge_size_cont c
-  | cont_infabsunion _ c => judge_size_cont c
-  | cont_infapp _ c => 4 + judge_size_cont c
-  | cont_inftapp _ c => judge_size_cont c
-  | cont_inftappunion _ _ c => judge_size_cont c
-  | cont_unioninftapp _ c => judge_size_cont c
-  | cont_unioninfabs _ c => judge_size_cont c
-  | cont_sub A => 0
+Fixpoint judge_size_conts (cs : conts) : nat :=
+  match cs with
+  | conts_infabs cd => judge_size_contd cd
+  | conts_inftapp _ cs => judge_size_conts cs
+  | conts_inftappunion _ _ cs => judge_size_conts cs
+  | conts_unioninftapp _ cs => judge_size_conts cs
+  | conts_sub _ => 0
+  end
+with judge_size_contd (cd : contd) : nat :=
+  match cd with
+  | contd_infabsunion _ cd => judge_size_contd cd
+  | contd_infapp _ _ cs => 5 + judge_size_conts cs
+  | contd_unioninfabs _ _ cd => judge_size_contd cd
   end.
 
 Definition judge_size_work (w : work) : nat :=
   match w with
-  | work_infer _ c => 2 + judge_size_cont c
-  | work_check _ _ => 3
-  | work_infabs _ c => judge_size_cont c
-  | work_infabsunion _ _ c => judge_size_cont c
-  | work_infapp _ _ c => 4 + judge_size_cont c
-  | work_inftapp _ _ c => judge_size_cont c
+  | work_infer e cs => 2 + judge_size_conts cs
+  | work_check e A => 3
+  | work_infabs _ cd => judge_size_contd cd
+  | work_infabsunion _ _ _ cd => judge_size_contd cd
+  | work_infapp _ _ e cs => 5 + judge_size_conts cs
+  | work_inftapp _ _ cs => judge_size_conts cs
   | work_sub _ _ => 0
-  | work_inftappunion _ _ _ c => judge_size_cont c
-  | work_unioninftapp _ _ c => judge_size_cont c
-  | work_unioninfabs _ _ c => judge_size_cont c
-  | work_apply c _ => 1 + judge_size_cont c
+  | work_inftappunion _ _ _ cs => judge_size_conts cs
+  | work_unioninftapp _ _ cs => judge_size_conts cs
+  | work_unioninfabs _ _ _ _ cd => judge_size_contd cd
+  | work_applys cs _ => 1 + judge_size_conts cs
+  | work_applyd cd _ _ => 1 + judge_size_contd cd
   end.
 
 Fixpoint judge_size_wl (Γ : aworklist) : nat :=
   match Γ with
   | aworklist_empty => 0 
-  | aworklist_constvar Γ' _ _ => judge_size_wl Γ'
-  | aworklist_consvar Γ' _ _ => judge_size_wl Γ'
-  | aworklist_conswork Γ' w => judge_size_work w + judge_size_wl Γ'
+  | aworklist_cons_var Γ' _ _ => judge_size_wl Γ'
+  | aworklist_cons_work Γ' w => judge_size_work w + judge_size_wl Γ'
   end.
 
-Inductive split_size : aworklist -> typ -> nat -> Prop :=
-  | split_size_unit : forall Γ,
-      split_size Γ typ_unit 0
-  | split_size_bot : forall Γ,
-      split_size Γ typ_bot 0
-  | split_size_top : forall Γ,
-      split_size Γ typ_top 0
-  | split_size_var_f : forall Γ X,
-      split_size Γ (typ_var_f X) 0
-  | split_size_var_b : forall Γ n,
-      split_size Γ (typ_var_b n) 0
-  | split_size_arrow : forall Γ A1 A2,
-      a_mono_typ (awl_to_aenv Γ) (typ_arrow A1 A2) ->
-      split_size Γ (typ_arrow A1 A2) 0
-  | split_size_arrow_s : forall Γ A1 A2 n1 n2 n,
-      ~ a_mono_typ (awl_to_aenv Γ) (typ_arrow A1 A2) ->
-      split_size Γ A1 n1 -> split_size Γ A2 n2 ->
-      n = n1 + n2 ->
-      split_size Γ (typ_arrow A1 A2) (S n)
-  | split_size_all : forall L Γ A n,
-      ( forall X , X \notin L ->
-        split_size (aworklist_constvar Γ X abind_stvar_empty) (open_typ_wrt_typ A (typ_var_f X)) n) ->
-      split_size Γ (typ_all A) n
-  | split_size_union : forall Γ A1 A2 n1 n2 n,
-      split_size Γ A1 n1 ->
-      split_size Γ A2 n2 ->
-      n = n1 + n2 ->
-      split_size Γ (typ_union A1 A2) (S n)
-  | split_size_intersection : forall Γ A1 A2 n1 n2 n,
-      split_size Γ A1 n1 ->
-      split_size Γ A2 n2 ->
-      n = n1 + n2 ->
-      split_size Γ (typ_intersection A1 A2) (S n).
-
-Theorem split_size_total : forall Γ A,
-  a_wf_typ (awl_to_aenv Γ) A -> exists n, split_size Γ A n.
-Admitted.
-
-Theorem split_size_det : forall Γ A n1 n2,
-  split_size Γ A n1 -> split_size Γ A n2 -> n1 = n2.
-Admitted.
-
-Inductive split_size_work : aworklist -> work -> nat -> Prop :=
-  | split_size_work_infer : forall Γ e c,
-      split_size_work Γ (work_infer e c) 0
-  | split_size_work_check : forall Γ e A,
-      split_size_work Γ (work_check e A) 0
-  | split_size_work_infabs : forall Γ A c n,
-      split_size Γ A n ->
-      split_size_work Γ (work_infabs A c) n
-  | split_size_work_infabsunion : forall Γ A1 A2 c,
-      split_size_work Γ (work_infabsunion A1 A2 c) 0
-  | split_size_work_infapp : forall Γ A e c,
-      split_size_work Γ (work_infapp A e c) 0
-  | split_size_work_inftapp : forall Γ A1 A2 c,
-      split_size_work Γ (work_inftapp A1 A2 c) 0
-  | split_size_work_sub : forall Γ A1 A2 n1 n2 n,
-      split_size Γ A1 n1 ->
-      split_size Γ A2 n2 ->
-      n = n1 + n2 ->
-      split_size_work Γ (work_sub A1 A2) n
-  | split_size_work_inftappunion : forall Γ A1 A2 A3 c,
-      split_size_work Γ (work_inftappunion A1 A2 A3 c) 0
-  | split_size_work_unioninftapp : forall Γ A1 A2 c,
-      split_size_work Γ (work_unioninftapp A1 A2 c) 0
-  | split_size_work_unioninfabs : forall Γ A1 A2 c,
-      split_size_work Γ (work_unioninfabs A1 A2 c) 0
-  | split_size_work_apply : forall Γ c A,
-      split_size_work Γ (work_apply c A) 0.
-
-Theorem split_size_work_total : forall Γ w,
-  a_wf_work (awl_to_aenv Γ) w -> exists n, split_size_work Γ w n.
-Admitted.
-
-Theorem split_size_work_det : forall Γ w n1 n2,
-  split_size_work Γ w n1 -> split_size_work Γ w n2 -> n1 = n2.
-Admitted.
-
-Inductive split_size_wl : aworklist -> nat -> Prop :=
-  | split_size_wl_empty : split_size_wl aworklist_empty 0
-  | split_size_wl_constvar : forall Γ X A n,
-      split_size_wl Γ n ->
-      split_size_wl (aworklist_constvar Γ X A) n
-  | split_size_wl_consvar : forall Γ X A n,
-      split_size_wl Γ n ->
-      split_size_wl (aworklist_consvar Γ X A) n
-  | split_size_wl_conswork : forall Γ w m n k,
-      split_size_work Γ w m ->
-      split_size_wl Γ n ->
-      k = m + n ->
-      split_size_wl (aworklist_conswork Γ w) k.
-
-Theorem split_size_wl_det : forall Γ n1 n2,
-  split_size_wl Γ n1 -> split_size_wl Γ n2 -> n1 = n2.
-Admitted.
-
-Theorem split_size_wl_total : forall Γ,
-  a_wf_wl Γ -> exists n, split_size_wl Γ n.
-Admitted.
-
-Fixpoint all_size (A : typ) : nat :=
+Fixpoint split_depth_rec (Σ : aenv) (A:typ) (n:nat) : nat :=
   match A with
-  | typ_unit => 0
-  | typ_bot => 0
-  | typ_top => 0
-  | typ_var_f _ => 0
-  | typ_var_b _ => 0
-  | typ_arrow A1 A2 => all_size A1 + all_size A2
-  | typ_all A => 1 + all_size A
-  | typ_union A1 A2 => all_size A1 + all_size A2
-  | typ_intersection A1 A2 => all_size A1 + all_size A2
+  | typ_var_f X => match lookup_tvar_bind Σ X with
+                   | Some abind_stvar_empty => n
+                   | _ => 0
+                   end
+  | typ_var_b _ => n
+  | typ_top => n
+  | typ_bot => n
+  | typ_arrow A1 A2 => split_depth_rec Σ A1 (S n) + split_depth_rec Σ A2 (S n)
+  | typ_all A => n + split_depth_rec Σ A n
+  | typ_intersection A1 A2 => n + split_depth_rec Σ A1 n + split_depth_rec Σ A2 n
+  | typ_union A1 A2 => n + split_depth_rec Σ A1 n + split_depth_rec Σ A2 n
+  | _ => 0
   end.
 
-Definition all_size_work (w : work) : nat :=
+Definition split_depth (Σ : aenv) (A : typ) : nat := split_depth_rec Σ A 1.
+
+Definition split_depth_work (Σ : aenv) (w : work) : nat :=
   match w with
-  | work_infer _ _ => 0
-  | work_check _ _ => 0
-  | work_infabs A _ => all_size A
-  | work_infabsunion _ _ _ => 0
-  | work_infapp _ _ _ => 0
-  | work_inftapp _ _ _ => 0
-  | work_sub A1 A2 => all_size A1 + all_size A2
-  | work_inftappunion _ _ _ _ => 0
-  | work_unioninftapp _ _ _ => 0
-  | work_unioninfabs _ _ _ => 0
-  | work_apply _ _ => 0
+  | work_sub A1 A2 => split_depth Σ A1 * (1 + iu_size A2) + split_depth Σ A2 * (1 + iu_size A1)
+  | _ => 0
   end.
 
-Fixpoint all_size_wl (Γ : aworklist) : nat :=
+Fixpoint split_depth_wl (Γ : aworklist) : nat :=
   match Γ with
-  | aworklist_empty => 0 
-  | aworklist_constvar Γ' _ _ => all_size_wl Γ'
-  | aworklist_consvar Γ' _ _ => all_size_wl Γ'
-  | aworklist_conswork Γ' w => all_size_work w + all_size_wl Γ'
+  | aworklist_empty => 0
+  | aworklist_cons_var Γ' _ _ => split_depth_wl Γ'
+  | aworklist_cons_work Γ' w => split_depth_work (awl_to_aenv Γ) w + split_depth_wl Γ'
   end.
 
-Inductive measp : aworklist -> typ -> nat -> Prop :=
-  | measp_typ : forall Γ A m n,
-      split_size Γ A m -> 
-      n = 3 * m + all_size A ->
-      measp Γ A n.
-
-Theorem measp_total : forall Γ A,
-  a_wf_typ (awl_to_aenv Γ) A -> exists n, measp Γ A n.
-Admitted.
-
-Theorem measp_det : forall Γ A n1 n2,
-  measp Γ A n1 -> measp Γ A n2 -> n1 = n2.
-Admitted.
-
-Inductive measp_work : aworklist -> work -> nat -> Prop :=
-  | measp_work_infer : forall Γ e c,
-      measp_work Γ (work_infer e c) 0
-  | measp_work_check : forall Γ e A,
-      measp_work Γ (work_check e A) 0
-  | measp_work_infabs : forall Γ A c,
-      measp_work Γ (work_infabs A c) 0
-  | measp_work_infabsunion : forall Γ A1 A2 c,
-      measp_work Γ (work_infabsunion A1 A2 c) 0
-  | measp_work_infapp : forall Γ A e c,
-      measp_work Γ (work_infapp A e c) 0
-  | measp_work_inftapp : forall Γ A1 A2 c,
-      measp_work Γ (work_inftapp A1 A2 c) 0
-  | measp_work_sub : forall Γ A1 A2 n1 n2 n,
-      measp Γ A1 n1 -> measp Γ A2 n2 ->
-      n = n1 * (1 + iu_size A2) + n2 * (1 + iu_size A1) ->
-      measp_work Γ (work_sub A1 A2) n
-  | measp_work_inftappunion : forall Γ A1 A2 A3 c,
-      measp_work Γ (work_inftappunion A1 A2 A3 c) 0
-  | measp_work_unioninftapp : forall Γ A1 A2 c,
-      measp_work Γ (work_unioninftapp A1 A2 c) 0
-  | measp_work_unioninfabs : forall Γ A1 A2 c,
-      measp_work Γ (work_unioninfabs A1 A2 c) 0
-  | measp_work_apply : forall Γ c A,
-      measp_work Γ (work_apply c A) 0.
-
-Theorem measp_work_total : forall Γ w,
-  a_wf_work (awl_to_aenv Γ) w -> exists n, measp_work Γ w n.
-Admitted.
-
-Theorem measp_work_det : forall Γ w n1 n2,
-  measp_work Γ w n1 -> measp_work Γ w n2 -> n1 = n2.
-Admitted.
-
-Inductive measp_wl : aworklist -> nat -> Prop :=
-  | measp_wl_empty : measp_wl aworklist_empty 0
-  | measp_wl_consevar : forall Γ X n,
-      measp_wl Γ n ->
-      measp_wl (aworklist_constvar Γ X abind_etvar_empty) (S n)
-  | measp_wl_constvar : forall Γ X n,
-      measp_wl Γ n ->
-      measp_wl (aworklist_constvar Γ X abind_tvar_empty) n
-  | measp_wl_conssvar : forall Γ X n,
-      measp_wl Γ n ->
-      measp_wl (aworklist_constvar Γ X abind_stvar_empty) n
-  | measp_wl_consvar : forall Γ X A n,
-      measp_wl Γ n ->
-      measp_wl (aworklist_consvar Γ X A) n
-  | measp_wl_conswork : forall Γ w m n k,
-      measp_work Γ w m ->
-      measp_wl Γ n ->
-      k = m + n ->
-      measp_wl (aworklist_conswork Γ w) k.
-
-#[local]Hint Constructors split_size split_size_work split_size_wl : core.
-#[local]Hint Constructors measp measp_work measp_wl : core.
-#[local]Hint Constructors a_wl_red a_wf_wl : core.
-
-Theorem measp_wl_total : forall Γ,
-  a_wf_wl Γ -> exists n, measp_wl Γ n.
-Admitted.
-
-Theorem measp_wl_det : forall Γ n1 n2,
-  measp_wl Γ n1 -> measp_wl Γ n2 -> n1 = n2.
-Admitted.
-
-Lemma measp_mono' : forall Γ A n,
-  measp Γ A n -> a_mono_typ (awl_to_aenv Γ) A -> n = 0.
-Admitted.
-
-Lemma measp_mono : forall Γ A,
-  a_mono_typ (awl_to_aenv Γ) A -> measp Γ A 0.
+Lemma split_depth_rec_mono : forall Σ A n,
+  ⊢ᵃ Σ -> a_mono_typ Σ A -> split_depth_rec Σ A n = 0.
 Proof.
-  intros Γ A Hmono.
-  eapply a_mono_typ_wf in Hmono as H.
-  eapply measp_total in H.
-  dependent destruction H.
-  eapply measp_mono' in H as H'; eauto.
-  subst. eauto.
+  intros Σ A n Hwf Hmono. generalize dependent n.
+  induction A; simpl; eauto; intros; try solve [inversion Hmono].
+  - dependent destruction Hmono;
+      apply binds_lookup_tvar_bind in H; eauto;
+      rewrite H; auto. 
+  - dependent destruction Hmono.
+    specialize (IHA1 Hmono1 (S n)). specialize (IHA2 Hmono2 (S n)). lia.
 Qed.
 
-Lemma measp_top' : forall Γ n,
-  measp Γ typ_top n -> n = 0.
+Lemma split_depth_mono : forall Σ A,
+  ⊢ᵃ Σ -> a_mono_typ Σ A -> split_depth Σ A = 0.
 Proof.
-  intros. dependent destruction H.
-  dependent destruction H. simpl. lia.
-Qed.
-
-Lemma measp_bot : forall Γ n,
-  measp Γ typ_bot n -> n = 0.
-Proof.
-  intros. dependent destruction H.
-  dependent destruction H. simpl. lia.
+  intros. unfold split_depth. eapply split_depth_rec_mono; eauto.
 Qed.
 
 Fixpoint weight (A : typ) : nat :=
@@ -389,9 +190,8 @@ Definition weight_work (w : work) : nat :=
 Fixpoint weight_wl (Γ : aworklist) : nat :=
   match Γ with
   | aworklist_empty => 0 
-  | aworklist_constvar Γ' _ _ => 1 + weight_wl Γ'
-  | aworklist_consvar Γ' _ _ => 1 + weight_wl Γ'
-  | aworklist_conswork Γ' w => weight_work w + weight_wl Γ'
+  | aworklist_cons_var Γ' _ _ => 1 + weight_wl Γ'
+  | aworklist_cons_work Γ' w => weight_work w + weight_wl Γ'
   end.
 
 #[local]Hint Constructors a_wl_red a_wf_wl : core.
@@ -408,53 +208,35 @@ Fixpoint infabs_depth (A : typ) : nat :=
   | _ => 0
   end.
 
-Fixpoint infabs_depth_cont (c : cont) : nat :=
-  match c with
-  | cont_infabs c => 1 + infabs_depth_cont c
-  | cont_infabsunion A c => 1 + infabs_depth A + infabs_depth_cont c
-  | cont_unioninfabs _ c => 1 + infabs_depth_cont c
+Fixpoint infabs_depth_contd (cd : contd) : nat :=
+  match cd with
+  | contd_infabsunion A cd => 1 + infabs_depth A + infabs_depth_contd cd
+  | contd_unioninfabs _ _ cd => 1 + infabs_depth_contd cd
+  | _ => 0
+  end.
+
+Definition infabs_depth_conts (cs : conts) : nat :=
+  match cs with
+  | conts_infabs cd => 1 + infabs_depth_contd cd
   | _ => 0
   end.
 
 Definition infabs_depth_work (w : work) : nat :=
   match w with
-  | work_infabs A c => infabs_depth A + infabs_depth_cont c
-  | work_infabsunion _ A c => 1 + infabs_depth A + infabs_depth_cont c
-  | work_unioninfabs _ _ c => 1 + infabs_depth_cont c
+  | work_infabs A c => infabs_depth A + infabs_depth_contd c
+  | work_infabsunion _ _ A c => 1 + infabs_depth A + infabs_depth_contd c
+  | work_unioninfabs _ _ _ _ c => 1 + infabs_depth_contd c
   | _ => 0
   end.
 
 Fixpoint infabs_depth_wl (Γ : aworklist) : nat :=
   match Γ with
   | aworklist_empty => 0 
-  | aworklist_constvar Γ' _ _ => infabs_depth_wl Γ'
-  | aworklist_consvar Γ' _ _ => infabs_depth_wl Γ'
-  | aworklist_conswork Γ' w => infabs_depth_work w + infabs_depth_wl Γ'
+  | aworklist_cons_var Γ' _ _ => infabs_depth_wl Γ'
+  | aworklist_cons_work Γ' w => infabs_depth_work w + infabs_depth_wl Γ'
   end.
 
 #[local]Hint Unfold infabs_depth infabs_depth_work infabs_depth_wl : core.
-
-Fixpoint inftapp_all_size (A : typ) : nat :=
-  match A with
-  | typ_all A => 1 + inftapp_all_size A
-  | typ_union A1 A2 => inftapp_all_size A1 + inftapp_all_size A2
-  | typ_intersection A1 A2 => inftapp_all_size A1 + inftapp_all_size A2
-  | _ => 0
-  end.
-
-Definition inftapp_all_size_work (w : work) : nat :=
-  match w with
-  | work_inftapp A _ _ => inftapp_all_size A
-  | _ => 0
-  end.
-
-Fixpoint inftapp_all_size_wl (Γ : aworklist) : nat :=
-  match Γ with
-  | aworklist_empty => 0 
-  | aworklist_constvar Γ' _ _ => inftapp_all_size_wl Γ'
-  | aworklist_consvar Γ' _ _ => inftapp_all_size_wl Γ'
-  | aworklist_conswork Γ' w => inftapp_all_size_work w + inftapp_all_size_wl Γ'
-  end.
 
 Fixpoint inftapp_depth (A : typ) : nat :=
   match A with
@@ -465,209 +247,194 @@ Fixpoint inftapp_depth (A : typ) : nat :=
   | _ => 0
   end.
 
-Fixpoint inftapp_depth_cont_tail_rec (c : cont) (ans : nat) : nat :=
-  match c with
-  | cont_inftapp B c        => inftapp_depth_cont_tail_rec c ((2 + inftapp_depth B) * ans)
-  | cont_inftappunion A B c => inftapp_depth_cont_tail_rec c ((inftapp_depth A) * (2 + inftapp_depth B) + 1 + ans)
-  | cont_infabs c           => inftapp_depth_cont_tail_rec c ans
-  | cont_infabsunion _ c    => inftapp_depth_cont_tail_rec c ans
-  | cont_infapp _ c         => inftapp_depth_cont_tail_rec c ans
-  | cont_unioninftapp A c   => inftapp_depth_cont_tail_rec c (1 + inftapp_depth A + ans)
-  | cont_unioninfabs _ c    => inftapp_depth_cont_tail_rec c ans
-  | _                       => ans
+Fixpoint inftapp_depth_conts_tail_rec (cs : conts) (ans : nat) : nat :=
+  match cs with
+  | conts_infabs cd            => inftapp_depth_contd_tail_rec cd ans
+  | conts_inftapp B cs         => inftapp_depth_conts_tail_rec cs ((2 + inftapp_depth B) * ans)
+  | conts_inftappunion A B cs  => inftapp_depth_conts_tail_rec cs ((inftapp_depth A) * (2 + inftapp_depth B) + 1 + ans)
+  | conts_unioninftapp A cs    => inftapp_depth_conts_tail_rec cs (1 + inftapp_depth A + ans)
+  | _                          => ans
+  end
+with inftapp_depth_contd_tail_rec (cd : contd) (ans : nat) : nat :=
+  match cd with
+  | contd_infabsunion _ cd => inftapp_depth_contd_tail_rec cd ans
+  | contd_infapp _ _ cs => inftapp_depth_conts_tail_rec cs ans
+  | contd_unioninfabs _ _ cd => inftapp_depth_contd_tail_rec cd ans
   end.
 
 Definition inftapp_depth_work (w : work) : nat :=
   match w with
-  | work_inftapp A B c => inftapp_depth_cont_tail_rec (cont_inftapp B c) (inftapp_depth A)
-  | work_inftappunion A1 A2 B c => inftapp_depth_cont_tail_rec c (inftapp_depth A1 + (inftapp_depth A2) * (2 + inftapp_depth B) + 1)
-  | work_infer _ c => inftapp_depth_cont_tail_rec c 0
-  | work_infabs _ c => inftapp_depth_cont_tail_rec c 0
-  | work_infabsunion _ _ c => inftapp_depth_cont_tail_rec c 0
-  | work_infapp _ _ c => inftapp_depth_cont_tail_rec c 0
-  | work_unioninftapp A1 A2 c => inftapp_depth_cont_tail_rec c (1 + inftapp_depth A1 + inftapp_depth A2)
-  | work_unioninfabs _ _ c => inftapp_depth_cont_tail_rec c 0
+  | work_inftapp A B cs => inftapp_depth_conts_tail_rec (conts_inftapp B cs) (inftapp_depth A)
+  | work_inftappunion A1 A2 B cs => inftapp_depth_conts_tail_rec cs (inftapp_depth A1 + (inftapp_depth A2) * (2 + inftapp_depth B) + 1)
+  | work_infer _ cs => inftapp_depth_conts_tail_rec cs 0
+  | work_infabs _ cd => inftapp_depth_contd_tail_rec cd 0
+  | work_infabsunion _ _ _ cd => inftapp_depth_contd_tail_rec cd 0
+  | work_infapp _ _ _ cs => inftapp_depth_conts_tail_rec cs 0
+  | work_unioninftapp A1 A2 cs => inftapp_depth_conts_tail_rec cs (1 + inftapp_depth A1 + inftapp_depth A2)
+  | work_unioninfabs _ _ _ _ cd => inftapp_depth_contd_tail_rec cd 0
   | _ => 0
   end.
 
 Fixpoint inftapp_depth_wl (Γ : aworklist) : nat :=
   match Γ with
-  | aworklist_empty => 0 
-  | aworklist_constvar Γ' _ _ => inftapp_depth_wl Γ'
-  | aworklist_consvar Γ' _ _ => inftapp_depth_wl Γ'
-  | aworklist_conswork Γ' w => inftapp_depth_work w + inftapp_depth_wl Γ'
+  | aworklist_empty => 0
+  | aworklist_cons_var Γ' _ _ => inftapp_depth_wl Γ'
+  | aworklist_cons_work Γ' w => inftapp_depth_work w + inftapp_depth_wl Γ'
   end.
 
-#[local] Hint Unfold inftapp_depth_cont_tail_rec inftapp_depth inftapp_depth_work inftapp_depth_wl : core.
+#[local] Hint Unfold inftapp_depth_conts_tail_rec inftapp_depth_contd_tail_rec inftapp_depth inftapp_depth_work inftapp_depth_wl : core.
 
-Fixpoint infabs_judge_size_cont (c : cont) : nat :=
-  match c with
-  | cont_infabs c => 1 + infabs_judge_size_cont c
-  | cont_infabsunion _ c => 3 + infabs_judge_size_cont c
-  | cont_infapp _ c => infabs_judge_size_cont c
-  | cont_inftapp _ c => infabs_judge_size_cont c
-  | cont_inftappunion _ _ c => infabs_judge_size_cont c
-  | cont_unioninftapp _ c => infabs_judge_size_cont c
-  | cont_unioninfabs _ c => 1 + infabs_judge_size_cont c
-  | cont_sub A => 0
+Fixpoint infabs_judge_size_conts (cs : conts) : nat :=
+  match cs with
+  | conts_infabs cd => 1 + infabs_judge_size_contd cd
+  | conts_inftapp _ cs => infabs_judge_size_conts cs
+  | conts_inftappunion _ _ cs => infabs_judge_size_conts cs
+  | conts_unioninftapp _ cs => infabs_judge_size_conts cs
+  | conts_sub _ => 0
+  end
+with infabs_judge_size_contd (cd : contd) : nat :=
+  match cd with
+  | contd_infabsunion _ cd => 3 + infabs_judge_size_contd cd
+  | contd_infapp _ _ cs => infabs_judge_size_conts cs
+  | contd_unioninfabs _ _ cd => 1 + infabs_judge_size_contd cd
   end.
 
 Definition infabs_judge_size_work (w : work) : nat :=
   match w with
-  | work_infer _ c => infabs_judge_size_cont c
+  | work_infer _ cs => infabs_judge_size_conts cs
   | work_check _ _ => 0
-  | work_infabs _ c => 1 + infabs_judge_size_cont c
-  | work_infabsunion _ _ c => 3 + infabs_judge_size_cont c
-  | work_infapp _ _ c => infabs_judge_size_cont c
-  | work_inftapp _ _ c => infabs_judge_size_cont c
+  | work_infabs _ cd => 1 + infabs_judge_size_contd cd
+  | work_infabsunion _ _ _ cd => 3 + infabs_judge_size_contd cd
+  | work_infapp _ _ _ cs => infabs_judge_size_conts cs
+  | work_inftapp _ _ cs => infabs_judge_size_conts cs
   | work_sub _ _ => 0
-  | work_inftappunion _ _ _ c => infabs_judge_size_cont c
-  | work_unioninftapp _ _ c => infabs_judge_size_cont c
-  | work_unioninfabs _ _ c => 1 + infabs_judge_size_cont c
-  | work_apply c _ => infabs_judge_size_cont c
+  | work_inftappunion _ _ _ cs => infabs_judge_size_conts cs
+  | work_unioninftapp _ _ cs => infabs_judge_size_conts cs
+  | work_unioninfabs _ _ _ _ cd => 1 + infabs_judge_size_contd cd
+  | work_applys cs _ => infabs_judge_size_conts cs
+  | work_applyd cd _ _ => infabs_judge_size_contd cd
   end.
 
 Fixpoint infabs_judge_size_wl (Γ : aworklist) : nat :=
   match Γ with
-  | aworklist_empty => 0 
-  | aworklist_constvar Γ' _ _ => infabs_judge_size_wl Γ'
-  | aworklist_consvar Γ' _ _ => infabs_judge_size_wl Γ'
-  | aworklist_conswork Γ' w => infabs_judge_size_work w + infabs_judge_size_wl Γ'
+  | aworklist_empty => 0
+  | aworklist_cons_var Γ' _ _ => infabs_judge_size_wl Γ'
+  | aworklist_cons_work Γ' w => infabs_judge_size_work w + infabs_judge_size_wl Γ'
   end.
 
-Fixpoint inftapp_judge_size_cont (c : cont) : nat :=
-  match c with
-  | cont_infabs c => inftapp_judge_size_cont c
-  | cont_infabsunion _ c => inftapp_judge_size_cont c
-  | cont_infapp _ c => inftapp_judge_size_cont c
-  | cont_inftapp _ c => 1 + inftapp_judge_size_cont c
-  | cont_inftappunion _ _ c => 3 + inftapp_judge_size_cont c
-  | cont_unioninftapp _ c => 1 + inftapp_judge_size_cont c
-  | cont_unioninfabs _ c => inftapp_judge_size_cont c
-  | cont_sub A => 0
+Fixpoint inftapp_judge_size_conts (cs : conts) : nat :=
+  match cs with
+  | conts_infabs cd => inftapp_judge_size_contd cd
+  | conts_inftapp _ cs => 1 + inftapp_judge_size_conts cs
+  | conts_inftappunion _ _ cs => 3 + inftapp_judge_size_conts cs
+  | conts_unioninftapp _ cs => 1 + inftapp_judge_size_conts cs
+  | conts_sub _ => 0
+  end
+with inftapp_judge_size_contd (cd : contd) : nat :=
+  match cd with
+  | contd_infabsunion _ cd => inftapp_judge_size_contd cd
+  | contd_infapp _ _ cs => inftapp_judge_size_conts cs
+  | contd_unioninfabs _ _ cd => inftapp_judge_size_contd cd
   end.
 
 Definition inftapp_judge_size_work (w : work) : nat :=
   match w with
-  | work_infer _ c => inftapp_judge_size_cont c
+  | work_infer _ cs => inftapp_judge_size_conts cs
   | work_check _ _ => 0
-  | work_infabs _ c => inftapp_judge_size_cont c
-  | work_infabsunion _ _ c => inftapp_judge_size_cont c
-  | work_infapp _ _ c => inftapp_judge_size_cont c
-  | work_inftapp _ _ c => 1 + inftapp_judge_size_cont c
+  | work_infabs _ cd => inftapp_judge_size_contd cd
+  | work_infabsunion _ _ _ cd => inftapp_judge_size_contd cd
+  | work_infapp _ _ _ cs => inftapp_judge_size_conts cs
+  | work_inftapp _ _ cs => 1 + inftapp_judge_size_conts cs
   | work_sub _ _ => 0
-  | work_inftappunion _ _ _ c => 3 + inftapp_judge_size_cont c
-  | work_unioninftapp _ _ c => 1 + inftapp_judge_size_cont c
-  | work_unioninfabs _ _ c => inftapp_judge_size_cont c
-  | work_apply c _ => inftapp_judge_size_cont c
+  | work_inftappunion _ _ _ cs => 3 + inftapp_judge_size_conts cs
+  | work_unioninftapp _ _ cs => 1 + inftapp_judge_size_conts cs
+  | work_unioninfabs _ _ _ _ cd => inftapp_judge_size_contd cd
+  | work_applys cs _ => inftapp_judge_size_conts cs
+  | work_applyd cd _ _ => inftapp_judge_size_contd cd
   end.
 
 Fixpoint inftapp_judge_size_wl (Γ : aworklist) : nat :=
   match Γ with
-  | aworklist_empty => 0 
-  | aworklist_constvar Γ' _ _ => inftapp_judge_size_wl Γ'
-  | aworklist_consvar Γ' _ _ => inftapp_judge_size_wl Γ'
-  | aworklist_conswork Γ' w => inftapp_judge_size_work w + inftapp_judge_size_wl Γ'
+  | aworklist_empty => 0
+  | aworklist_cons_var Γ' _ _ => inftapp_judge_size_wl Γ'
+  | aworklist_cons_work Γ' w => inftapp_judge_size_work w + inftapp_judge_size_wl Γ'
   end.
 
-Lemma abind_etvar_tvar_false : forall Γ X,
-  a_wf_wl Γ ->
-  binds X abind_etvar_empty (awl_to_aenv Γ) ->
-  binds X abind_tvar_empty (awl_to_aenv Γ) -> False.
-Admitted.
-
-Lemma abind_etvar_stvar_false : forall Γ X,
-  a_wf_wl Γ ->
-  binds X abind_etvar_empty (awl_to_aenv Γ) ->
-  binds X abind_stvar_empty (awl_to_aenv Γ) -> False.
-Admitted.
-
-Lemma abind_tvar_stvar_false : forall Γ X,
-  a_wf_wl Γ ->
-  binds X abind_tvar_empty (awl_to_aenv Γ) ->
-  binds X abind_stvar_empty (awl_to_aenv Γ) -> False.
-Admitted.
-
-Lemma iu_size_mono : forall Γ A,
-  a_mono_typ Γ A -> iu_size A = 0.
+Lemma iuv_size_mono : forall Σ A,
+  Σ ᵗ⊢ᵃₘ A -> iuv_size A = 0.
 Proof.
-  intros Γ A Hmono.
+  intros Σ A Hmono.
   induction Hmono; simpl; eauto; try lia.
 Qed.
 
-Lemma iu_size_subst_mono : forall Γ A X A0,
-  a_mono_typ Γ A ->
-  iu_size (subst_tvar_in_typ A X A0) = iu_size A0.
+Lemma iuv_size_subst_mono : forall Σ A X A0,
+  Σ ᵗ⊢ᵃₘ A ->
+  iuv_size (subst_tvar_in_typ A X A0) = iuv_size A0.
 Proof.
-  intros Γ A X A0 Hmono.
+  intros Σ A X A0 Hmono.
   induction A0; simpl; auto.
   destruct (eq_dec X0 X); subst; simpl; eauto.
-  eapply iu_size_mono; eauto.
+  eapply iuv_size_mono; eauto.
 Qed.
 
-Lemma exp_size_wl_awl_app : forall Γ1 Γ2,
-  exp_size_wl (awl_app Γ1 Γ2) = exp_size_wl Γ1 + exp_size_wl Γ2.
+Lemma exp_split_size_subst_tvar_in_exp_mono : forall n Σ A X e,
+  size_exp e < n ->
+  Σ ᵗ⊢ᵃₘ A -> exp_split_size Σ ({A ᵉ/ₜ X} e) = exp_split_size Σ e.
 Proof.
-  intros Γ1.
-  induction Γ1; simpl; auto;
-    try solve [intros; rewrite IHΓ1; simpl; lia].
+  intro n. induction n; try lia.
+  intros Σ A X e Hsize Hmono.
+  destruct e; simpl in *; eauto.
+  - erewrite IHn; eauto; try lia.
+  - erewrite IHn; eauto; try lia.
+    erewrite IHn; eauto; try lia.
+  - destruct body5. simpl in *.
+    erewrite IHn; eauto; try lia.
+    erewrite iuv_size_subst_mono; eauto.
+  - erewrite IHn; eauto; try lia.
+    erewrite iuv_size_subst_mono; eauto.
+  - erewrite IHn; eauto; try lia.
+    erewrite iuv_size_subst_mono; eauto.
 Qed.
 
 Lemma exp_size_subst_tvar_in_exp_mono : forall Γ A X e,
-  a_mono_typ Γ A ->
-  exp_size (subst_tvar_in_exp A X e) = exp_size e
+  ⌊ Γ ⌋ᵃ ᵗ⊢ᵃₘ A ->
+  exp_size Γ ({A ᵉ/ₜ X} e) = exp_size Γ e
 with body_size_subst_tvar_in_body_mono : forall Γ A X b,
-  a_mono_typ Γ A ->
-  body_size (subst_tvar_in_body A X b) = body_size b.
+  ⌊ Γ ⌋ᵃ ᵗ⊢ᵃₘ A ->
+  body_size Γ ({A ᵇ/ₜ X} b) = body_size Γ b.
 Proof.
   - intros Γ A X e Hmono.
-  induction e; simpl; eauto.
-  erewrite iu_size_subst_mono; eauto.
-  - intros. destruct b. simpl. 
-  erewrite iu_size_subst_mono; eauto. 
+    induction e; simpl; eauto.
+    erewrite IHe1. erewrite exp_split_size_subst_tvar_in_exp_mono; eauto.
+    erewrite IHe. erewrite iu_size_subst_mono; eauto.
+  - intros. destruct b. simpl.
+    erewrite iu_size_subst_mono; eauto. 
 Qed.
 
-Lemma exp_size_cont_subst_tvar_in_cont_mono : forall Γ X A c,
-  a_mono_typ Γ A ->
-  exp_size_cont (subst_tvar_in_conts A X c) = exp_size_cont c.
+Lemma exp_size_conts_subst_tvar_in_conts_mono : forall Γ X A c,
+  ⌊ Γ ⌋ᵃ ᵗ⊢ᵃₘ A ->
+  exp_size_conts Γ ({A ᶜˢ/ₜ X} c) = exp_size_conts Γ c
+with exp_size_contd_subst_tvar_in_contd_mono : forall Γ X A c,
+  ⌊ Γ ⌋ᵃ ᵗ⊢ᵃₘ A ->
+  exp_size_contd Γ ({A ᶜᵈ/ₜ X} c) = exp_size_contd Γ c.
 Proof.
+  intros Γ X A c Hmono.
+  induction c; simpl; eauto.
   intros Γ X A c Hmono.
   induction c; simpl; eauto.
   erewrite exp_size_subst_tvar_in_exp_mono; eauto.
 Qed.
 
 Lemma exp_size_work_subst_tvar_in_work_mono : forall Γ X A w,
-  a_mono_typ Γ A ->
-  exp_size_work (subst_tvar_in_work A X w) = exp_size_work w.
+  ⌊ Γ ⌋ᵃ ᵗ⊢ᵃₘ A ->
+  exp_size_work Γ ({A ʷ/ₜ X} w) = exp_size_work Γ w.
 Proof.
   intros Γ X A w Hmono.
   induction w; intros; simpl;
     try erewrite exp_size_subst_tvar_in_exp_mono;
-    try erewrite exp_size_cont_subst_tvar_in_cont_mono;
+    try erewrite exp_size_conts_subst_tvar_in_conts_mono;
+    try erewrite exp_size_contd_subst_tvar_in_contd_mono;
     try erewrite iu_size_subst_mono; eauto.
-Qed.
-
-Lemma exp_size_wl_subst_tvar_in_aworklist_mono : forall Γ Γ' X A,
-  a_mono_typ Γ' A ->
-  exp_size_wl (subst_tvar_in_aworklist A X Γ) = exp_size_wl Γ.
-Proof.
-  intros Γ.
-  induction Γ; intros; simpl in *;
-    try erewrite exp_size_work_subst_tvar_in_work_mono; eauto.
-Qed. 
-
-Lemma exp_size_wl_aworklist_subst : forall Γ X A E Γ1 Γ2,
-  aworklist_subst Γ X A E Γ1 Γ2 ->
-  exp_size_wl Γ = exp_size_wl Γ1 + exp_size_wl Γ2.
-Proof.
-  intros Γ X A E Γ1 Γ2 Hsubst.
-  induction Hsubst; simpl; auto; try lia.
-Qed.
-
-Lemma exp_size_wl_etvar_list : forall E,
-  exp_size_wl (etvar_list_to_awl E) = 0.
-Proof.
-  induction E; simpl; auto.
 Qed.
 
 Lemma judge_size_wl_awl_app : forall Γ1 Γ2,
@@ -678,11 +445,16 @@ Proof.
     try solve [intros; rewrite IHΓ1; simpl; lia].
 Qed.
 
-Lemma judge_size_cont_subst_tvar_in_cont : forall X A c,
-  judge_size_cont (subst_tvar_in_conts A X c) = judge_size_cont c.
+Lemma judge_size_conts_subst_tvar_in_conts : forall X A c,
+  judge_size_conts (subst_tvar_in_conts A X c) = judge_size_conts c
+with judge_size_contd_subst_tvar_in_contd : forall X A c,
+  judge_size_contd (subst_tvar_in_contd A X c) = judge_size_contd c.
 Proof.
   intros X A c.
   induction c; simpl; eauto.
+  intros X A c.
+  induction c; simpl; eauto.
+  erewrite judge_size_conts_subst_tvar_in_conts; eauto.
 Qed.
 
 Lemma judge_size_work_subst_tvar_in_work : forall X A w,
@@ -690,7 +462,8 @@ Lemma judge_size_work_subst_tvar_in_work : forall X A w,
 Proof.
   intros X A w.
   induction w; intros; simpl;
-    try erewrite judge_size_cont_subst_tvar_in_cont; eauto.
+    try erewrite judge_size_conts_subst_tvar_in_conts;
+    try erewrite judge_size_contd_subst_tvar_in_contd; eauto.
 Qed.
 
 Lemma judge_size_wl_subst_tvar_in_aworklist : forall Γ X A,
@@ -701,145 +474,153 @@ Proof.
     try erewrite judge_size_work_subst_tvar_in_work; eauto.
 Qed. 
 
-Lemma judge_size_wl_aworklist_subst : forall Γ X A E Γ1 Γ2,
-  aworklist_subst Γ X A E Γ1 Γ2 ->
-  judge_size_wl Γ = judge_size_wl Γ1 + judge_size_wl Γ2.
-Proof.
-  intros Γ X A E Γ1 Γ2 Hsubst.
-  induction Hsubst; simpl; auto; try lia.
-Qed.
-
-Lemma judge_size_wl_etvar_list : forall E,
-  judge_size_wl (etvar_list_to_awl E) = 0.
-Proof.
-  induction E; simpl; auto.
-Qed.
-
-Lemma measp_wl_aworklist_subst : forall Γ X A E Γ1 Γ2 n,
-  aworklist_subst Γ X A E Γ1 Γ2 ->
-  measp_wl Γ n ->
-  measp_wl
-    (awl_app (subst_tvar_in_aworklist A X Γ2)
-      (awl_app (etvar_list_to_awl E) Γ1)) n.
-Proof.
-  intros Γ X A E Γ1 Γ2 n Hsubst Hmeas.
-  induction Hsubst; simpl.
-  (* rev? *)
-Abort.
-
-Lemma apply_cont_det : forall c A w1 w2,
-  apply_cont c A w1 -> apply_cont c A w2 -> w1 = w2.
+Lemma apply_conts_det : forall c A w1 w2,
+  apply_conts c A w1 -> apply_conts c A w2 -> w1 = w2.
 Proof.
   intros c A w1 w2 Happly1 Happly2.
   induction Happly1; dependent destruction Happly2; eauto.
 Qed.
 
-Lemma apply_cont_dec : forall c A,
-  (exists w, apply_cont c A w) \/ ((exists w, apply_cont c A w) -> False).
+Lemma apply_contd_det : forall c A B w1 w2,
+  apply_contd c A B w1 -> apply_contd c A B w2 -> w1 = w2.
+Proof.
+  intros c A B w1 w2 Happly1 Happly2.
+  induction Happly1; dependent destruction Happly2; eauto.
+Qed.
+
+Lemma apply_conts_dec : forall c A,
+  (exists w, apply_conts c A w) \/ ((exists w, apply_conts c A w) -> False).
 Proof.
   intros c A.
-  destruct c; eauto using apply_cont.
-  - destruct A;
-      try solve [right; intros Hcontra; dependent destruction Hcontra; dependent destruction H];
-      eauto using apply_cont.
-  - destruct A;
-      try solve [right; intros Hcontra; dependent destruction Hcontra; dependent destruction H].
-    destruct A2;
-      try solve [right; intros Hcontra; dependent destruction Hcontra; dependent destruction H];
-      eauto using apply_cont.
+  destruct c; eauto using apply_conts.
 Qed.
 
-Lemma apply_cont_exp_size : forall c A w,
-  apply_cont c A w -> exp_size_work w = exp_size_cont c.
+Lemma apply_contd_dec : forall c A B,
+  (exists w, apply_contd c A B w) \/ ((exists w, apply_contd c A B w) -> False).
+Proof.
+  intros c A B.
+  destruct c; eauto using apply_contd.
+  destruct (le_lt_dec (iu_size A) n); eauto.
+  right. intros [w Happly]. dependent destruction Happly. lia.
+Qed.
+
+Lemma apply_conts_exp_size : forall Γ c A w,
+  apply_conts c A w -> exp_size_work Γ w = exp_size_conts Γ c.
+Proof.
+  intros Γ c A w Happly.
+  induction Happly; simpl; eauto.
+Qed.
+
+Lemma apply_contd_exp_size : forall Γ c A B w,
+  apply_contd c A B w -> exp_size_work Γ w <= exp_size_contd Γ c.
+Proof.
+  intros Γ c A B w Happly.
+  induction Happly; simpl; eauto; try lia.
+  assert (exp_size Γ e * S (iu_size A) <= exp_size Γ e * S n).
+  { eapply mult_le_compat; eauto. lia. } lia.
+Qed.
+
+Lemma apply_conts_judge_size : forall c A w,
+  apply_conts c A w -> judge_size_work w = judge_size_conts c.
 Proof.
   intros c A w Happly.
   induction Happly; simpl; eauto.
 Qed.
 
-Lemma apply_cont_judge_size : forall c A w,
-  apply_cont c A w -> judge_size_work w = judge_size_cont c.
+Lemma apply_contd_judge_size : forall c A B w,
+  apply_contd c A B w -> judge_size_work w = judge_size_contd c.
 Proof.
-  intros c A w Happly.
+  intros c A B w Happly.
   induction Happly; simpl; eauto.
 Qed.
 
-Lemma apply_cont_infabs_depth_arr : forall c A B w,
-  apply_cont c (typ_arrow A B) w -> infabs_depth_work w <= infabs_depth_cont c.
+Lemma apply_contd_infabs_depth : forall c A B w,
+  apply_contd c A B w -> infabs_depth_work w = infabs_depth_contd c.
 Proof.
   intros c A B w Happly.
   dependent destruction Happly; simpl; eauto.
 Qed.
 
-Lemma inftapp_depth_cont_tail_rec_le : forall c ans1 ans2,
+Lemma inftapp_depth_conts_tail_rec_le : forall c ans1 ans2,
   ans1 <= ans2 ->
-  inftapp_depth_cont_tail_rec c ans1 <= inftapp_depth_cont_tail_rec c ans2.
+  inftapp_depth_conts_tail_rec c ans1 <= inftapp_depth_conts_tail_rec c ans2
+with inftapp_depth_contd_tail_rec_le : forall c ans1 ans2,
+  ans1 <= ans2 ->
+  inftapp_depth_contd_tail_rec c ans1 <= inftapp_depth_contd_tail_rec c ans2.
 Proof.
   intros c.
   induction c; intros; simpl; eauto; try eapply IHc; try lia.
   assert (inftapp_depth A * ans1 <= inftapp_depth A * ans2).
   { eapply mult_le_compat; eauto. } lia.
+  intros c.
+  induction c; intros; simpl; eauto; try eapply IHc; try lia.
 Qed.
 
-Lemma inftapp_depth_cont_tail_rec_lt : forall c ans1 ans2,
+Lemma inftapp_depth_conts_tail_rec_lt : forall c ans1 ans2,
   ans1 < ans2 ->
-  inftapp_depth_cont_tail_rec c ans1 < inftapp_depth_cont_tail_rec c ans2.
+  inftapp_depth_conts_tail_rec c ans1 < inftapp_depth_conts_tail_rec c ans2
+with inftapp_depth_contd_tail_rec_lt : forall c ans1 ans2,
+  ans1 < ans2 ->
+  inftapp_depth_contd_tail_rec c ans1 < inftapp_depth_contd_tail_rec c ans2.
 Proof.
   intros c.
   induction c; intros; simpl; eauto; try eapply IHc; try lia.
   assert (inftapp_depth A * ans1 <= inftapp_depth A * ans2).
   { eapply mult_le_compat; eauto. lia. } lia.
+  intros c.
+  induction c; intros; simpl; eauto; try eapply IHc; try lia.
 Qed.
 
-Lemma apply_cont_inftapp_depth_arr : forall c A B w,
-  apply_cont c (typ_arrow A B) w -> inftapp_depth_work w <= inftapp_depth_cont_tail_rec c 0.
+Lemma apply_contd_inftapp_depth : forall c A B w,
+  apply_contd c A B w -> inftapp_depth_work w <= inftapp_depth_contd_tail_rec c 0.
 Proof.
   intros c A B w Happly.
   dependent destruction Happly; try solve [simpl; eauto].
-  simpl. eapply inftapp_depth_cont_tail_rec_le; lia.
 Qed.
 
-Lemma apply_cont_inftapp_all_size_arr : forall c A B w,
-  apply_cont c (typ_arrow A B) w -> inftapp_all_size_work w = 0.
+Lemma apply_conts_inftapp_depth_bot : forall c w,
+  apply_conts c typ_bot w -> inftapp_depth_work w <= inftapp_depth_conts_tail_rec c 0.
+Proof.
+  intros c w Happly.
+  dependent destruction Happly; simpl; eauto.
+  simpl. eapply inftapp_depth_conts_tail_rec_le; lia.
+Qed.
+
+Lemma apply_contd_infabs_judge_size : forall c A B w,
+  apply_contd c A B w -> infabs_judge_size_work w = infabs_judge_size_contd c.
 Proof.
   intros c A B w Happly.
-  dependent destruction Happly; simpl; eauto.
-Qed.
+  induction Happly; simpl; eauto.
+Qed. 
 
-Lemma apply_cont_inftapp_depth_bot : forall c w,
-  apply_cont c typ_bot w -> inftapp_depth_work w <= inftapp_depth_cont_tail_rec c 0.
-Proof.
-  intros c w Happly.
-  dependent destruction Happly; simpl; eauto.
-  simpl. eapply inftapp_depth_cont_tail_rec_le; lia.
-Qed.
-
-Lemma apply_cont_inftapp_all_size_bot : forall c w,
-  apply_cont c typ_bot w -> inftapp_all_size_work w = 0.
-Proof.
-  intros c w Happly.
-  dependent destruction Happly; simpl; eauto.
-Qed.
-
-Lemma apply_cont_infabs_judge_size : forall c A w,
-  apply_cont c A w -> infabs_judge_size_work w = infabs_judge_size_cont c.
+Lemma apply_conts_infabs_judge_size : forall c A w,
+  apply_conts c A w -> infabs_judge_size_work w = infabs_judge_size_conts c.
 Proof.
   intros c A w Happly.
   induction Happly; simpl; eauto.
 Qed.
 
-Lemma apply_cont_inftapp_judge_size : forall c A w,
-  apply_cont c A w -> inftapp_judge_size_work w = inftapp_judge_size_cont c.
+Lemma apply_contd_inftapp_judge_size : forall c A B w,
+  apply_contd c A B w -> inftapp_judge_size_work w = inftapp_judge_size_contd c.
+Proof.
+  intros c A B w Happly.
+  induction Happly; simpl; eauto.
+Qed.
+
+Lemma apply_conts_inftapp_judge_size : forall c A w,
+  apply_conts c A w -> inftapp_judge_size_work w = inftapp_judge_size_conts c.
 Proof.
   intros c A w Happly.
   induction Happly; simpl; eauto.
 Qed.
 
-Lemma apply_cont_inftapp_depth : forall c A w,
-  apply_cont c A w -> inftapp_depth_work w <= inftapp_depth_cont_tail_rec c (inftapp_depth A).
+Lemma apply_conts_inftapp_depth : forall c A w,
+  apply_conts c A w -> inftapp_depth_work w <= inftapp_depth_conts_tail_rec c (inftapp_depth A).
 Proof.
   intros c A w Happly.
   induction Happly; simpl;
-    try eapply inftapp_depth_cont_tail_rec_le; try lia.
+    try eapply inftapp_depth_conts_tail_rec_le;
+    try eapply inftapp_depth_contd_tail_rec_le; try lia.
 Qed.
 
 Lemma inftapp_depth_open_typ_wrt_typ_rec : forall A B n,
@@ -861,15 +642,471 @@ Proof.
   apply inftapp_depth_open_typ_wrt_typ_rec.
 Qed.
 
-Lemma decidablity_lemma : forall ne nj nt ntj na naj nm nw Γ m,
-  ⊢ᵃʷ Γ ->
+Lemma a_wf_twl_binds_etvar_aworklist_subst_dec' : forall Γ1 Γ2 X A,
+  ⊢ᵃʷₜ (Γ2 ⧺ X ~ᵃ ⬒ ;ᵃ Γ1) -> 
+  (exists Γ'1 Γ'2, aworklist_subst (Γ2 ⧺ X ~ᵃ ⬒ ;ᵃ Γ1) X A Γ'1 Γ'2) \/ ~ (exists Γ'1 Γ'2, aworklist_subst (Γ2 ⧺ X ~ᵃ ⬒ ;ᵃ Γ1) X A Γ'1 Γ'2).
+Proof with eauto.
+  intros. generalize dependent Γ1. induction Γ2.
+  - left. exists Γ1, aworklist_empty. simpl. constructor.
+  - intros. assert (X0 `in` ftvar_in_typ A \/ (~ X0 `in` ftvar_in_typ A)) by fsetdec. 
+    dependent destruction H.
+    + apply IHΓ2 in H1. destruct H1.
+      * destruct H1 as [Γ'1 [Γ'2 Hsubst]]. left. exists Γ'1, (X0 ~ᵃ A0;ᵃ Γ'2). simpl...
+      * right. unfold not. intros Hcontra. destruct Hcontra as [Γ'1 [Γ'2 Hsubst]].
+        dependent destruction Hsubst. eauto.
+    + apply IHΓ2 in H0. destruct H1.
+      * right. unfold not. intros Hcontra. destruct Hcontra as [Γ'1 [Γ'2 Hsubst]].
+        dependent destruction Hsubst. contradiction. 
+      * destruct H0. 
+        -- destruct H0 as [Γ'1 [Γ'2 Hsubst]]. left. exists Γ'1, (X0 ~ᵃ □ ;ᵃ Γ'2). simpl...
+           constructor... rewrite awl_to_aenv_app in H. simpl in H. unfold not. intros. subst. solve_notin_eq X.
+        -- right. unfold not. intros Hcontra. destruct Hcontra as [Γ'1 [Γ'2 Hsubst]].
+           dependent destruction Hsubst. eauto.
+    + destruct H1.
+      * assert (⊢ᵃʷₜ (Γ2 ⧺ X ~ᵃ ⬒ ;ᵃ X0 ~ᵃ ⬒ ;ᵃ Γ1)) by (eapply a_wf_twl_move_etvar_back; eauto).
+        apply IHΓ2 in H2. destruct H2.
+        -- destruct H2 as [Γ'1 [Γ'2 Hsubst]]. left. exists Γ'1, Γ'2. simpl...
+           constructor...  rewrite awl_to_aenv_app in H. simpl in H. unfold not. intros. subst. solve_notin_eq X.
+        -- right. unfold not. intros Hcontra. destruct Hcontra as [Γ'1 [Γ'2 Hsubst]].
+           dependent destruction Hsubst.
+           ++ rewrite awl_to_aenv_app in H. simpl in H. unfold not. intros. subst. solve_notin_eq X0.
+           ++ contradiction.
+           ++ apply worklist_split_etvar_det in x...
+              destruct x; subst.
+              eauto.
+              assert (X ∉ union (dom (awl_to_aenv Γ1)) (dom (awl_to_aenv Γ2))) by (eapply a_wf_twl_avar_notin_remaining; eauto)...
+      * apply IHΓ2 in H0. destruct H0.
+        -- left. destruct H0 as [Γ'1 [Γ'2 Hsubst]]. exists Γ'1, (X0 ~ᵃ ⬒ ;ᵃ Γ'2). simpl...
+           constructor... rewrite awl_to_aenv_app in H. simpl in H. unfold not. intros. subst. solve_notin_eq X.
+        -- right. unfold not. intros Hcontra. destruct Hcontra as [Γ'1 [Γ'2 Hsubst]].
+           dependent destruction Hsubst.
+           ++ rewrite awl_to_aenv_app in H. simpl in H. unfold not. intros. subst. solve_notin_eq X0. 
+           ++ eauto.
+           ++ contradiction.
+  - intros. dependent destruction H.
+    apply IHΓ2 in H1. destruct H1.
+    + destruct H1 as [Γ'1 [Γ'2 Hsubst]]. left. exists Γ'1, (w ⫤ᵃ Γ'2). simpl...
+    + right. unfold not. intros Hcontra. destruct Hcontra as [Γ'1 [Γ'2 Hsubst]].
+      dependent destruction Hsubst. 
+      assert ((∃ Γ'1 Γ'2 : aworklist, aworklist_subst (Γ2 ⧺ X ~ᵃ ⬒ ;ᵃ Γ1) X A Γ'1 Γ'2)) by eauto.
+      contradiction.
+Qed.
+
+Lemma a_wf_wl_binds_etvar_aworklist_subst_dec' : forall Γ1 Γ2 X A,
+  ⊢ᵃʷₛ (Γ2 ⧺ X ~ᵃ ⬒ ;ᵃ Γ1) -> 
+  (exists Γ'1 Γ'2, aworklist_subst (Γ2 ⧺ X ~ᵃ ⬒ ;ᵃ Γ1) X A Γ'1 Γ'2) \/ ~ (exists Γ'1 Γ'2, aworklist_subst (Γ2 ⧺ X ~ᵃ ⬒ ;ᵃ Γ1) X A Γ'1 Γ'2).
+Proof with eauto.
+  intros. generalize dependent Γ1. induction Γ2.
+  - left. exists Γ1, aworklist_empty. simpl. constructor.
+  - intros. assert (X0 `in` ftvar_in_typ A \/ (~ X0 `in` ftvar_in_typ A)) by fsetdec. 
+    dependent destruction H.
+    + eapply a_wf_twl_binds_etvar_aworklist_subst_dec'...
+    + apply IHΓ2 in H0. destruct H1.
+      * right. unfold not. intros Hcontra. destruct Hcontra as [Γ'1 [Γ'2 Hsubst]].
+        dependent destruction Hsubst. contradiction. 
+      * destruct H0. 
+        -- destruct H0 as [Γ'1 [Γ'2 Hsubst]]. left. exists Γ'1, (X0 ~ᵃ ■ ;ᵃ Γ'2). simpl...
+           constructor... rewrite awl_to_aenv_app in H. simpl in H. unfold not. intros. subst. solve_notin_eq X.
+        -- right. unfold not. intros Hcontra. destruct Hcontra as [Γ'1 [Γ'2 Hsubst]].
+           dependent destruction Hsubst. eauto.
+    + destruct H1.
+      * assert (⊢ᵃʷₛ (Γ2 ⧺ X ~ᵃ ⬒ ;ᵃ X0 ~ᵃ ⬒ ;ᵃ Γ1)) by (eapply a_wf_wl_move_etvar_back; eauto).
+        apply IHΓ2 in H2. destruct H2.
+        -- destruct H2 as [Γ'1 [Γ'2 Hsubst]]. left. exists Γ'1, Γ'2. simpl...
+           constructor...  rewrite awl_to_aenv_app in H. simpl in H. unfold not. intros. subst. solve_notin_eq X.
+        -- right. unfold not. intros Hcontra. destruct Hcontra as [Γ'1 [Γ'2 Hsubst]].
+           dependent destruction Hsubst.
+           ++ rewrite awl_to_aenv_app in H. simpl in H. unfold not. intros. subst. solve_notin_eq X0.
+           ++ contradiction.
+           ++ apply worklist_split_etvar_det in x...
+              destruct x; subst.
+              eauto.
+              assert (X ∉ union (dom (awl_to_aenv Γ1)) (dom (awl_to_aenv Γ2))) by (eapply a_wf_wl_avar_notin_remaining; eauto)...
+      * apply IHΓ2 in H0. destruct H0.
+        -- left. destruct H0 as [Γ'1 [Γ'2 Hsubst]]. exists Γ'1, (X0 ~ᵃ ⬒ ;ᵃ Γ'2). simpl...
+           constructor... rewrite awl_to_aenv_app in H. simpl in H. unfold not. intros. subst. solve_notin_eq X.
+        -- right. unfold not. intros Hcontra. destruct Hcontra as [Γ'1 [Γ'2 Hsubst]].
+           dependent destruction Hsubst.
+           ++ rewrite awl_to_aenv_app in H. simpl in H. unfold not. intros. subst. solve_notin_eq X0. 
+           ++ eauto.
+           ++ contradiction.
+  - intros. dependent destruction H.
+    eapply a_wf_twl_binds_etvar_aworklist_subst_dec'...
+    apply IHΓ2 in H1. destruct H1.
+    + destruct H1 as [Γ'1 [Γ'2 Hsubst]]. left. exists Γ'1, (work_sub A0 B ⫤ᵃ Γ'2). simpl...
+    + right. unfold not. intros Hcontra. destruct Hcontra as [Γ'1 [Γ'2 Hsubst]].
+      dependent destruction Hsubst. 
+      assert ((∃ Γ'1 Γ'2 : aworklist, aworklist_subst (Γ2 ⧺ X ~ᵃ ⬒ ;ᵃ Γ1) X A Γ'1 Γ'2)) by eauto.
+      contradiction.
+Qed.
+
+Lemma a_wf_wl_binds_etvar_aworklist_subst_dec : forall Γ X A,
+  ⊢ᵃʷₛ Γ -> X ~ ⬒ ∈ᵃ ⌊ Γ ⌋ᵃ ->
+  (exists Γ1 Γ2, aworklist_subst Γ X A Γ1 Γ2) \/ ~ (exists Γ1 Γ2, aworklist_subst Γ X A Γ1 Γ2).
+Proof with eauto. 
+  intros. apply awl_split_etvar in H0... destruct H0 as [Γ1 [Γ2 Hsplit]]...
+  subst. apply a_wf_wl_binds_etvar_aworklist_subst_dec'...
+Qed.
+
+Lemma a_wf_twl_aworklist_subst_no_etvar_false : forall Γ Γ1 Γ2 X A,
+  ⊢ᵃʷₜ Γ ->
+  (X ~ ⬒ ∈ᵃ ⌊ Γ ⌋ᵃ → False) ->
+  aworklist_subst Γ X A Γ1 Γ2 -> False.
+Proof with eauto.
+  intros. dependent induction H1.
+  - assert (binds X abind_etvar_empty (awl_to_aenv (X ~ᵃ ⬒ ;ᵃ Γ))).
+    { simpl. constructor; auto. } auto.
+  - apply IHaworklist_subst.
+    + dependent destruction H...
+    + intros. apply H0. simpl...
+  - apply IHaworklist_subst.
+    + dependent destruction H...
+    + intros. apply H0. simpl...
+  - apply IHaworklist_subst.
+    + dependent destruction H...
+    + intros. apply H0. simpl...  
+  - apply IHaworklist_subst.
+    + dependent destruction H...
+    + intros. apply H0. simpl...  
+  - apply IHaworklist_subst.
+    + dependent destruction H...
+    + intros. apply H0. simpl...
+  - apply IHaworklist_subst.
+    + eapply a_wf_twl_move_etvar_back; eauto. 
+    + intros. apply H0. simpl...
+      rewrite awl_to_aenv_app. simpl...
+Qed.
+
+Lemma a_wf_wl_aworklist_subst_no_etvar_false : forall Γ Γ1 Γ2 X A,
+  ⊢ᵃʷₛ Γ ->
+  (X ~ ⬒ ∈ᵃ ⌊ Γ ⌋ᵃ → False) ->
+  aworklist_subst Γ X A Γ1 Γ2 -> False.
+Proof with eauto.
+  intros. dependent induction H1.
+  - assert (binds X abind_etvar_empty (awl_to_aenv (X ~ᵃ ⬒ ;ᵃ Γ))).
+    { simpl. constructor; auto. } auto.
+  - dependent destruction H.
+    eapply a_wf_twl_aworklist_subst_no_etvar_false...
+  - dependent destruction H.
+    eapply a_wf_twl_aworklist_subst_no_etvar_false...
+  - dependent destruction H.
+    eapply a_wf_twl_aworklist_subst_no_etvar_false...
+    apply IHaworklist_subst...
+    intros. apply H1. simpl... 
+  - dependent destruction H.
+    eapply a_wf_twl_aworklist_subst_no_etvar_false...
+    apply IHaworklist_subst...
+  - dependent destruction H.
+    eapply a_wf_twl_aworklist_subst_no_etvar_false...
+    apply IHaworklist_subst...
+    intros. apply H1. simpl...
+  - dependent destruction H.
+    eapply a_wf_twl_aworklist_subst_no_etvar_false...
+    apply IHaworklist_subst.
+    + eapply a_wf_wl_move_etvar_back; eauto. 
+    + intros. apply H1. simpl...
+      rewrite awl_to_aenv_app. simpl... 
+Qed.
+
+Lemma typ_eq_bool : forall (A1 A2:typ),
+  sumbool (A1 = A2) (A1 <> A2).
+Proof.
+  intro A1. induction A1; intro A2; induction A2; eauto;
+    try solve [right; unfold not; intros Hcontra; inversion Hcontra].
+  - destruct (n == n0); auto.
+    right. unfold not. intros. inversion H. contradiction. 
+  - destruct (X == X0); subst. auto.
+    right. unfold not. intros. inversion H. contradiction. 
+  - pose proof (IHA1_1 A2_1).
+    pose proof (IHA1_2 A2_2).
+    destruct H; destruct H0; subst; eauto;  
+      right; unfold not; intros Hcontra; inversion Hcontra; contradiction. 
+  - pose proof (IHA1 A2). destruct H.
+    + subst. auto.
+    + right. unfold not. intros Hcontra. dependent destruction Hcontra. contradiction.
+  - pose proof (IHA1_1 A2_1).
+    pose proof (IHA1_2 A2_2).
+    destruct H; destruct H0; subst; eauto;  
+      right; unfold not; intros Hcontra; inversion Hcontra; contradiction.
+  - pose proof (IHA1_1 A2_1).
+    pose proof (IHA1_2 A2_2).
+    destruct H; destruct H0; subst; eauto;  
+      right; unfold not; intros Hcontra; inversion Hcontra; contradiction.  
+Qed.
+
+Lemma a_bind_eq_bool : forall (b1 b2:abind),
+  sumbool (b1 = b2) (b1 <> b2).
+Proof.
+  intros. destruct b1; destruct b2; eauto;
+    try solve [right; unfold not; intros Hcontra; inversion Hcontra].
+  - pose proof (typ_eq_bool A A0).
+    destruct H; subst; eauto;
+      right; unfold not; intros Hcontra; inversion Hcontra; contradiction.
+Qed.
+
+
+Lemma a_wf_wl_aworklist_subst_dec : forall Γ X A,
+  ⊢ᵃʷₛ Γ -> 
+  (exists Γ1 Γ2, aworklist_subst Γ X A Γ1 Γ2) \/ ~ (exists Γ1 Γ2, aworklist_subst Γ X A Γ1 Γ2).
+Proof.
+  intros.
+  assert (sumbool (binds X abind_etvar_empty (awl_to_aenv Γ)) (~ binds X abind_etvar_empty (awl_to_aenv Γ))). {
+    apply binds_dec. apply a_bind_eq_bool.
+  }
+  destruct H0.
+  - apply a_wf_wl_binds_etvar_aworklist_subst_dec; eauto.
+  - right. unfold not. intros. destruct H0 as [Γ1 [Γ2 Hsubst]]. 
+    eapply a_wf_wl_aworklist_subst_no_etvar_false; eauto.
+Qed.
+
+(*
+
+Lemma exp_size_wl_aworklist_subst' : forall Γ2 Γ X A Γ1 Γ1' Γ2',
+  ⊢ᵃʷ (Γ2 ⧺ X ~ᵃ ⬒ ;ᵃ Γ1) -> 
+  aworklist_subst (Γ2 ⧺ X ~ᵃ ⬒ ;ᵃ Γ1) X A Γ1' Γ2' -> a_mono_typ (awl_to_aenv Γ) A ->
+  (* ⌊ Γ2 ⧺ X ~ᵃ ⬒ ;ᵃ Γ1 ⌋ᵃ *)
+  exp_size_wl (subst_tvar_in_aworklist A X Γ2' ⧺ Γ1') = exp_size_wl (Γ2 ⧺ X ~ᵃ ⬒ ;ᵃ Γ1).
+Proof.
+  intros Γ2. induction Γ2; intros;
+    dependent destruction H0; dependent destruction H; simpl in *; eauto;
+    try solve [exfalso; eauto].
+  - eapply worklist_split_etvar_det in x. destruct x. subst.
+    eapply IHΓ2 in H1; eauto. admit. admit. admit.
+Admitted.
+
+Lemma exp_size_wl_aworklist_subst : forall Γ X A Γ1 Γ2,
+  ⊢ᵃʷ Γ -> 
+  aworklist_subst Γ X A Γ1 Γ2 -> a_mono_typ (awl_to_aenv Γ) A ->
+  exp_size_wl (subst_tvar_in_aworklist A X Γ2 ⧺ Γ1) = exp_size_wl Γ.
+Admitted.
+
+Lemma lookup_tvar_bind_etvar : forall Γ2 Γ1 X X0,
+  X ≠ X0 ->
+  lookup_tvar_bind (⌊ Γ2 ⧺ Γ1 ⌋ᵃ) X = lookup_tvar_bind (⌊ Γ2 ⧺ X0 ~ᵃ ⬒ ;ᵃ Γ1 ⌋ᵃ) X.
+Proof.
+  intros Γ2. induction Γ2; simpl; intros; eauto.
+  - destruct (X == X0); subst; auto; try contradiction.
+  - destruct (X == x); subst; auto.
+  - destruct (X0 == X); subst; auto.
+Qed.
+
+
+Lemma split_depth_rec_etvar : forall A Γ1 Γ2 X n,
+  ⊢ᵃʷ (Γ2 ⧺ Γ1) ->
+  X ∉ ftvar_in_typ A ->
+  X ∉ dom (⌊ Γ2 ⧺ Γ1 ⌋ᵃ) ->
+  split_depth_rec (⌊ Γ2 ⧺ Γ1 ⌋ᵃ) A n = split_depth_rec (⌊ Γ2 ⧺ X ~ᵃ ⬒ ;ᵃ Γ1 ⌋ᵃ) A n.
+Proof.
+  intros A. induction A; intros Γ1 Γ2 X0 n0 Hwf Hnotin1 Hnotin2; eauto.
+  - destruct (X == X0); subst.
+    eapply notin_singleton_1 in Hnotin1. contradiction.
+    simpl. erewrite lookup_tvar_bind_etvar; eauto.
+  - simpl in *.
+    specialize (IHA1 Γ1 Γ2 X0 (S n0) Hwf).
+    specialize (IHA2 Γ1 Γ2 X0 (S n0) Hwf). auto.
+  - simpl in *.
+    specialize (IHA Γ1 Γ2 X0 n0 Hwf). auto.
+  - simpl in *.
+    specialize (IHA1 Γ1 Γ2 X0 n0 Hwf).
+    specialize (IHA2 Γ1 Γ2 X0 n0 Hwf). auto.
+  - simpl in *.
+    specialize (IHA1 Γ1 Γ2 X0 n0 Hwf).
+    specialize (IHA2 Γ1 Γ2 X0 n0 Hwf). auto.
+Qed.
+
+Lemma split_depth_etvar : forall A Γ1 Γ2 X,
+  ⊢ᵃʷ (Γ2 ⧺ Γ1) ->
+  X ∉ ftvar_in_typ A ->
+  X ∉ dom (⌊ Γ2 ⧺ Γ1 ⌋ᵃ) ->
+  split_depth (⌊ Γ2 ⧺ Γ1 ⌋ᵃ) A = split_depth (⌊ Γ2 ⧺ X ~ᵃ ⬒ ;ᵃ Γ1 ⌋ᵃ) A.
+Proof.
+  unfold split_depth. simpl. intros. erewrite split_depth_rec_etvar; eauto.
+Qed.
+
+Lemma split_depth_work_etvar : forall Γ1 Γ2 X w,
+  ⊢ᵃʷ (Γ2 ⧺ Γ1) ->
+  X ∉ ftvar_in_work w ->
+  X ∉ dom (⌊ Γ2 ⧺ Γ1 ⌋ᵃ) ->
+  split_depth_work (⌊ Γ2 ⧺ Γ1 ⌋ᵃ) w = split_depth_work (⌊ Γ2 ⧺ X ~ᵃ ⬒ ;ᵃ Γ1 ⌋ᵃ) w.
+Proof.
+  intros Γ1 Γ2 X w. dependent destruction w; simpl; auto.
+  intros Hwf Hnotin1 Hnotin2.
+  erewrite <- split_depth_etvar; eauto.
+  erewrite <- split_depth_etvar; eauto.
+Qed.
+
+Lemma split_depth_wl_etvar : forall Γ1 Γ2 X,
+  ⊢ᵃʷ (Γ2 ⧺ Γ1) ->
+  X ∉ dom (⌊ Γ2 ⧺ Γ1 ⌋ᵃ) ->
+  split_depth_wl (Γ2 ⧺ Γ1) = split_depth_wl (Γ2 ⧺ X ~ᵃ ⬒ ;ᵃ Γ1).
+Proof.
+  intros Γ1 Γ2.
+  generalize dependent Γ1.
+  induction Γ2; simpl; intros; try solve [dependent destruction H; auto].
+  dependent destruction H.
+  assert (X ∉ ftvar_in_work w) by admit.
+  erewrite <- split_depth_work_etvar; eauto. 
+Admitted.
+
+
+Lemma split_depth_wl_aworklist_subst : forall Γ2 X A Γ1 Γ1' Γ2',
+  ⊢ᵃʷ (Γ2 ⧺ X ~ᵃ ⬒ ;ᵃ Γ1) -> 
+  aworklist_subst (Γ2 ⧺ X ~ᵃ ⬒ ;ᵃ Γ1) X A Γ1' Γ2' -> a_mono_typ (⌊ Γ2 ⧺ X ~ᵃ ⬒ ;ᵃ Γ1 ⌋ᵃ) A ->
+  X ∉ ftvar_in_typ A ->
+  split_depth_wl (subst_tvar_in_aworklist A X Γ2' ⧺ Γ1') = split_depth_wl (Γ2 ⧺ X ~ᵃ ⬒ ;ᵃ Γ1).
+Proof.
+  intros Γ2. induction Γ2; intros * Hwf Hsubst Hmono Hnotin; simpl in *.
+  - eapply a_mono_typ_strengthen_cons in Hmono; eauto.
+    dependent destruction Hsubst; simpl; eauto; try contradiction.
+  - erewrite IHΓ2; eauto. admit. admit. admit.
+  - dependent destruction Hsubst; simpl; destruct_a_wf_wl; eauto.
+    + eapply a_mono_typ_strengthen_cons in Hmono; eauto.
+    + eapply a_mono_typ_strengthen_cons in Hmono; eauto.
+    + eapply a_mono_typ_strengthen_cons in Hmono; eauto.
+    + assert (⊢ᵃʷ (Γ2 ⧺ X0 ~ᵃ ⬒ ;ᵃ X ~ᵃ ⬒ ;ᵃ Γ1)) by admit.
+      eapply worklist_split_etvar_det in x. destruct x. subst.
+      eapply IHΓ2 with (A := A) in H2; eauto. admit. admit. admit.
+  - dependent destruction Hsubst; simpl; destruct_a_wf_wl; eauto.
+    admit.
+Admitted.
+
+(* Lemma split_depth_rec_aworklist_subst : forall Γ2 Γ X A B Γ1 Γ1' Γ2',
+  ⊢ᵃʷ (Γ2 ⧺ X ~ᵃ ⬒ ;ᵃ Γ1) -> 
+  X ∉ ftvar_in_typ B ->
+  aworklist_subst (Γ2 ⧺ X ~ᵃ ⬒ ;ᵃ Γ1) X A Γ1' Γ2' -> a_mono_typ (awl_to_aenv Γ) A ->
+  split_depth (⌊ subst_tvar_in_aworklist A X Γ2' ⧺ Γ1' ⌋ᵃ) B = split_depth (⌊ Γ2 ⧺ X ~ᵃ ⬒ ;ᵃ Γ1 ⌋ᵃ) B.
+Proof.
+  intros Γ2. induction Γ2; intros Γ X0 A B Γ1 Γ1' Γ2' Hwf Hnotin Hsubst Hmono;
+    dependent destruction Hsubst; dependent destruction Hwf; simpl in *; eauto;
+    try solve [exfalso; eauto].
+  admit.
+    dependent destruction H0; dependent destruction H; simpl in *; eauto;
+    try solve [exfalso; eauto].
+
+Lemma split_depth_work_aworklist_subst : forall Γ2 Γ X A Γ1 Γ1' Γ2',
+  ⊢ᵃʷ (Γ2 ⧺ X ~ᵃ ⬒ ;ᵃ Γ1) -> 
+  aworklist_subst (Γ2 ⧺ X ~ᵃ ⬒ ;ᵃ Γ1) X A Γ1' Γ2' -> a_mono_typ (awl_to_aenv Γ) A ->
+  split_depth_work (subst_tvar_in_aworklist A X Γ2' ⧺ Γ1') = split_depth_wl (Γ2 ⧺ X ~ᵃ ⬒ ;ᵃ Γ1). *)
+
+(* Lemma split_depth_rec_non_mono_lt : forall A Γ1 Γ2 n m,
+  ⊢ᵃʷ Γ -> a_mono_typ (awl_to_aenv Γ) A ->
+  split_depth_rec (⌊ Γ ⌋ᵃ) A n < split_depth_rec (⌊ Γ ⌋ᵃ) A m. *)
+
+Lemma split_depth_rec_non_mono_non_zero : forall A Γ n,
+  ⊢ᵃʷ Γ -> a_wf_typ (awl_to_aenv Γ) A ->
+  (a_mono_typ (awl_to_aenv Γ) A -> False) -> n > 0 ->
+  split_depth_rec (⌊ Γ ⌋ᵃ) A n > 0.
+Proof.
+  intros A Γ n Hwf Hwf1 Hmono.
+  generalize dependent n.
+  dependent induction Hwf1; simpl; intros n Hgt; eauto; try solve [exfalso; eauto]; try lia.
+  - erewrite lookup_tvar_bind_binds in H; eauto.
+    destruct (lookup_tvar_bind (⌊ Γ ⌋ᵃ) X); inversion H; eauto.
+  - destruct (a_mono_typ_dec Γ A1); destruct (a_mono_typ_dec Γ A2); eauto.
+    + exfalso. eauto.
+    + eapply IHHwf1_2 with (n := S n) in H0; eauto. lia.
+    + eapply IHHwf1_1 with (n := S n) in H; eauto. lia.
+    + eapply IHHwf1_1 with (n := S n) in H; eauto. lia.
+Qed.
+
+Lemma split_depth_rec_non_zero_non_mono : forall A Γ n,
+  ⊢ᵃʷ Γ -> split_depth_rec (⌊ Γ ⌋ᵃ) A n > 0 ->
+  a_mono_typ (awl_to_aenv Γ) A -> False.
+Proof.
+  intros A. induction A; simpl; intros Γ n0 Hwf Hgt Hmono;
+    try solve [inversion Hgt; inversion Hmono].
+  - destruct (lookup_tvar_bind (⌊ Γ ⌋ᵃ) X) eqn:Heq.
+    destruct a; try solve [inversion Hgt; exfalso; eauto]; eauto.
+    rewrite <- lookup_tvar_bind_binds in Heq; eauto.
+    dependent destruction Hmono; try unify_binds. inversion Hgt.
+  - specialize (IHA1 Γ (S n0) Hwf). specialize (IHA2 Γ (S n0) Hwf).
+    dependent destruction Hmono.
+    destruct (split_depth_rec (⌊ Γ ⌋ᵃ) A1 (S n0)) eqn:Heq1;
+    destruct (split_depth_rec (⌊ Γ ⌋ᵃ) A2 (S n0)) eqn:Heq2; eauto.
+    eapply IHA1; eauto. lia. eapply IHA2; eauto. lia.
+Qed.
+
+Lemma split_depth_rec_non_mono_lt_ : forall A Γ n m,
+  ⊢ᵃʷ Γ -> split_depth_rec (⌊ Γ ⌋ᵃ) A n > 0 -> n < m ->
+  split_depth_rec (⌊ Γ ⌋ᵃ) A n < split_depth_rec (⌊ Γ ⌋ᵃ) A m.
+Proof.
+  intros A. induction A; simpl; intros Γ n0 m Hwf Hgt Hlt; eauto.
+  - destruct (lookup_tvar_bind (⌊ Γ ⌋ᵃ) X) eqn:Heq.
+    destruct a; try solve [exfalso; eauto]; eauto. inversion Hgt.
+  - destruct (split_depth_rec (⌊ Γ ⌋ᵃ) A1 (S n0)) eqn:Heq1.
+    destruct (split_depth_rec (⌊ Γ ⌋ᵃ) A2 (S n0)) eqn:Heq2.
+    + inversion Hgt.
+    + specialize (IHA2 Γ (S n0) (S m) Hwf). lia.
+    + specialize (IHA1 Γ (S n0) (S m) Hwf).
+      specialize (IHA2 Γ (S n0) (S m) Hwf). lia.
+  - specialize (IHA Γ n0 m Hwf). lia.
+  - specialize (IHA1 Γ n0 m Hwf).
+    specialize (IHA2 Γ n0 m Hwf). lia.
+  - specialize (IHA1 Γ n0 m Hwf).
+    specialize (IHA2 Γ n0 m Hwf). lia.
+Qed.
+
+Lemma split_depth_rec_non_mono_lt : forall A Γ n m,
+  ⊢ᵃʷ Γ -> ⌊ Γ ⌋ᵃ ᵗ⊢ᵃ A -> (a_mono_typ (awl_to_aenv Γ) A -> False) ->
+  n > 0 -> n < m ->
+  split_depth_rec (⌊ Γ ⌋ᵃ) A n < split_depth_rec (⌊ Γ ⌋ᵃ) A m.
+Proof.
+  intros.
+  eapply split_depth_rec_non_mono_lt_; eauto.
+  eapply split_depth_rec_non_mono_non_zero; eauto.
+Qed.
+
+Lemma split_depth_rec_aworklist_subst_ : forall B Γ2 X A Γ1 Γ1' Γ2' n,
+  ⊢ᵃʷ (Γ2 ⧺ X ~ᵃ ⬒ ;ᵃ Γ1) -> 
+  aworklist_subst (Γ2 ⧺ X ~ᵃ ⬒ ;ᵃ Γ1) X A Γ1' Γ2' -> a_mono_typ (⌊ Γ2 ⧺ X ~ᵃ ⬒ ;ᵃ Γ1 ⌋ᵃ) A ->
+  X ∉ ftvar_in_typ B ->
+  split_depth_rec (⌊ subst_tvar_in_aworklist A X Γ2' ⧺ Γ1' ⌋ᵃ) B n = split_depth_rec (⌊ Γ2 ⧺ X ~ᵃ ⬒ ;ᵃ Γ1 ⌋ᵃ) B n.
+Proof.
+  intros B. induction B; intros * Hwf Hsubst Hmono Hnotin; unfold split_depth; simpl in *; eauto.
+  - admit.
+Admitted.
+
+Lemma split_depth_rec_subst : forall B Γ2 X A Γ1 n,
+  ⊢ᵃʷ (Γ2 ⧺ X ~ᵃ ⬒ ;ᵃ Γ1) -> a_mono_typ (⌊ Γ2 ⧺ X ~ᵃ ⬒ ;ᵃ Γ1 ⌋ᵃ) A ->
+  split_depth_rec (⌊ Γ2 ⧺ X ~ᵃ ⬒ ;ᵃ Γ1 ⌋ᵃ) B n = split_depth_rec (⌊ Γ2 ⧺ X ~ᵃ ⬒ ;ᵃ Γ1 ⌋ᵃ) ({A /ᵗ X} B) n.
+Proof.
+  intros B. induction B; intros * Hwf Hmono; unfold split_depth; simpl in *; eauto.
+  - admit.
+Admitted.
+
+Lemma split_depth_rec_aworklist_subst : forall B Γ2 X A Γ1 Γ1' Γ2' n,
+  ⊢ᵃʷ (Γ2 ⧺ X ~ᵃ ⬒ ;ᵃ Γ1) -> 
+  aworklist_subst (Γ2 ⧺ X ~ᵃ ⬒ ;ᵃ Γ1) X A Γ1' Γ2' -> a_mono_typ (⌊ Γ2 ⧺ X ~ᵃ ⬒ ;ᵃ Γ1 ⌋ᵃ) A ->
+  X ∉ ftvar_in_typ A ->
+  split_depth_rec (⌊ subst_tvar_in_aworklist A X Γ2' ⧺ Γ1' ⌋ᵃ) ({A /ᵗ X} B) n = split_depth_rec (⌊ Γ2 ⧺ X ~ᵃ ⬒ ;ᵃ Γ1 ⌋ᵃ) B n.
+Proof.
+  intros.
+  erewrite split_depth_rec_subst; eauto. erewrite split_depth_rec_aworklist_subst_; eauto.
+  eapply subst_tvar_in_typ_fresh_same; eauto.
+Qed.  
+
+*)
+
+Lemma exp_size_weaken_work : forall Γ e w,
+  ⊢ᵃʷₛ Γ -> exp_size (w ⫤ᵃ Γ) e = exp_size Γ e
+with body_size_weaken_work : forall Γ b w,
+  ⊢ᵃʷₛ Γ -> body_size (w ⫤ᵃ Γ) b = body_size Γ b.
+Proof.
+  intros Γ e w Hwf. dependent destruction e; simpl; auto.
+  intros Γ e w Hwf. dependent destruction e; simpl; auto.
+Qed.
+
+#[local] Hint Extern 1 ((exists _, _) -> False) => try solve_false : core.
+
+Lemma decidablity_lemma : forall ne nj nt ntj na naj nm nw Γ,
+  ⊢ᵃʷₛ Γ ->
   exp_size_wl Γ < ne ->
   judge_size_wl Γ < nj ->
   inftapp_depth_wl Γ < nt ->
   inftapp_judge_size_wl Γ < ntj ->
   infabs_depth_wl Γ < na ->
   infabs_judge_size_wl Γ < naj ->
-  measp_wl Γ m -> m < nm ->
+  split_depth_wl Γ < nm ->
   weight_wl Γ < nw ->
   Γ ⟶ᵃʷ⁎⋅ \/ ¬ Γ ⟶ᵃʷ⁎⋅.
 Proof.
@@ -881,976 +1118,1034 @@ Proof.
   intros naj; induction naj;
   intros nm; induction nm;
   intros nw; induction nw; try lia.
-  intros Γ m Hwf He Hj Ht Htj Ha Haj Hm Hlt Hw.
+  intros Γ Hwf He Hj Ht Htj Ha Haj Hm Hw.
   dependent destruction Hwf; auto.
-  - dependent destruction Hm. simpl in *.
-    assert (Jg: a_wl_red aW \/ ~ a_wl_red aW).
-    { eapply IHnw; eauto. lia. }
-    destruct Jg as [Jg | Jg]; auto.
-    right. intro Hcontra.
-    dependent destruction Hcontra.
-    apply Jg; auto.
-  - dependent destruction Hm. simpl in *.
-    assert (Jg: a_wl_red aW \/ ~ a_wl_red aW).
-    { eapply IHnw; eauto. lia. }
-    destruct Jg as [Jg | Jg]; auto.
-    right. intro Hcontra.
-    dependent destruction Hcontra.
-    apply Jg; auto.
-  - dependent destruction Hm. simpl in *.
-    assert (Jg: a_wl_red aW \/ ~ a_wl_red aW).
-    { eapply IHnw; eauto. lia. }
-    destruct Jg as [Jg | Jg]; auto.
-    right. intro Hcontra.
-    dependent destruction Hcontra.
-    apply Jg; auto.
-  - dependent destruction Hm. simpl in *.
-    assert (Jg: a_wl_red aW \/ ~ a_wl_red aW).
-    { eapply IHnw; eauto; lia. }
-    destruct Jg as [Jg | Jg]; auto.
-    right. intro Hcontra.
-    dependent destruction Hcontra.
-    apply Jg; auto.
-  - dependent destruction H.
-    + dependent destruction Hm.
-      dependent destruction H; simpl in *.
-      * assert (Jg: a_wl_red (aworklist_conswork aW (work_apply c typ_unit)) \/
-                  ~ a_wl_red (aworklist_conswork aW (work_apply c typ_unit))).
-        { eapply IHne; eauto; simpl; try lia. }
-        destruct Jg as [Jg | Jg]; auto.
-        right. intro Hcontra.
-        dependent destruction Hcontra.
-        apply Jg; auto.
-      * assert (Jg: a_wl_red (aworklist_conswork aW (work_apply c A)) \/
-                  ~ a_wl_red (aworklist_conswork aW (work_apply c A))).
-        { eapply IHne; eauto; simpl; try lia. admit. (* safe: wf *) }
-        destruct Jg as [Jg | Jg]; eauto.
-        right. intro Hcontra.
-        dependent destruction Hcontra.
-        apply binds_unique with (b:= (abind_var_typ A0)) in H; auto. dependent destruction H.
-        subst. apply Jg; auto.
-        admit.
-      * right. intro Hcontra.
-        dependent destruction Hcontra.
-        admit. (* TODO *)
-      * assert (Jg:   (work_infer e1 (cont_infabs (cont_infapp e2 c)) ⫤ aW) ⟶ᵃʷ⁎⋅ \/
-                    ¬ (work_infer e1 (cont_infabs (cont_infapp e2 c)) ⫤ aW) ⟶ᵃʷ⁎⋅).
-        { eapply IHne; eauto; simpl; try lia. }
-        destruct Jg as [Jg | Jg]; eauto.
-        right. intro Hcontra.
-        dependent destruction Hcontra.
-        apply Jg; auto.
-      * destruct body5. admit.
-        (* TODO *)
+  - rename H into Hwf. dependent destruction Hwf; auto.
+    + simpl in *.
+      assert (Jg: Γ ⟶ᵃʷ⁎⋅ \/ ¬ Γ ⟶ᵃʷ⁎⋅).
+      { eapply IHnw; eauto. lia. }
+      destruct Jg as [Jg | Jg]; auto.
+      right. intro Hcontra.
+      dependent destruction Hcontra.
+      apply Jg; auto.
+    + simpl in *.
+      assert (Jg: Γ ⟶ᵃʷ⁎⋅ \/ ¬ Γ ⟶ᵃʷ⁎⋅).
+      { eapply IHnw; eauto. lia. }
+      destruct Jg as [Jg | Jg]; auto.
+      right. intro Hcontra.
+      dependent destruction Hcontra.
+      apply Jg; auto.
+    + simpl in *.
+      assert (Jg: Γ ⟶ᵃʷ⁎⋅ \/ ¬ Γ ⟶ᵃʷ⁎⋅).
+      { eapply IHnw; eauto. lia. }
+      destruct Jg as [Jg | Jg]; auto.
+      right. intro Hcontra.
+      dependent destruction Hcontra.
+      apply Jg; auto.
+    + dependent destruction H.
+      * dependent destruction H; simpl in *.
+        -- assert (Jg: (work_applys cs typ_unit ⫤ᵃ Γ) ⟶ᵃʷ⁎⋅ \/
+                     ~ (work_applys cs typ_unit ⫤ᵃ Γ) ⟶ᵃʷ⁎⋅).
+           { eapply IHne; eauto; simpl; try lia. }
+           destruct Jg as [Jg | Jg]; auto.
+           right. intro Hcontra.
+           dependent destruction Hcontra.
+           apply Jg; auto.
+        -- assert (Jg: (work_applys cs A ⫤ᵃ Γ) ⟶ᵃʷ⁎⋅ \/
+                     ~ (work_applys cs A ⫤ᵃ Γ) ⟶ᵃʷ⁎⋅).
+           { eapply IHne; eauto; simpl; try lia.
+             eapply a_wf_wl_a_wf_bind_typ in H; eauto. }
+           destruct Jg as [Jg | Jg]; eauto.
+           right. intro Hcontra.
+           dependent destruction Hcontra.
+           apply binds_unique with (b:= (abind_var_typ A0)) in H; auto. dependent destruction H.
+           subst. apply Jg; auto.
+        -- pick fresh x. inst_cofinites_with x.
+           pick fresh X1. pick fresh X2.
+           assert (Jg: (work_check (e ᵉ^ₑ exp_var_f x) ` X2 ⫤ᵃ x ~ᵃ ` X1 ;ᵃ work_applys cs (typ_arrow ` X1 ` X2) ⫤ᵃ X2 ~ᵃ ⬒ ;ᵃ X1 ~ᵃ ⬒ ;ᵃ Γ) ⟶ᵃʷ⁎⋅ \/
+                     ~ (work_check (e ᵉ^ₑ exp_var_f x) ` X2 ⫤ᵃ x ~ᵃ ` X1 ;ᵃ work_applys cs (typ_arrow ` X1 ` X2) ⫤ᵃ X2 ~ᵃ ⬒ ;ᵃ X1 ~ᵃ ⬒ ;ᵃ Γ) ⟶ᵃʷ⁎⋅).
+           { eapply IHne; eauto; simpl; try lia.
+             constructor; auto. constructor; simpl; auto. constructor; simpl; auto.
+             eapply a_wf_exp_weaken_etvar_twice with (T := T); eauto.
+             constructor; simpl; auto. constructor; simpl; auto.
+             constructor; auto. apply a_wf_conts_weaken_cons. apply a_wf_conts_weaken_cons. auto.
+             admit. }
+           admit.
+        -- assert (Jg: (work_infer e1 (conts_infabs (contd_infapp (exp_split_size (⌊ Γ ⌋ᵃ) e1) e2 cs)) ⫤ᵃ Γ) ⟶ᵃʷ⁎⋅ \/
+                     ¬ (work_infer e1 (conts_infabs (contd_infapp (exp_split_size (⌊ Γ ⌋ᵃ) e1) e2 cs)) ⫤ᵃ Γ) ⟶ᵃʷ⁎⋅).
+           { eapply IHne; eauto; simpl; try lia. constructor; auto. }
+           destruct Jg as [Jg | Jg]; eauto.
+           right. intro Hcontra.
+           dependent destruction Hcontra.
+           apply Jg; auto.
+        -- destruct body5. pick fresh X.
+           assert (Jg: (work_check (e ᵉ^ₜ ` X) (A ᵗ^ₜ X) ⫤ᵃ X ~ᵃ □ ;ᵃ work_applys cs (typ_all A) ⫤ᵃ Γ) ⟶ᵃʷ⁎⋅ \/
+                     ~ (work_check (e ᵉ^ₜ ` X) (A ᵗ^ₜ X) ⫤ᵃ X ~ᵃ □ ;ᵃ work_applys cs (typ_all A) ⫤ᵃ Γ) ⟶ᵃʷ⁎⋅).
+           { eapply IHne; eauto; simpl; try lia. admit. admit. }
+           admit.
+        -- assert (Jg: (work_infer e (conts_inftapp A cs) ⫤ᵃ Γ) ⟶ᵃʷ⁎⋅ \/
+                     ¬ (work_infer e (conts_inftapp A cs) ⫤ᵃ Γ) ⟶ᵃʷ⁎⋅).
+           { eapply IHne; eauto; simpl; try lia. }
+           destruct Jg as [Jg | Jg]; eauto.
+           right. intro Hcontra.
+           dependent destruction Hcontra.
+           apply Jg; auto.
+        -- assert (Jg: (work_check e A ⫤ᵃ work_applys cs A ⫤ᵃ Γ) ⟶ᵃʷ⁎⋅ \/
+                     ¬ (work_check e A ⫤ᵃ work_applys cs A ⫤ᵃ Γ) ⟶ᵃʷ⁎⋅).
+           { assert (exp_size (work_applys cs A ⫤ᵃ Γ) e = exp_size Γ e) by (eapply exp_size_weaken_work; eauto).
+             eapply IHne; eauto; simpl; try lia. constructor; auto. }
+           destruct Jg as [Jg | Jg]; eauto.
+           right. intro Hcontra.
+           dependent destruction Hcontra.
+           apply Jg; auto.
       * simpl in *.
-        assert (Jg:   (work_infer e (cont_inftapp A c) ⫤ aW) ⟶ᵃʷ⁎⋅ \/
-                    ¬ (work_infer e (cont_inftapp A c) ⫤ aW) ⟶ᵃʷ⁎⋅).
-        { eapply IHne; eauto; simpl; try lia. }
+        assert (He': exp_size Γ e > 0) by apply exp_size_gt_0.
+        assert (Jg: (work_infer e (conts_sub A) ⫤ᵃ Γ) ⟶ᵃʷ⁎⋅ \/
+                  ¬ (work_infer e (conts_sub A) ⫤ᵃ Γ) ⟶ᵃʷ⁎⋅).
+        { eapply IHnj; eauto; simpl; try lia. }
+        assert (Jg1: forall A1 A2, A = typ_union A1 A2 ->
+                       (work_check e A1 ⫤ᵃ Γ) ⟶ᵃʷ⁎⋅ \/ ¬ (work_check e A1 ⫤ᵃ Γ) ⟶ᵃʷ⁎⋅).
+        { intros A1 A2 Heq. subst. dependent destruction H0. simpl in *.
+          eapply IHne; eauto; simpl; try lia. }
+        assert (Jg2: forall A1 A2, A = typ_union A1 A2 ->
+                       (work_check e A2 ⫤ᵃ Γ) ⟶ᵃʷ⁎⋅ \/ ¬ (work_check e A2 ⫤ᵃ Γ) ⟶ᵃʷ⁎⋅).
+        { intros A1 A2 Heq. subst. dependent destruction H0. simpl in *.
+          eapply IHne; eauto; simpl; try lia. }
+        assert (Jg': forall A1 A2, A = typ_intersection A1 A2 ->
+                       (work_check e A2 ⫤ᵃ work_check e A1 ⫤ᵃ Γ) ⟶ᵃʷ⁎⋅ \/
+                     ¬ (work_check e A2 ⫤ᵃ work_check e A1 ⫤ᵃ Γ) ⟶ᵃʷ⁎⋅ ).
+        { intros A1 A2 Heq. subst. dependent destruction H0. simpl in *.
+          assert (exp_size (work_check e A1 ⫤ᵃ Γ) e = exp_size Γ e) by (eapply exp_size_weaken_work; eauto).
+          eapply IHne; eauto; simpl; try lia. constructor; auto. }
         destruct Jg as [Jg | Jg]; eauto.
-        right. intro Hcontra.
-        dependent destruction Hcontra.
-        apply Jg; auto.
-      * simpl in *.
-        assert (Jg:   (work_check e A ⫤ work_apply c A ⫤ aW) ⟶ᵃʷ⁎⋅ \/
-                    ¬ (work_check e A ⫤ work_apply c A ⫤ aW) ⟶ᵃʷ⁎⋅).
-        { eapply IHne; eauto; simpl; try lia. }
-        destruct Jg as [Jg | Jg]; eauto.
-        right. intro Hcontra.
-        dependent destruction Hcontra.
-        apply Jg; auto.
-    + dependent destruction Hm. simpl in *.
-      assert (He': exp_size e >= 1) by apply exp_size_gt_0.
-      assert (Jg:   (work_infer e (cont_sub A) ⫤ aW) ⟶ᵃʷ⁎⋅ \/
-                  ¬ (work_infer e (cont_sub A) ⫤ aW) ⟶ᵃʷ⁎⋅).
-      { eapply IHnj; eauto; simpl; try lia. }
-      assert (Jg1: forall A1 A2, A = typ_union A1 A2 ->
-                (work_check e A1 ⫤ aW) ⟶ᵃʷ⁎⋅ \/ ¬ (work_check e A1 ⫤ aW) ⟶ᵃʷ⁎⋅).
-      { intros A1 A2 Heq. subst. dependent destruction H0. simpl in *.
-        eapply IHne; eauto; simpl; try lia. }
-      assert (Jg2: forall A1 A2, A = typ_union A1 A2 ->
-                (work_check e A2 ⫤ aW) ⟶ᵃʷ⁎⋅ \/ ¬ (work_check e A2 ⫤ aW) ⟶ᵃʷ⁎⋅).
-      { intros A1 A2 Heq. subst. dependent destruction H0. simpl in *.
-        eapply IHne; eauto; simpl; try lia. }
-      assert (Jg': forall A1 A2, A = typ_intersection A1 A2 ->
-                 (work_check e A2 ⫤ work_check e A1 ⫤ aW) ⟶ᵃʷ⁎⋅
-            \/ ¬ (work_check e A2 ⫤ work_check e A1 ⫤ aW) ⟶ᵃʷ⁎⋅ ).
-      { intros A1 A2 Heq. subst. dependent destruction H0. simpl in *.
-        eapply IHne; eauto; simpl; try lia. }
-      destruct Jg as [Jg | Jg]; eauto.
-      dependent destruction H; simpl in *.
-      * dependent destruction H0; simpl in *;
-          try solve [right; intro Hcontra; dependent destruction Hcontra; eapply Jg; eauto].
-        -- specialize (Jg1 A1 A2). destruct Jg1 as [Jg1 | Jg1]; eauto.
-           specialize (Jg2 A1 A2). destruct Jg2 as [Jg2 | Jg2]; eauto.
-           right. intro Hcontra. dependent destruction Hcontra.
-           apply Jg; auto. apply Jg1; auto. apply Jg2; auto.
-        -- specialize (Jg' A1 A2). destruct Jg' as [Jg' | Jg']; eauto.
-           right. intro Hcontra. dependent destruction Hcontra.
-           apply Jg; auto. apply Jg'; auto.
-      * dependent destruction H0; simpl in *;
-          try solve [right; intro Hcontra; dependent destruction Hcontra; eapply Jg; eauto].
-        -- specialize (Jg1 A1 A2). destruct Jg1 as [Jg1 | Jg1]; eauto.
-           specialize (Jg2 A1 A2). destruct Jg2 as [Jg2 | Jg2]; eauto.
-           right. intro Hcontra. dependent destruction Hcontra.
-           apply Jg; auto. apply Jg1; auto. apply Jg2; auto.
-        -- specialize (Jg' A1 A2). destruct Jg' as [Jg' | Jg']; eauto.
-           right. intro Hcontra. dependent destruction Hcontra.
-           apply Jg; auto. apply Jg'; auto.
-      * dependent destruction H1; simpl in *;
-          try solve [right; intro Hcontra; dependent destruction Hcontra; eapply Jg; eauto].
-        -- inst_cofinites_by (L `union` (ftvar_in_typ T) `union` (ftvar_in_aworklist aW)).
-           assert (Jgt:   (work_check (e ᵉ^ₑ exp_var_f x) typ_top ⫤ x ~ᵃ typ_bot;ᵃ aW) ⟶ᵃʷ⁎⋅ \/ 
-                        ¬ (work_check (e ᵉ^ₑ exp_var_f x) typ_top ⫤ x ~ᵃ typ_bot;ᵃ aW) ⟶ᵃʷ⁎⋅).
-           { eapply IHne; eauto; simpl; try lia. admit. (* safe: wf *)
-             assert (Hexp: exp_size (open_exp_wrt_exp e (exp_var_f x)) = exp_size e) by admit. (* should be fine *)
-             lia. }
-           destruct Jgt as [Jgt | Jgt].
-           ++ left. eapply a_wl_red__chk_abstop with (L := L `union` (ftvar_in_typ T) `union` (ftvar_in_aworklist aW)).
-              intros x' Hnin. admit. (* TODO: rename var *)
+        dependent destruction H; simpl in *.
+        -- dependent destruction H0; simpl in *;
+             try solve [right; intro Hcontra; dependent destruction Hcontra; eapply Jg; eauto].
+           ++ specialize (Jg1 A1 A2). destruct Jg1 as [Jg1 | Jg1]; eauto.
+              specialize (Jg2 A1 A2). destruct Jg2 as [Jg2 | Jg2]; eauto.
+              right. intro Hcontra. dependent destruction Hcontra.
+              apply Jg; auto. apply Jg1; auto. apply Jg2; auto.
+           ++ specialize (Jg' A1 A2). destruct Jg' as [Jg' | Jg']; eauto.
+              right. intro Hcontra. dependent destruction Hcontra.
+              apply Jg; auto. apply Jg'; auto.
+        -- dependent destruction H0; simpl in *;
+             try solve [right; intro Hcontra; dependent destruction Hcontra; eapply Jg; eauto].
+           ++ specialize (Jg1 A1 A2). destruct Jg1 as [Jg1 | Jg1]; eauto.
+              specialize (Jg2 A1 A2). destruct Jg2 as [Jg2 | Jg2]; eauto.
+              right. intro Hcontra. dependent destruction Hcontra.
+              apply Jg; auto. apply Jg1; auto. apply Jg2; auto.
+           ++ specialize (Jg' A1 A2). destruct Jg' as [Jg' | Jg']; eauto.
+              right. intro Hcontra. dependent destruction Hcontra.
+              apply Jg; auto. apply Jg'; auto.
+        -- dependent destruction H1; simpl in *;
+             try solve [right; intro Hcontra; dependent destruction Hcontra; eapply Jg; eauto].
+           ++ pick fresh x.
+              assert (Jgt: (work_check (e ᵉ^ₑ exp_var_f x) typ_top ⫤ᵃ x ~ᵃ typ_bot;ᵃ Γ) ⟶ᵃʷ⁎⋅ \/
+                         ¬ (work_check (e ᵉ^ₑ exp_var_f x) typ_top ⫤ᵃ x ~ᵃ typ_bot;ᵃ Γ) ⟶ᵃʷ⁎⋅).
+              { eapply IHne; eauto; simpl; try lia.
+                constructor; auto. constructor; auto. constructor; auto.
+                admit.
+                assert (Hexp: exp_size (x ~ᵃ typ_bot;ᵃ Γ) (e ᵉ^ₑ exp_var_f x) = exp_size Γ e) by admit. (* should be fine *)
+                lia. }
+              destruct Jgt as [Jgt | Jgt].
+              ** left. eapply a_wl_red__chk_abstop with (L := L `union` (ftvar_in_typ T) `union` (ftvar_in_aworklist Γ)).
+                  intros x' Hnin. admit. (* TODO: rename var *)
+              ** right. intro Hcontra. dependent destruction Hcontra.
+                  --- apply Jg; auto.
+                  --- admit. (* TODO: rename var  *) 
            ++ right. intro Hcontra. dependent destruction Hcontra.
-              ** apply Jg; auto.
-              ** admit. (* TODO: rename var  *) 
-        -- right. intro Hcontra. dependent destruction Hcontra.
-           ++ eapply Jg; eauto.
-           ++ admit. (* safe: wf *)
-        -- right. intro Hcontra. dependent destruction Hcontra.
-           ++ eapply Jg; eauto.
-           ++ eapply abind_etvar_stvar_false; eauto.
-        -- right. intro Hcontra. dependent destruction Hcontra; eauto.
-           admit. (* TODO *)
-        -- pick fresh x.
-           assert (JgArr:   (work_check (e ᵉ^ₑ exp_var_f x) A2 ⫤ x ~ᵃ A1;ᵃ aW) ⟶ᵃʷ⁎⋅ \/ 
-                          ¬ (work_check (e ᵉ^ₑ exp_var_f x) A2 ⫤ x ~ᵃ A1;ᵃ aW) ⟶ᵃʷ⁎⋅).
-           { eapply IHne; eauto; simpl; try lia. admit. (* safe: wf *)
-             assert (Hexp: exp_size (open_exp_wrt_exp e (exp_var_f x)) = exp_size e) by admit. (* should be fine *)
-             rewrite Hexp. lia. } 
-           destruct JgArr as [JgArr | JgArr]; auto.
-           ++ left. eapply a_wl_red__chk_absarrow with (L := union L (union (ftvar_in_typ T) (union (ftvar_in_typ A1) (ftvar_in_typ A2)))); eauto.
-              intros x' Hnin.              
-              admit. (* TODO: rename var *)
+              eapply Jg; eauto. unify_binds.
            ++ right. intro Hcontra. dependent destruction Hcontra.
-              ** apply Jg; auto.
-              ** admit. (* TODO: rename var *) 
-        -- specialize (Jg1 A1 A2). destruct Jg1 as [Jg1 | Jg1]; eauto.
+              eapply Jg; eauto. unify_binds.
+           ++ admit.
+           ++ pick fresh x.
+              assert (JgArr: (work_check (e ᵉ^ₑ exp_var_f x) A2 ⫤ᵃ x ~ᵃ A1;ᵃ Γ) ⟶ᵃʷ⁎⋅ \/ 
+                           ¬ (work_check (e ᵉ^ₑ exp_var_f x) A2 ⫤ᵃ x ~ᵃ A1;ᵃ Γ) ⟶ᵃʷ⁎⋅).
+              { eapply IHne; eauto; simpl; try lia.
+                constructor; auto. constructor; auto. constructor; auto.
+                admit. admit.
+                assert (Hexp: exp_size (x ~ᵃ A1;ᵃ Γ) (e ᵉ^ₑ exp_var_f x) = exp_size Γ e) by admit. (* should be fine *)
+                rewrite Hexp. lia. } 
+              destruct JgArr as [JgArr | JgArr]; auto.
+              ** left. eapply a_wl_red__chk_absarrow with (L := union L (union (ftvar_in_typ T) (union (ftvar_in_typ A1) (ftvar_in_typ A2)))); eauto.
+                  intros x' Hnin.              
+                  admit. (* TODO: rename var *)
+              ** right. intro Hcontra. dependent destruction Hcontra.
+                  --- apply Jg; auto.
+                  --- admit. (* TODO: rename var *) 
+        ++ specialize (Jg1 A1 A2). destruct Jg1 as [Jg1 | Jg1]; eauto.
            specialize (Jg2 A1 A2). destruct Jg2 as [Jg2 | Jg2]; eauto.
            right. intro Hcontra. dependent destruction Hcontra.
            apply Jg; auto. apply Jg1; auto. apply Jg2; auto.
-        -- specialize (Jg' A1 A2). destruct Jg' as [Jg' | Jg']; eauto.
+        ++ specialize (Jg' A1 A2). destruct Jg' as [Jg' | Jg']; eauto.
            right. intro Hcontra. dependent destruction Hcontra.
            apply Jg; auto. apply Jg'; auto.
-      * dependent destruction H1; simpl in *;
+      -- dependent destruction H1; simpl in *;
           try solve [right; intro Hcontra; dependent destruction Hcontra; eapply Jg; eauto].
-        -- specialize (Jg1 A1 A2). destruct Jg1 as [Jg1 | Jg1]; eauto.
+        ** specialize (Jg1 A1 A2). destruct Jg1 as [Jg1 | Jg1]; eauto.
            specialize (Jg2 A1 A2). destruct Jg2 as [Jg2 | Jg2]; eauto.
            right. intro Hcontra. dependent destruction Hcontra.
            apply Jg; auto. apply Jg1; auto. apply Jg2; auto.
-        -- specialize (Jg' A1 A2). destruct Jg' as [Jg' | Jg']; eauto.
+        ** specialize (Jg' A1 A2). destruct Jg' as [Jg' | Jg']; eauto.
            right. intro Hcontra. dependent destruction Hcontra.
            apply Jg; auto. apply Jg'; auto.
-      * destruct body5.
-        dependent destruction H0; simpl in *;
+      -- destruct body5.
+        dependent destruction H1; simpl in *;
           try solve [right; intro Hcontra; dependent destruction Hcontra; eapply Jg; eauto].
-        -- specialize (Jg1 A1 A2). destruct Jg1 as [Jg1 | Jg1]; eauto.
+        ** specialize (Jg1 A1 A2). destruct Jg1 as [Jg1 | Jg1]; eauto.
            specialize (Jg2 A1 A2). destruct Jg2 as [Jg2 | Jg2]; eauto.
            right. intro Hcontra. dependent destruction Hcontra.
            apply Jg; auto. apply Jg1; auto. apply Jg2; auto.
-        -- specialize (Jg' A1 A2). destruct Jg' as [Jg' | Jg']; eauto.
+        ** specialize (Jg' A1 A2). destruct Jg' as [Jg' | Jg']; eauto.
            right. intro Hcontra. dependent destruction Hcontra.
            apply Jg; auto. apply Jg'; auto.
-      * dependent destruction H1; simpl in *;
+      -- dependent destruction H1; simpl in *;
           try solve [right; intro Hcontra; dependent destruction Hcontra; eapply Jg; eauto].
-        -- specialize (Jg1 A1 A2). destruct Jg1 as [Jg1 | Jg1]; eauto.
+        ** specialize (Jg1 A1 A2). destruct Jg1 as [Jg1 | Jg1]; eauto.
            specialize (Jg2 A1 A2). destruct Jg2 as [Jg2 | Jg2]; eauto.
            right. intro Hcontra. dependent destruction Hcontra.
            apply Jg; auto. apply Jg1; auto. apply Jg2; auto.
-        -- specialize (Jg' A1 A2). destruct Jg' as [Jg' | Jg']; eauto.
+        ** specialize (Jg' A1 A2). destruct Jg' as [Jg' | Jg']; eauto.
            right. intro Hcontra. dependent destruction Hcontra.
            apply Jg; auto. apply Jg'; auto.
-      * dependent destruction H1; simpl in *;
+      -- dependent destruction H1; simpl in *;
           try solve [right; intro Hcontra; dependent destruction Hcontra; eapply Jg; eauto].
-        -- specialize (Jg1 A1 A2). destruct Jg1 as [Jg1 | Jg1]; eauto.
+        ** specialize (Jg1 A1 A2). destruct Jg1 as [Jg1 | Jg1]; eauto.
            specialize (Jg2 A1 A2). destruct Jg2 as [Jg2 | Jg2]; eauto.
            right. intro Hcontra. dependent destruction Hcontra.
            apply Jg; auto. apply Jg1; auto. apply Jg2; auto.
-        -- specialize (Jg' A1 A2). destruct Jg' as [Jg' | Jg']; eauto.
+        ** specialize (Jg' A1 A2). destruct Jg' as [Jg' | Jg']; eauto.
            right. intro Hcontra. dependent destruction Hcontra.
            apply Jg; auto. apply Jg'; auto.
-    + simpl in *. dependent destruction Hm. dependent destruction H1.
-      dependent destruction H;
-        try solve [right; intro Hcontra; dependent destruction Hcontra].
-      * assert (Jg:   (work_infabs (typ_arrow typ_top typ_bot) c ⫤ Γ) ⟶ᵃʷ⁎⋅ \/ 
-                    ¬ (work_infabs (typ_arrow typ_top typ_bot) c ⫤ Γ) ⟶ᵃʷ⁎⋅).
-        { eapply IHna; eauto; simpl in *; try lia. }
-        destruct Jg as [Jg | Jg]; eauto.
-        right. intro Hcontra.
-        dependent destruction Hcontra.
-        apply Jg; auto.
-      * right. intro Hcontra.
-        dependent destruction Hcontra.
-        admit. (* safe: wf *)
-      * right. intro Hcontra.
-        dependent destruction Hcontra.
-        admit. (* safe: wf *)
-      * admit. (* TODO *)
-      * destruct (apply_cont_dec c (typ_arrow A1 A2)) as [[w Happly] | Happly];
+      * simpl in *. dependent destruction H;
+          try solve [right; intro Hcontra; dependent destruction Hcontra].
+        -- assert (Jg:   (work_infabs (typ_arrow typ_top typ_bot) cd ⫤ᵃ Γ) ⟶ᵃʷ⁎⋅ \/ 
+                       ¬ (work_infabs (typ_arrow typ_top typ_bot) cd ⫤ᵃ Γ) ⟶ᵃʷ⁎⋅).
+          { eapply IHna; eauto; simpl in *; try lia. }
+          destruct Jg as [Jg | Jg]; eauto.
+          right. intro Hcontra.
+          dependent destruction Hcontra.
+          apply Jg; auto.
+        -- right. intro Hcontra.
+           dependent destruction Hcontra. unify_binds.
+        -- right. intro Hcontra.
+           dependent destruction Hcontra. unify_binds.
+        -- admit. (* TODO *)
+      -- destruct (apply_contd_dec cd A1 A2) as [[w Happly] | Happly];
           try solve [right; intro Hcontra; dependent destruction Hcontra; dependent destruction Hcontra;
                      eapply Happly; eauto].
-        assert (Jg: a_wl_red (aworklist_conswork Γ w) \/ 
-                    ~ a_wl_red (aworklist_conswork Γ w)).
-        { destruct (measp_wl_total (aworklist_conswork Γ w)) as [m Hm'].
-          admit. (* safe: wf *)
-          eapply IHnaj; eauto; simpl in *; try lia.
-          admit. (* safe: wf *)
-          eapply apply_cont_exp_size in Happly; lia.
-          eapply apply_cont_judge_size in Happly; lia.
-          eapply apply_cont_inftapp_depth_arr in Happly. lia.
-          eapply apply_cont_inftapp_judge_size in Happly; lia.
-          eapply apply_cont_infabs_depth_arr in Happly; lia.
-          eapply apply_cont_infabs_judge_size in Happly; lia. }
-        destruct Jg as [Jg | Jg]; eauto.
-        right. intro Hcontra.
-        dependent destruction Hcontra.
-        dependent destruction Hcontra.
-        eapply apply_cont_det in Happly; eauto.
-        subst. eauto.
-      * pick fresh X. inst_cofinites_with X.
-        assert (Jg: a_wl_red (aworklist_conswork (aworklist_constvar Γ X abind_etvar_empty) (work_infabs (open_typ_wrt_typ A (typ_var_f X)) c)) \/
-                    ~ a_wl_red (aworklist_conswork (aworklist_constvar Γ X abind_etvar_empty) (work_infabs (open_typ_wrt_typ A (typ_var_f X)) c))).
-        { assert (Heq: infabs_depth (open_typ_wrt_typ A (typ_var_f X)) = infabs_depth A) by admit. (* should be fine *)
-          eapply IHna; eauto; simpl in *; try lia.
-          admit. (* safe: wf *) }
-        destruct Jg as [Jg | Jg]; eauto.
-        -- left. inst_cofinites_for a_wl_red__infabs_all.
-           intros X' Hnin. 
-           apply a_wl_red_rename_tvar with (X:=X) (X':=X') in Jg.
-           ++ simpl in Jg.
-              unfold eq_dec in Jg.
-              destruct (EqDec_eq_of_X X X) in Jg.
-              ** rewrite rename_tvar_in_aworklist_fresh_eq in Jg; auto.
-                 rewrite subst_tvar_in_cont_fresh_eq in Jg; auto.
-                 rewrite subst_tvar_in_typ_open_typ_wrt_typ_tvar2 in Jg; auto.
-              ** contradiction.
-            ++ admit.
-            ++ admit. (* wf *)
-            ++ simpl. rewrite ftvar_in_typ_open_typ_wrt_typ_upper. auto.
-        -- right. intro Hcontra.
-           dependent destruction Hcontra.
-           pick fresh X1.
-           inst_cofinites_with X1.
-           apply a_wl_red_rename_tvar with (X:=X1) (X':=X) in H2; auto.
-           ++ simpl in H2.
-              unfold eq_dec in H2.
-              destruct (EqDec_eq_of_X X1 X1) in H2.
-              ** rewrite rename_tvar_in_aworklist_fresh_eq in H2; auto.
-                  rewrite subst_tvar_in_cont_fresh_eq in H2; auto.
-                  rewrite subst_tvar_in_typ_open_typ_wrt_typ_tvar2 in H2; auto.
-              ** contradiction.
-            ++ admit. (* wf *)  
-            ++ simpl. rewrite ftvar_in_typ_open_typ_wrt_typ_upper. auto.
-      * assert (Jg: a_wl_red (aworklist_conswork Γ (work_infabs A1  (  (cont_infabsunion A2 c)  ) )) \/
-                  ~ a_wl_red (aworklist_conswork Γ (work_infabs A1  (  (cont_infabsunion A2 c)  ) ))).
-        { eapply IHna; eauto; simpl in *; try lia. }
-        destruct Jg as [Jg | Jg]; eauto.
-        right. intro Hcontra.
-        dependent destruction Hcontra.
-        apply Jg; auto.
-      * assert (Jg1: a_wl_red (aworklist_conswork Γ (work_infabs A1 c)) \/
-                   ~ a_wl_red (aworklist_conswork Γ (work_infabs A1 c))).
-        { eapply IHna; eauto; simpl in *; try lia. }
-        assert (Jg2: a_wl_red (aworklist_conswork Γ (work_infabs A2 c)) \/
-                   ~ a_wl_red (aworklist_conswork Γ (work_infabs A2 c))).
-        { eapply IHna; eauto; simpl in *; try lia. }
-        destruct Jg1 as [Jg1 | Jg1]; eauto.
-        destruct Jg2 as [Jg2 | Jg2]; eauto.
-        right. intro Hcontra.
-        dependent destruction Hcontra.
-        apply Jg1; auto. apply Jg2; auto.
-    + simpl in *. dependent destruction Hm. dependent destruction H;
-        try solve [right; intro Hcontra; dependent destruction Hcontra].
-      assert (Jg:  (work_infabs A2 (cont_unioninfabs (typ_arrow A1 A0) c) ⫤ aW) ⟶ᵃʷ⁎⋅ \/
-                 ¬ (work_infabs A2 (cont_unioninfabs (typ_arrow A1 A0) c) ⫤ aW) ⟶ᵃʷ⁎⋅).
-      { eapply IHnaj; eauto; simpl in *; try lia. }
+         assert (Jg: (w ⫤ᵃ Γ) ⟶ᵃʷ⁎⋅ \/ ¬ (w ⫤ᵃ Γ) ⟶ᵃʷ⁎⋅).
+         { eapply IHnaj; eauto; simpl in *; try lia.
+           eapply a_wf_wl_apply_contd; eauto.
+           eapply apply_contd_exp_size with (Γ := Γ) in Happly; lia.
+           eapply apply_contd_judge_size in Happly; lia.
+           eapply apply_contd_inftapp_depth in Happly; lia.
+           eapply apply_contd_inftapp_judge_size in Happly; lia.
+           eapply apply_contd_infabs_depth in Happly; lia.
+           eapply apply_contd_infabs_judge_size in Happly; lia. }
+         destruct Jg as [Jg | Jg]; eauto.
+         right. intro Hcontra.
+         dependent destruction Hcontra.
+         dependent destruction Hcontra.
+         eapply apply_contd_det in Happly; eauto.
+         subst. eauto.
+      -- pick fresh X. inst_cofinites_with X.
+         assert (Jg: (work_infabs (A ᵗ^ₜ X) cd ⫤ᵃ X ~ᵃ ⬒ ;ᵃ Γ) ⟶ᵃʷ⁎⋅ \/
+                   ¬ (work_infabs (A ᵗ^ₜ X) cd ⫤ᵃ X ~ᵃ ⬒ ;ᵃ Γ) ⟶ᵃʷ⁎⋅).
+         { assert (Heq: infabs_depth (open_typ_wrt_typ A (typ_var_f X)) = infabs_depth A) by admit. (* should be fine *)
+           eapply IHna; eauto; simpl in *; try lia.
+           constructor; simpl; auto. constructor; simpl; auto. constructor; simpl; auto.
+           eapply a_wf_typ_tvar_etvar with (Σ2 := nil). simpl. auto.
+           eapply a_wf_contd_weaken_cons; auto.
+           admit. (* TODO *) }
+         destruct Jg as [Jg | Jg]; eauto.
+         ++ left. inst_cofinites_for a_wl_red__infabs_all.
+            intros X' Hnin.
+            apply rename_tvar_in_a_wf_wwl_a_wl_red with (X:=X) (Y:=X') in Jg.
+            ** simpl in Jg. destruct_eq_atom.
+               rewrite rename_tvar_in_aworklist_fresh_eq in Jg; auto.
+               rewrite subst_tvar_in_contd_fresh_eq in Jg; auto.
+               rewrite subst_tvar_in_typ_open_typ_wrt_typ_tvar2 in Jg; auto.
+            ** unfold not. intros. subst. solve_notin_eq X'.
+            ** eapply a_wf_wl_a_wf_wwl.
+               constructor; simpl; auto. constructor; simpl; auto. constructor; simpl; auto.
+               eapply a_wf_typ_tvar_etvar with (Σ2 := nil). simpl. auto.
+               eapply a_wf_contd_weaken_cons; auto.
+            ** simpl. auto.
+         ++ right. intro Hcontra.
+            dependent destruction Hcontra.
+            pick fresh X1. inst_cofinites_with X1.
+            apply rename_tvar_in_a_wf_wwl_a_wl_red with (X:=X1) (Y:=X) in H3; auto.
+            ** simpl in H3. destruct_eq_atom.
+               rewrite rename_tvar_in_aworklist_fresh_eq in H3; auto.
+               rewrite subst_tvar_in_contd_fresh_eq in H3; auto.
+               rewrite subst_tvar_in_typ_open_typ_wrt_typ_tvar2 in H3; auto.
+            ** eapply a_wf_wl_a_wf_wwl.
+               constructor; simpl; auto. constructor; auto. admit.
+      -- assert (Jg: (work_infabs A1 (contd_infabsunion A2 cd) ⫤ᵃ Γ) ⟶ᵃʷ⁎⋅ \/
+                   ¬ (work_infabs A1 (contd_infabsunion A2 cd) ⫤ᵃ Γ) ⟶ᵃʷ⁎⋅).
+         { eapply IHna; eauto; simpl in *; try lia. }
+         destruct Jg as [Jg | Jg]; eauto.
+         right. intro Hcontra.
+         dependent destruction Hcontra.
+         apply Jg; auto.
+      -- assert (Jg1: (work_infabs A1 cd ⫤ᵃ Γ) ⟶ᵃʷ⁎⋅ \/
+                    ¬ (work_infabs A1 cd ⫤ᵃ Γ) ⟶ᵃʷ⁎⋅).
+         { eapply IHna; eauto; simpl in *; try lia. }
+         assert (Jg2: (work_infabs A2 cd ⫤ᵃ Γ) ⟶ᵃʷ⁎⋅ \/
+                    ¬ (work_infabs A2 cd ⫤ᵃ Γ) ⟶ᵃʷ⁎⋅).
+         { eapply IHna; eauto; simpl in *; try lia. }
+         destruct Jg1 as [Jg1 | Jg1]; eauto.
+         destruct Jg2 as [Jg2 | Jg2]; eauto.
+         right. intro Hcontra.
+         dependent destruction Hcontra.
+         apply Jg1; auto. apply Jg2; auto.
+    * simpl in *. dependent destruction H;
+      try solve [right; intro Hcontra; dependent destruction Hcontra].
+      assert (Jg:  (work_infabs A2 (contd_unioninfabs A1 B1 cd) ⫤ᵃ Γ) ⟶ᵃʷ⁎⋅ \/
+                 ¬ (work_infabs A2 (contd_unioninfabs A1 B1 cd) ⫤ᵃ Γ) ⟶ᵃʷ⁎⋅).
+      { eapply IHnaj; eauto; simpl in *; try lia. constructor; auto. }
+      destruct Jg as [Jg | Jg]; eauto.
+      right. intro Hcontra. 
+      dependent destruction Hcontra. eauto.
+    * dependent destruction H; try solve [right; intro Hcontra; dependent destruction Hcontra].
+      assert (Jg:  (work_applys cs B ⫤ᵃ work_check e A ⫤ᵃ Γ) ⟶ᵃʷ⁎⋅ \/
+                 ¬ (work_applys cs B ⫤ᵃ work_check e A ⫤ᵃ Γ) ⟶ᵃʷ⁎⋅).
+      { eapply IHnj; eauto; simpl in *; try lia. constructor; auto. admit. }
       destruct Jg as [Jg | Jg]; eauto.
       right. intro Hcontra.
       dependent destruction Hcontra. eauto.
-    + dependent destruction H; try solve [right; intro Hcontra; dependent destruction Hcontra].
-      assert (Jg:  (work_apply c A2 ⫤ work_check e A1 ⫤ aW) ⟶ᵃʷ⁎⋅ \/
-                 ¬ (work_apply c A2 ⫤ work_check e A1 ⫤ aW) ⟶ᵃʷ⁎⋅).
-      { (* TODO!! *) admit. }
-      destruct Jg as [Jg | Jg]; eauto.
-      right. intro Hcontra.
-      dependent destruction Hcontra. eauto.
-    + simpl in *. dependent destruction Hm. dependent destruction H2.
-      dependent destruction H;
+    * simpl in *. dependent destruction H;
         try solve [right; intro Hcontra; dependent destruction Hcontra].
-      * destruct (apply_cont_dec c typ_bot) as [[w Happly] | Happly];
-        try solve [right; intro Hcontra; dependent destruction Hcontra; dependent destruction Hcontra;
-          eapply Happly; eauto].
-        assert (Jg: a_wl_red (aworklist_conswork Γ w) \/
-                  ~ a_wl_red (aworklist_conswork Γ w)).
-        { destruct (measp_wl_total (aworklist_conswork Γ w)) as [m Hm'].
-          admit. (* safe: wf *)
-          eapply IHntj; eauto; simpl in *; try lia.
-          admit. (* safe: wf *)
-          eapply apply_cont_exp_size in Happly; lia.
-          eapply apply_cont_judge_size in Happly; lia.
-          eapply apply_cont_inftapp_depth_bot in Happly.
-          rewrite mult_0_r in Ht. lia.
-          eapply apply_cont_inftapp_judge_size in Happly; lia. }
-        destruct Jg as [Jg | Jg]; eauto.
-        right. intro Hcontra.
-        dependent destruction Hcontra.
-        dependent destruction Hcontra.
-        eapply apply_cont_det in Happly; eauto.
-        subst. eauto.
-      * destruct (apply_cont_dec c (open_typ_wrt_typ A A2)) as [[w Happly] | Happly];
-        try solve [right; intro Hcontra; dependent destruction Hcontra; dependent destruction Hcontra;
-          eapply Happly; eauto].
-        assert (Jg: (w ⫤ Γ) ⟶ᵃʷ⁎⋅ \/ ¬ (w ⫤ Γ) ⟶ᵃʷ⁎⋅).
-        { destruct (measp_wl_total (aworklist_conswork Γ w)) as [m Hm'].
-          admit. (* safe: wf *)
-          eapply IHntj; eauto; simpl in *; try lia.
-          admit. (* safe: wf *)
-          eapply apply_cont_exp_size in Happly; lia.
-          eapply apply_cont_judge_size in Happly; lia.
-          eapply apply_cont_inftapp_depth in Happly.
-          assert (Hfact: inftapp_depth (open_typ_wrt_typ A A2) < (1 + inftapp_depth A) * (1 + inftapp_depth A2))
-            by eapply inftapp_depth_open_typ_wrt_typ.
-          assert (Hfact': inftapp_depth_work w <= inftapp_depth_cont_tail_rec c ((1 + inftapp_depth A) * (1 + inftapp_depth A2))).
-          { eapply le_trans; eauto. eapply inftapp_depth_cont_tail_rec_le. lia. }
-          assert (Hfact'': inftapp_depth_cont_tail_rec c ((1 + inftapp_depth A) * (1 + inftapp_depth A2)) <= inftapp_depth_cont_tail_rec c
-          (S
-             (inftapp_depth A +
-              S
-                (inftapp_depth A +
-                 inftapp_depth A2 * S (inftapp_depth A))))).
-          { eapply inftapp_depth_cont_tail_rec_le; eauto; lia. }
-          lia.
-          eapply apply_cont_inftapp_judge_size in Happly; lia. }
-        destruct Jg as [Jg | Jg]; eauto.
-        right. intro Hcontra.
-        dependent destruction Hcontra.
-        dependent destruction Hcontra.  
-        eapply apply_cont_det in Happly; eauto.
-        subst. eauto.
-      * assert (Jg:   (work_inftapp A1 A2 (cont_inftappunion A0 A2 c) ⫤ Γ) ⟶ᵃʷ⁎⋅ \/
-                    ¬ (work_inftapp A1 A2 (cont_inftappunion A0 A2 c) ⫤ Γ) ⟶ᵃʷ⁎⋅).
-        { eapply IHnt; eauto; simpl in *; try lia.
-          assert (inftapp_depth_cont_tail_rec c
-          (inftapp_depth A0 * S (S (inftapp_depth A2)) + 1 +
-           (inftapp_depth A1 +
-            (inftapp_depth A1 + inftapp_depth A2 * inftapp_depth A1)))
-            < inftapp_depth_cont_tail_rec c
-            (S
-               (inftapp_depth A1 + inftapp_depth A0 +
-                S
-                  (inftapp_depth A1 + inftapp_depth A0 +
-                   inftapp_depth A2 *
-                   S (inftapp_depth A1 + inftapp_depth A0))))).
-          { eapply inftapp_depth_cont_tail_rec_lt; eauto; try lia. }
-          lia. }
-        destruct Jg as [Jg | Jg]; eauto.
-        right. intro Hcontra.
-        dependent destruction Hcontra.
-        apply Jg; auto.
-      * assert (Jg1: (work_inftapp A1 A2 c ⫤ Γ) ⟶ᵃʷ⁎⋅ \/ ¬ (work_inftapp A1 A2 c ⫤ Γ) ⟶ᵃʷ⁎⋅).
-        { eapply IHnt; eauto; simpl in *; try lia.
-          assert (inftapp_depth_cont_tail_rec c
-          (inftapp_depth A1 +
-           (inftapp_depth A1 + inftapp_depth A2 * inftapp_depth A1))
-                    <  inftapp_depth_cont_tail_rec c
-                    (S
-                       (inftapp_depth A1 + inftapp_depth A0 +
-                        S
-                          (inftapp_depth A1 + inftapp_depth A0 +
-                           inftapp_depth A2 *
-                           S (inftapp_depth A1 + inftapp_depth A0))))).
-          { eapply inftapp_depth_cont_tail_rec_lt; eauto; try lia. }
-          lia. }
-        assert (Jg2: (work_inftapp A0 A2 c ⫤ Γ) ⟶ᵃʷ⁎⋅ \/ ¬ (work_inftapp A0 A2 c ⫤ Γ) ⟶ᵃʷ⁎⋅).
-        { eapply IHnt; eauto; simpl in *; try lia.
-          assert (inftapp_depth_cont_tail_rec c
-          (inftapp_depth A0 +
-           (inftapp_depth A0 + inftapp_depth A2 * inftapp_depth A0))
-                    < inftapp_depth_cont_tail_rec c
-                    (S
-                       (inftapp_depth A1 + inftapp_depth A0 +
-                        S
-                          (inftapp_depth A1 + inftapp_depth A0 +
-                           inftapp_depth A2 *
-                           S (inftapp_depth A1 + inftapp_depth A0))))).
-          { eapply inftapp_depth_cont_tail_rec_lt; eauto; try lia. }
-          lia. }
-        destruct Jg1 as [Jg1 | Jg1]; eauto.
-        destruct Jg2 as [Jg2 | Jg2]; eauto.
-        right. intro Hcontra.
-        dependent destruction Hcontra.
-        apply Jg1; auto. apply Jg2; auto.
-    + simpl in *. dependent destruction Hm. dependent destruction H3.
-      assert (Jg:  (work_inftapp A2 B (cont_unioninftapp A1 c) ⫤ Γ) ⟶ᵃʷ⁎⋅ \/ 
-                 ¬ (work_inftapp A2 B (cont_unioninftapp A1 c) ⫤ Γ) ⟶ᵃʷ⁎⋅).
+      -- destruct (apply_conts_dec cs typ_bot) as [[w Happly] | Happly];
+         try solve [right; intro Hcontra; dependent destruction Hcontra; dependent destruction Hcontra;
+           eapply Happly; eauto].
+         assert (Jg: a_wl_red (aworklist_cons_work Γ w) \/
+                   ~ a_wl_red (aworklist_cons_work Γ w)).
+         { eapply IHntj; eauto; simpl in *; try lia.
+           eapply a_wf_wl_apply_conts; eauto.
+           eapply apply_conts_exp_size with (Γ := Γ) in Happly; lia.
+           eapply apply_conts_judge_size in Happly; lia.
+           admit. (* TODO *)
+           eapply apply_conts_inftapp_judge_size in Happly; lia. }
+         destruct Jg as [Jg | Jg]; eauto.
+         right. intro Hcontra.
+         dependent destruction Hcontra.
+         dependent destruction Hcontra.
+         eapply apply_conts_det in Happly; eauto.
+         subst. eauto.
+      -- destruct (apply_conts_dec cs (open_typ_wrt_typ A A2)) as [[w Happly] | Happly];
+         try solve [right; intro Hcontra; dependent destruction Hcontra; dependent destruction Hcontra;
+           eapply Happly; eauto].
+         assert (Jg: (w ⫤ᵃ Γ) ⟶ᵃʷ⁎⋅ \/ ¬ (w ⫤ᵃ Γ) ⟶ᵃʷ⁎⋅).
+         { eapply IHntj; eauto; simpl in *; try lia.
+           eapply a_wf_wl_apply_conts; eauto.
+           constructor; auto. constructor; auto.
+           eapply a_wf_typ_all_open; eauto.
+           eapply apply_conts_exp_size with (Γ := Γ) in Happly; lia.
+           eapply apply_conts_judge_size in Happly; lia.
+           eapply apply_conts_inftapp_depth in Happly.
+           assert (Hfact: inftapp_depth (open_typ_wrt_typ A A2) < (1 + inftapp_depth A) * (1 + inftapp_depth A2))
+             by eapply inftapp_depth_open_typ_wrt_typ.
+           assert (Hfact': inftapp_depth_work w <= inftapp_depth_conts_tail_rec cs ((1 + inftapp_depth A) * (1 + inftapp_depth A2))).
+           { eapply le_trans; eauto. eapply inftapp_depth_conts_tail_rec_le. lia. }
+           assert (Hfact'': inftapp_depth_conts_tail_rec cs ((1 + inftapp_depth A) * (1 + inftapp_depth A2)) <= inftapp_depth_conts_tail_rec cs (S (inftapp_depth A + S (inftapp_depth A + inftapp_depth A2 * S (inftapp_depth A))))).
+           { eapply inftapp_depth_conts_tail_rec_le; eauto; lia. }
+           lia.
+           eapply apply_conts_inftapp_judge_size in Happly; lia. }
+         destruct Jg as [Jg | Jg]; eauto.
+         right. intro Hcontra.
+         dependent destruction Hcontra.
+         dependent destruction Hcontra.
+         eapply apply_conts_det in Happly; eauto.
+         subst. eauto.
+      -- assert (Jg: (work_inftapp A1 A2 (conts_inftappunion A0 A2 cs) ⫤ᵃ Γ) ⟶ᵃʷ⁎⋅ \/
+                   ¬ (work_inftapp A1 A2 (conts_inftappunion A0 A2 cs) ⫤ᵃ Γ) ⟶ᵃʷ⁎⋅).
+         { eapply IHnt; eauto; simpl in *; try lia.
+           assert (inftapp_depth_conts_tail_rec cs
+                    (inftapp_depth A0 * S (S (inftapp_depth A2)) + 1 +
+                      (inftapp_depth A1 + (inftapp_depth A1 + inftapp_depth A2 * inftapp_depth A1)))
+                  < inftapp_depth_conts_tail_rec cs
+                    (S (inftapp_depth A1 + inftapp_depth A0 +
+                       S (inftapp_depth A1 + inftapp_depth A0 +
+                         inftapp_depth A2 * S (inftapp_depth A1 + inftapp_depth A0))))).
+           { eapply inftapp_depth_conts_tail_rec_lt; eauto; try lia. }
+           lia. }
+         destruct Jg as [Jg | Jg]; eauto.
+         right. intro Hcontra.
+         dependent destruction Hcontra.
+         apply Jg; auto.
+      -- assert (Jg1: (work_inftapp A1 A2 cs ⫤ᵃ Γ) ⟶ᵃʷ⁎⋅ \/ ¬ (work_inftapp A1 A2 cs ⫤ᵃ Γ) ⟶ᵃʷ⁎⋅).
+         { eapply IHnt; eauto; simpl in *; try lia.
+           assert (inftapp_depth_conts_tail_rec cs
+                    (inftapp_depth A1 +
+                      (inftapp_depth A1 + inftapp_depth A2 * inftapp_depth A1))
+                  < inftapp_depth_conts_tail_rec cs
+                    (S (inftapp_depth A1 + inftapp_depth A0 +
+                        S (inftapp_depth A1 + inftapp_depth A0 +
+                           inftapp_depth A2 * S (inftapp_depth A1 + inftapp_depth A0))))).
+           { eapply inftapp_depth_conts_tail_rec_lt; eauto; try lia. }
+           lia. }
+         assert (Jg2: (work_inftapp A0 A2 cs ⫤ᵃ Γ) ⟶ᵃʷ⁎⋅ \/ ¬ (work_inftapp A0 A2 cs ⫤ᵃ Γ) ⟶ᵃʷ⁎⋅).
+         { eapply IHnt; eauto; simpl in *; try lia.
+           assert (inftapp_depth_conts_tail_rec cs
+                    (inftapp_depth A0 +
+                      (inftapp_depth A0 + inftapp_depth A2 * inftapp_depth A0))
+                  < inftapp_depth_conts_tail_rec cs
+                    (S (inftapp_depth A1 + inftapp_depth A0 +
+                        S (inftapp_depth A1 + inftapp_depth A0 +
+                           inftapp_depth A2 * S (inftapp_depth A1 + inftapp_depth A0))))).
+           { eapply inftapp_depth_conts_tail_rec_lt; eauto; try lia. }
+           lia. }
+         destruct Jg1 as [Jg1 | Jg1]; eauto.
+         destruct Jg2 as [Jg2 | Jg2]; eauto.
+         right. intro Hcontra.
+         dependent destruction Hcontra.
+         apply Jg1; auto. apply Jg2; auto.
+    * simpl in *.
+      assert (Jg:  (work_inftapp A2 B (conts_unioninftapp A1 cs) ⫤ᵃ Γ) ⟶ᵃʷ⁎⋅ \/ 
+                 ¬ (work_inftapp A2 B (conts_unioninftapp A1 cs) ⫤ᵃ Γ) ⟶ᵃʷ⁎⋅).
       { eapply IHntj; eauto; simpl; try lia.
-        assert (inftapp_depth_cont_tail_rec c
-        (S
-           (inftapp_depth A1 +
-            (inftapp_depth A2 +
-             (inftapp_depth A2 + inftapp_depth B * inftapp_depth A2))))
-             <= inftapp_depth_cont_tail_rec c
-             (inftapp_depth A1 +
-              inftapp_depth A2 * S (S (inftapp_depth B)) + 1)).
-          { eapply inftapp_depth_cont_tail_rec_le; eauto; try lia. }
+        assert (inftapp_depth_conts_tail_rec cs
+                 (S (inftapp_depth A1 + (inftapp_depth A2 + (inftapp_depth A2 + inftapp_depth B * inftapp_depth A2))))
+            <= inftapp_depth_conts_tail_rec cs
+                 (inftapp_depth A1 + inftapp_depth A2 * S (S (inftapp_depth B)) + 1)).
+        { eapply inftapp_depth_conts_tail_rec_le; eauto; try lia. }
         lia. }
       destruct Jg as [Jg | Jg]; eauto.
       right. intro Hcontra.
       dependent destruction Hcontra.
       apply Jg; auto.
-    + simpl in *. dependent destruction Hm. dependent destruction H2.
-      destruct (apply_cont_dec c (typ_union A1 A2)) as [[w Happly] | Happly];
+    * simpl in *.
+      destruct (apply_conts_dec cs (typ_union A1 A2)) as [[w Happly] | Happly];
       try solve [right; intro Hcontra; dependent destruction Hcontra; dependent destruction Hcontra;
         eapply Happly; eauto].
-      assert (Jg: (w ⫤ Γ) ⟶ᵃʷ⁎⋅ \/ ¬ (w ⫤ Γ) ⟶ᵃʷ⁎⋅).
-      { destruct (measp_wl_total (aworklist_conswork Γ w)) as [m Hm'].
-        admit. (* safe: wf *)
-        eapply IHntj; eauto; simpl in *; try lia.
-        admit. (* safe: wf *)
-        eapply apply_cont_exp_size in Happly; lia.
-        eapply apply_cont_judge_size in Happly; lia.
-        eapply apply_cont_inftapp_depth in Happly.
-        assert (inftapp_depth_cont_tail_rec c
-        (inftapp_depth (typ_union A1 A2)) <= inftapp_depth_cont_tail_rec c
-        (S (inftapp_depth A1 + inftapp_depth A2))). 
-        { eapply inftapp_depth_cont_tail_rec_le; eauto; lia. }
+      assert (Jg: (w ⫤ᵃ Γ) ⟶ᵃʷ⁎⋅ \/ ¬ (w ⫤ᵃ Γ) ⟶ᵃʷ⁎⋅).
+      { eapply IHntj; eauto; simpl in *; try lia.
+        eapply a_wf_wl_apply_conts; eauto.
+        eapply apply_conts_exp_size with (Γ := Γ) in Happly; lia.
+        eapply apply_conts_judge_size in Happly; lia.
+        eapply apply_conts_inftapp_depth in Happly.
+        assert (inftapp_depth_conts_tail_rec cs (inftapp_depth (typ_union A1 A2))
+             <= inftapp_depth_conts_tail_rec cs (S (inftapp_depth A1 + inftapp_depth A2))). 
+        { eapply inftapp_depth_conts_tail_rec_le; eauto; lia. }
         lia.
-        eapply apply_cont_inftapp_judge_size in Happly; lia. }
+        eapply apply_conts_inftapp_judge_size in Happly; lia. }
       destruct Jg as [Jg | Jg]; eauto.
       right. intro Hcontra.
       dependent destruction Hcontra.
       dependent destruction Hcontra.
-      eapply apply_cont_det in Happly; eauto.
+      eapply apply_conts_det in Happly; eauto.
       subst. eauto.
-    + simpl in *. dependent destruction Hm. dependent destruction H2.
-      dependent destruction H;
+    * simpl in *. dependent destruction H;
         try solve [right; intro Hcontra; dependent destruction Hcontra];
       dependent destruction H1;
         try solve [right; intro Hcontra; dependent destruction Hcontra].
-      destruct (apply_cont_dec c (typ_arrow  ( (typ_intersection A1 A2) )   ( (typ_union A0 A3) ) )) as [[w Happly] | Happly];
+      destruct (apply_contd_dec cd ( (typ_intersection A1 A2) )   ( (typ_union B1 B2) ) ) as [[w Happly] | Happly];
       try solve [right; intro Hcontra; dependent destruction Hcontra; dependent destruction Hcontra;
         eapply Happly; eauto].
-      assert (Jg: (w ⫤ Γ) ⟶ᵃʷ⁎⋅ \/ ¬ (w ⫤ Γ) ⟶ᵃʷ⁎⋅).
-      { destruct (measp_wl_total (w ⫤ Γ)) as [m Hm'].
-        admit. (* safe: wf *)
-        eapply IHnaj; eauto; simpl in *; try lia.
-        admit. (* safe: wf *)
-        eapply apply_cont_exp_size in Happly; lia.
-        eapply apply_cont_judge_size in Happly; lia.
-        (* eapply apply_cont_inftapp_all_size_arr in Happly; lia. *)
-        eapply apply_cont_inftapp_depth_arr in Happly; lia.
-        eapply apply_cont_inftapp_judge_size in Happly; lia.
-        eapply apply_cont_infabs_depth_arr in Happly; lia.
-        eapply apply_cont_infabs_judge_size in Happly; lia. }
+      assert (Jg: (w ⫤ᵃ Γ) ⟶ᵃʷ⁎⋅ \/ ¬ (w ⫤ᵃ Γ) ⟶ᵃʷ⁎⋅).
+      { eapply IHnaj; eauto; simpl in *; try lia.
+        eapply a_wf_wl_apply_contd; eauto. constructor; auto.
+        eapply apply_contd_exp_size with (Γ := Γ) in Happly; lia.
+        eapply apply_contd_judge_size in Happly; lia.
+        eapply apply_contd_inftapp_depth in Happly; lia.
+        eapply apply_contd_inftapp_judge_size in Happly; lia.
+        eapply apply_contd_infabs_depth in Happly; lia.
+        eapply apply_contd_infabs_judge_size in Happly; lia. }
       destruct Jg as [Jg | Jg]; eauto.
       right. intro Hcontra.
       dependent destruction Hcontra.
       dependent destruction Hcontra.
-      eapply apply_cont_det in Happly; eauto.
+      eapply apply_contd_det in Happly; eauto.
       subst. eauto.
-    + simpl in *. dependent destruction Hm. dependent destruction H1.
-      dependent destruction H1. dependent destruction H3.
-      assert (Hw': weight A >= 1) by apply weight_gt_0.
-      assert (Hw'0: weight A0 >= 1) by apply weight_gt_0.
-      assert (Jg: a_wl_red Γ \/ ~ a_wl_red Γ).
-      { eapply IHnw; eauto; simpl; try lia. }
-      assert (JgInter1: forall A1 A2, A0 = typ_intersection A1 A2 ->
-          (work_sub A A2 ⫤ work_sub A A1 ⫤ Γ) ⟶ᵃʷ⁎⋅ \/ ¬ (work_sub A A2 ⫤ work_sub A A1 ⫤ Γ) ⟶ᵃʷ⁎⋅).
-      { intros A1 A2 Heq. subst. dependent destruction H3.
-        eapply IHnw with (m := ((3 * m + all_size A) * (1 + iu_size A2) + (3 * n2 + all_size A2) * (1 + iu_size A)) + ((3 * m + all_size A) * (1 + iu_size A1) + (3 * n1 + all_size A1) * (1 + iu_size A)) + n); eauto; try lia.
-        admit. (* safe: wf *)
-        assert (HspA: split_size (aworklist_conswork Γ (work_sub A A1)) A m) by admit.
-        assert (HspA2: split_size (aworklist_conswork Γ (work_sub A A1)) A2 n2) by admit.
-        eapply measp_wl_conswork with
-          (m := ((3 * m + all_size A) * (1 + iu_size A2) + (3 * n2 + all_size A2) * (1 + iu_size A)))
-          (n := ((3 * m + all_size A) * (1 + iu_size A1) + (3 * n1 + all_size A1) * (1 + iu_size A)) + n); eauto; try lia.
-        assert (Hle:
-          (3 * m + all_size A) * (1 + iu_size A2) +
-          (3 * n2 + all_size A2) * (1 + iu_size A) +
-          ((3 * m + all_size A) * (1 + iu_size A1) +
-          (3 * n1 + all_size A1) * (1 + iu_size A)) + n <=
-          (3 * m + all_size A) * (1 + iu_size (typ_intersection A1 A2)) +
-          (3 * S (n1 + n2) + all_size (typ_intersection A1 A2)) * (1 + iu_size A) + n).
-        { simpl. lia. }
-        lia. simpl in *. lia. }
-      assert (JgInter2: forall A1 A2, A = typ_intersection A1 A2 ->
-                a_wl_red (aworklist_conswork Γ (work_sub A1 A0)) \/
-              ~ a_wl_red (aworklist_conswork Γ (work_sub A1 A0))).
-      { intros A1 A2 Heq. subst. dependent destruction H1.
-        eapply IHnw; eauto; simpl in *; try lia.
-        admit. (* safe: wf *) }
-      assert (JgInter3: forall A1 A2, A = typ_intersection A1 A2 ->
-                a_wl_red (aworklist_conswork Γ (work_sub A2 A0)) \/
-              ~ a_wl_red (aworklist_conswork Γ (work_sub A2 A0))).
-      { intros A1 A2 Heq. subst. dependent destruction H1.
-        eapply IHnw; eauto; simpl in *; try lia.
-        admit. (* safe: wf *) }
-      assert (JgUnion1: forall A1 A2, A0 = typ_union A1 A2 ->
-                a_wl_red (aworklist_conswork Γ (work_sub A A1)) \/
-              ~ a_wl_red (aworklist_conswork Γ (work_sub A A1))).
-      { intros A1 A2 Heq. subst. dependent destruction H3.
-        eapply IHnw; eauto; simpl in *; try lia.
-        admit. (* safe: wf *) }
-      assert (JgUnion2: forall A1 A2, A0 = typ_union A1 A2 ->
-                a_wl_red (aworklist_conswork Γ (work_sub A A2)) \/
-              ~ a_wl_red (aworklist_conswork Γ (work_sub A A2))).
-      { intros A1 A2 Heq. subst. dependent destruction H3.
-        eapply IHnw; eauto; simpl in *; try lia.
-        admit. (* safe: wf *) }
-      assert (JgUnion3: forall A1 A2, A = typ_union A1 A2 ->
-                a_wl_red (aworklist_conswork (aworklist_conswork Γ (work_sub A1 A0)) (work_sub A2 A0)) \/
-              ~ a_wl_red (aworklist_conswork (aworklist_conswork Γ (work_sub A1 A0)) (work_sub A2 A0))).
-      { intros A1 A2 Heq. subst. dependent destruction H1.
-        eapply IHnw with (m := ((3 * n2 + all_size A2) * (1 + iu_size A0) + (3 * m0 + all_size A0) * (1 + iu_size A2)) +
-                                ((3 * n1 + all_size A1) * (1 + iu_size A0) + (3 * m0 + all_size A0) * (1 + iu_size A1)) + n); eauto; try lia.
-        admit. (* safe: wf *)
-        assert (HspA: split_size (aworklist_conswork Γ (work_sub A1 A0)) A0 m0) by admit.
-        assert (HspA2: split_size (aworklist_conswork Γ (work_sub A1 A0)) A2 n2) by admit.
-        eapply measp_wl_conswork with
-          (m := ((3 * n2 + all_size A2) * (1 + iu_size A0) + (3 * m0 + all_size A0) * (1 + iu_size A2)))
-          (n := ((3 * n1 + all_size A1) * (1 + iu_size A0) + (3 * m0 + all_size A0) * (1 + iu_size A1)) + n); eauto; try lia.
-        assert (Hle: (3 * n2 + all_size A2) * (1 + iu_size A0) +
-        (3 * m0 + all_size A0) * (1 + iu_size A2) +
-        ((3 * n1 + all_size A1) * (1 + iu_size A0) +
-        (3 * m0 + all_size A0) * (1 + iu_size A1)) + n <=
-        (3 * S (n1 + n2) + all_size (typ_union A1 A2)) * (1 + iu_size A0) +
-        (3 * m0 + all_size A0) * iu_size (typ_union A1 A2) + n).
-        { simpl. lia. }
-        lia. simpl in *. lia. }
-      assert (JgAlll: forall A1 X L, A = typ_all A1 ->
-                neq_all A0 ->
-                neq_intersection A0 ->
-                neq_union A0 ->
-                X \notin  L ->
-                a_wl_red (aworklist_conswork (aworklist_constvar Γ X abind_etvar_empty) (work_sub  ( open_typ_wrt_typ A1 (typ_var_f X) )  A0)) \/
-              ~ a_wl_red (aworklist_conswork (aworklist_constvar Γ X abind_etvar_empty) (work_sub  ( open_typ_wrt_typ A1 (typ_var_f X) )  A0))).
-      { intros A1 X L Heq HneqAll HneqInter HneqUnion Hnin. subst. dependent destruction H1.
-        assert (HspA: split_size (aworklist_constvar Γ X abind_etvar_empty) ( open_typ_wrt_typ A1 (typ_var_f X) ) n0) by admit.
-        assert (HspA0: split_size (aworklist_constvar Γ X abind_etvar_empty) A0 m0) by admit.
-        assert (Heq: iu_size (typ_all A1) = iu_size (A1 ᵗ^ₜ X)) by admit. (* safe *)
-        eapply IHnw with (m := (3 * n0 + all_size (A1 ᵗ^ₜ X)) * (1 + iu_size A0) +
-                                (3 * m0 + all_size A0) * (1 + iu_size (A1 ᵗ^ₜ X)) + S n); eauto; try lia.
-        admit. (* safe: wf *)
-        eapply measp_wl_conswork; eauto.
-        assert (Heq': all_size (typ_all A1) = all_size (A1 ᵗ^ₜ X) + 1) by admit. (* safe *)
-        rewrite Heq in Hlt. rewrite Heq' in Hlt. lia.
-        assert (Heq': weight (A1 ᵗ^ₜ X) = weight A1) by admit. (* safe *)
-        assert (Hgt: weight A0 >= 1) by apply weight_gt_0.
-        simpl in *. rewrite <- Heq. rewrite Heq'. lia. }
-      assert (JgInst1: forall (E:list typvar) (Γ1 Γ2:aworklist) (X:typvar),
-                A = typ_var_f X ->
-                binds X abind_etvar_empty (awl_to_aenv Γ) ->
-                a_mono_typ (awl_to_aenv Γ) A0 ->
-                aworklist_subst Γ X A0 E Γ1 Γ2 ->
-                a_wl_red (awl_app (subst_tvar_in_aworklist A0 X Γ2) (awl_app (etvar_list_to_awl E) Γ1)) \/
-                ~ a_wl_red (awl_app (subst_tvar_in_aworklist A0 X Γ2) (awl_app (etvar_list_to_awl E) Γ1))).
-      { intros E Γ1 Γ2 X Heq Hbin Hmono Hsub. subst.
-        eapply IHnw.
-        admit. (* safe: wf *)
-        - rewrite exp_size_wl_awl_app.
-          rewrite exp_size_wl_awl_app.
-          rewrite exp_size_wl_etvar_list.
-          erewrite exp_size_wl_subst_tvar_in_aworklist_mono; eauto. simpl.
-          eapply exp_size_wl_aworklist_subst in Hsub as Heq. lia.
-        - rewrite judge_size_wl_awl_app.
-          rewrite judge_size_wl_awl_app.
-          rewrite judge_size_wl_etvar_list.
-          erewrite judge_size_wl_subst_tvar_in_aworklist; eauto. simpl.
-          eapply judge_size_wl_aworklist_subst in Hsub as Heq. lia.
-        - admit.
-        - admit. 
-        - admit.
-        - admit.
-        - admit.
-        - admit.
-        - admit.
-      }
-      dependent destruction H.
-      * dependent destruction H0;
-          try solve [right; intro Hcontra;
-            dependent destruction Hcontra];
-          try solve [destruct Jg as [Jg | Jg]; eauto;
-            right; intro Hcontra; dependent destruction Hcontra;
-            eapply Jg; eauto].
-        -- right. intro Hcontra. dependent destruction Hcontra.
-           eapply abind_etvar_tvar_false; eauto.
-        -- right. intro Hcontra. dependent destruction Hcontra.
-            eapply abind_etvar_stvar_false; eauto.
-        -- admit. (* TODO *)
-        -- edestruct JgUnion1 as [JgUnion1' | JgUnion1']; eauto.
-           edestruct JgUnion2 as [JgUnion2' | JgUnion2']; eauto.
-           right. intro Hcontra. dependent destruction Hcontra.
-           eapply JgUnion1'; eauto. eapply JgUnion2'; eauto.
-        -- edestruct JgInter1 as [JgInter1' | JgInter1']; eauto.
-           right. intro Hcontra. dependent destruction Hcontra.
-           eapply JgInter1'; eauto.
-      * dependent destruction H0;
-          try solve [right; intro Hcontra;
-            dependent destruction Hcontra];
-          try solve [destruct Jg as [Jg | Jg]; eauto;
-            right; intro Hcontra; dependent destruction Hcontra;
-            eapply Jg; eauto];
-          destruct Jg as [Jg | Jg]; eauto;
-          try solve [right; intro Hcontra; dependent destruction Hcontra;
-            eapply Jg; eauto; dependent destruction H5].
-        -- edestruct JgUnion1 as [JgUnion1' | JgUnion1']; eauto.
-           edestruct JgUnion2 as [JgUnion2' | JgUnion2']; eauto.
-           right. intro Hcontra. dependent destruction Hcontra.
-           eapply Jg; eauto. eapply JgUnion1'; eauto. eapply JgUnion2'; eauto.
-        -- edestruct JgInter1 as [JgInter1' | JgInter1']; eauto.
-           right. intro Hcontra. dependent destruction Hcontra.
-           eapply Jg; eauto. eapply JgInter1'; eauto.
-      * dependent destruction H0;
-          try solve [right; intro Hcontra;
-            dependent destruction Hcontra];
-          try solve [destruct Jg as [Jg | Jg]; eauto;
-            right; intro Hcontra; dependent destruction Hcontra;
-            eapply Jg; eauto];
-          try solve [right; intro Hcontra; dependent destruction Hcontra;
-            dependent destruction H5].
-        -- edestruct JgUnion1 as [JgUnion1' | JgUnion1']; eauto.
-           edestruct JgUnion2 as [JgUnion2' | JgUnion2']; eauto.
-           right. intro Hcontra. dependent destruction Hcontra.
-           eapply JgUnion1'; eauto. eapply JgUnion2'; eauto.
-        -- edestruct JgInter1 as [JgInter1' | JgInter1']; eauto.
-           right. intro Hcontra. dependent destruction Hcontra.
-           eapply JgInter1'; eauto.
-      * admit. (* TODO *)
-      * admit. (* TODO *)
-      * admit. (* TODO *)
-      * dependent destruction H1;
-          try solve [right; intro Hcontra;
-            dependent destruction Hcontra];
-          try solve [destruct Jg as [Jg | Jg]; eauto;
-            right; intro Hcontra; dependent destruction Hcontra;
-            eapply Jg; eauto].
-        -- right. intro Hcontra. dependent destruction Hcontra.
-           eapply abind_etvar_tvar_false; eauto.
-           eapply abind_etvar_tvar_false; eauto.
-        -- right. intro Hcontra. dependent destruction Hcontra.
-           eapply abind_etvar_stvar_false; eauto.
-           eapply abind_etvar_stvar_false; eauto.
-        -- admit. (* TODO *)
-        -- assert (JgArr: a_wl_red (aworklist_conswork (aworklist_conswork Γ (work_sub A0 A1)) (work_sub A2 A3)) \/
-                        ~ a_wl_red (aworklist_conswork (aworklist_conswork Γ (work_sub A0 A1)) (work_sub A2 A3))).
-           { assert (Hle: forall ns1 ns2 ns0 ns3,
-                      split_size (aworklist_conswork Γ (work_sub A0 A1)) A2 ns2 ->
-                      split_size (aworklist_conswork Γ (work_sub A0 A1)) A3 ns3 ->
-                      split_size Γ A0 ns0 -> split_size Γ A1 ns1 ->
-                      ((3 * ns2 + all_size A2) * (1 + iu_size A3) +
-                      (3 * ns3 + all_size A3) * (1 + iu_size A2)) +
-                      ((3 * ns0 + all_size A0) * (1 + iu_size A1) +
-                      (3 * ns1 + all_size A1) * (1 + iu_size A0))
-                        <= n0 * (1 + iu_size (typ_arrow A0 A3)) + n1 * (1 + iu_size (typ_arrow A1 A2))).
-                    { intros ns1 ns2 ns0 ns3 Hns2 Hns3 Hns0 Hns1.
-                      rewrite H3. rewrite H5.
-                      assert (Hle': ns1 + ns2 <= m) by admit. (* CHECK THIS! *)
-                      assert (Hle'': ns0 + ns3 <= m0) by admit. (* CHECK THIS! *)
-                      eapply le_trans with (m := (3 * (ns1 + ns2) + all_size (typ_arrow A1 A2)) * (1 + iu_size (typ_arrow A0 A3))
-                                               + (3 * (ns0 + ns3) + all_size (typ_arrow A0 A3)) * (1 + iu_size (typ_arrow A1 A2))).
-                      simpl in *. lia. admit. (* safe: oh my lia. *) }
-            assert (Hs2: exists ns2, split_size (work_sub A0 A1 ⫤ Γ) A2 ns2) by admit.
-            assert (Hs3: exists ns3, split_size (work_sub A0 A1 ⫤ Γ) A3 ns3) by admit.
-            assert (Hs0: exists ns0, split_size Γ A0 ns0) by admit.
-            assert (Hs1: exists ns1, split_size Γ A1 ns1) by admit.
-            destruct Hs2 as [ns2 Hs2]. destruct Hs3 as [ns3 Hs3].
-            destruct Hs0 as [ns0 Hs0]. destruct Hs1 as [ns1 Hs1].
-            specialize (Hle ns1 ns2 ns0 ns3 Hs2 Hs3 Hs0 Hs1).
-            eapply IHnw with (m := ((3 * ns2 + all_size A2) * (1 + iu_size A3) +
-                                    (3 * ns3 + all_size A3) * (1 + iu_size A2)) +
-                                    ((3 * ns0 + all_size A0) * (1 + iu_size A1) +
-                                    (3 * ns1 + all_size A1) * (1 + iu_size A0)) + n); eauto.
-            eapply measp_wl_conswork with (n := ((3 * ns0 + all_size A0) * (1 + iu_size A1) +
-                                                    (3 * ns1 + all_size A1) * (1 + iu_size A0)) + n); eauto; try lia.
-            lia. simpl in *. lia. }
-            destruct JgArr as [JgArr | JgArr]; eauto.
+    * exfalso. apply H1. eauto.
+    * simpl in *. edestruct (apply_conts_dec cs A) as [[w Happly] | Happly].
+      -- eapply apply_conts_exp_size with (Γ := Γ) in Happly as Hes.
+         eapply apply_conts_judge_size in Happly as Hjs.
+         assert (JgApply: (w ⫤ᵃ Γ) ⟶ᵃʷ⁎⋅ \/ ¬ (w ⫤ᵃ Γ) ⟶ᵃʷ⁎⋅).
+         { eapply IHnj; simpl; eauto; try lia.
+           eapply a_wf_wl_apply_conts; eauto. }
+         destruct JgApply as [JgApply | JgApply]; eauto.
+         right. intro Hcontra. dependent destruction Hcontra.
+         eapply apply_conts_det in Happly; eauto. subst. eapply JgApply; eauto.
+      -- right; intro Hcontra; dependent destruction Hcontra;
+         eapply Happly; eauto.
+    * simpl in *. edestruct (apply_contd_dec cd A B) as [[w Happly] | Happly].
+      -- eapply apply_contd_exp_size with (Γ := Γ) in Happly as Hes.
+         eapply apply_contd_judge_size in Happly as Hjs.
+         assert (JgApply: (w ⫤ᵃ Γ) ⟶ᵃʷ⁎⋅ \/ ¬ (w ⫤ᵃ Γ) ⟶ᵃʷ⁎⋅).
+         { eapply IHnj; simpl; eauto; try lia.
+           eapply a_wf_wl_apply_contd; eauto. }
+         destruct JgApply as [JgApply | JgApply]; eauto.
+         right. intro Hcontra. dependent destruction Hcontra.
+         eapply apply_contd_det in Happly; eauto. subst. eapply JgApply; eauto.
+      -- right; intro Hcontra; dependent destruction Hcontra;
+         eapply Happly; eauto.
+  - simpl in *.
+    assert (Jg: a_wl_red Γ \/ ~ a_wl_red Γ).
+    { eapply IHnw; eauto. lia. }
+    destruct Jg as [Jg | Jg]; auto.
+    right. intro Hcontra.
+    dependent destruction Hcontra.
+    apply Jg; auto.
+  - simpl in *.
+    assert (Jg: a_wl_red Γ \/ ~ a_wl_red Γ).
+    { eapply IHnw; eauto. lia. }
+    destruct Jg as [Jg | Jg]; auto.
+    right. intro Hcontra.
+    dependent destruction Hcontra.
+    apply Jg; auto.
+  - simpl in *.
+    assert (HwA: weight A >= 1) by apply weight_gt_0.
+    assert (HwB: weight B >= 1) by apply weight_gt_0.
+    assert (Jg: Γ ⟶ᵃʷ⁎⋅ \/ ¬ Γ ⟶ᵃʷ⁎⋅).
+    { eapply IHnw; eauto; simpl; try lia. }
+    assert (JgInter1: forall A1 A2, B = typ_intersection A1 A2 ->
+        (work_sub A A2 ⫤ᵃ work_sub A A1 ⫤ᵃ Γ) ⟶ᵃʷ⁎⋅ \/ ¬ (work_sub A A2 ⫤ᵃ work_sub A A1 ⫤ᵃ Γ) ⟶ᵃʷ⁎⋅).
+    { intros A1 A2 Heq. subst.
+      eapply IHnw; eauto; simpl in *; unfold split_depth in *; simpl in *; try lia.
+      dependent destruction H0. apply a_wf_wl__conswork_sub; auto. }
+    assert (JgInter2: forall A1 A2, A = typ_intersection A1 A2 ->
+        (work_sub A1 B ⫤ᵃ Γ) ⟶ᵃʷ⁎⋅ \/ ¬ (work_sub A1 B ⫤ᵃ Γ) ⟶ᵃʷ⁎⋅).
+    { intros A1 A2 Heq. subst.
+      eapply IHnw; eauto; simpl in *; unfold split_depth in *; simpl in *; try lia.
+      dependent destruction H. apply a_wf_wl__conswork_sub; auto. }
+    assert (JgInter3: forall A1 A2, A = typ_intersection A1 A2 ->
+        (work_sub A2 B ⫤ᵃ Γ) ⟶ᵃʷ⁎⋅ \/ ¬ (work_sub A2 B ⫤ᵃ Γ) ⟶ᵃʷ⁎⋅).
+    { intros A1 A2 Heq. subst.
+      eapply IHnw; eauto; simpl in *; unfold split_depth in *; simpl in *; try lia.
+      dependent destruction H. apply a_wf_wl__conswork_sub; auto. }
+    assert (JgUnion1: forall A1 A2, B = typ_union A1 A2 ->
+        (work_sub A A1 ⫤ᵃ Γ) ⟶ᵃʷ⁎⋅ \/ ¬ (work_sub A A1 ⫤ᵃ Γ) ⟶ᵃʷ⁎⋅).
+    { intros A1 A2 Heq. subst.
+      eapply IHnw; eauto; simpl in *; unfold split_depth in *; simpl in *; try lia.
+      dependent destruction H0. apply a_wf_wl__conswork_sub; auto. }
+    assert (JgUnion2: forall A1 A2, B = typ_union A1 A2 ->
+        (work_sub A A2 ⫤ᵃ Γ) ⟶ᵃʷ⁎⋅ \/ ¬ (work_sub A A2 ⫤ᵃ Γ) ⟶ᵃʷ⁎⋅).
+    { intros A1 A2 Heq. subst.
+      eapply IHnw; eauto; simpl in *; unfold split_depth in *; simpl in *; try lia.
+      dependent destruction H0. apply a_wf_wl__conswork_sub; auto. }
+    assert (JgUnion3: forall A1 A2, A = typ_union A1 A2 ->
+        (work_sub A2 B ⫤ᵃ work_sub A1 B ⫤ᵃ Γ) ⟶ᵃʷ⁎⋅ \/ ¬ (work_sub A2 B ⫤ᵃ work_sub A1 B ⫤ᵃ Γ) ⟶ᵃʷ⁎⋅).
+    { intros A1 A2 Heq. subst.
+      eapply IHnw; eauto; simpl in *; unfold split_depth in *; simpl in *; try lia.
+      dependent destruction H. apply a_wf_wl__conswork_sub; auto. }
+    assert (JgAlll: forall A1 X L, A = typ_all A1 ->
+              neq_all B ->
+              neq_intersection B ->
+              neq_union B ->
+              X \notin  L `union` (dom (⌊ Γ ⌋ᵃ)) ->
+              (work_sub (A1 ᵗ^ₜ X) B ⫤ᵃ X ~ᵃ ⬒ ;ᵃ Γ) ⟶ᵃʷ⁎⋅ \/
+            ¬ (work_sub (A1 ᵗ^ₜ X) B ⫤ᵃ X ~ᵃ ⬒ ;ᵃ Γ) ⟶ᵃʷ⁎⋅).
+    { intros A1 X L Heq HneqAll HneqInter HneqUnion Hnin. subst.
+      eapply IHnm; eauto; simpl in *; try lia.
+      apply a_wf_wl__conswork_sub; auto.
+      apply a_wf_typ_all_open; auto.
+      apply a_wf_typ_weaken_cons; auto. simpl. auto.
+      apply a_wf_typ_weaken_cons; auto.
+      assert (HspA1: split_depth ((X, ⬒) :: ⌊ Γ ⌋ᵃ) (A1 ᵗ^ₜ X) <= split_depth (⌊ Γ ⌋ᵃ) A1) by admit.
+      assert (HspB: split_depth ((X, ⬒) :: ⌊ Γ ⌋ᵃ) B <= split_depth (⌊ Γ ⌋ᵃ) B) by admit.
+      eapply mult_le_compat_r with (p := S (iu_size B)) in HspA1.
+      eapply mult_le_compat_r with (p := S (iu_size A1)) in HspB.
+      assert (Heq: iu_size A1 = iu_size (A1 ᵗ^ₜ X)) by admit. (* safe *)
+      rewrite <- Heq.
+      simpl in *. unfold split_depth in *. simpl in *.
+      admit. (* oh my lia *) }
+    assert (JgInst1: forall (Γ1 Γ2:aworklist) (X:typvar),
+              A = typ_var_f X ->
+              binds X abind_etvar_empty (awl_to_aenv Γ) ->
+              a_mono_typ (awl_to_aenv Γ) B ->
+              aworklist_subst Γ X B Γ1 Γ2 ->
+              (subst_tvar_in_aworklist B X Γ2 ⧺ Γ1) ⟶ᵃʷ⁎⋅ \/
+            ~ (subst_tvar_in_aworklist B X Γ2 ⧺ Γ1) ⟶ᵃʷ⁎⋅).
+    { intros Γ1 Γ2 X Heq Hbin Hmono Hsub. subst.
+      eapply IHnw; eauto; simpl in *; try lia.
+      admit.
+      (* admit. (* safe: wf *)
+      admit. (* erewrite exp_size_wl_aworklist_subst; eauto. *)
+      admit. (* TODO: should be fine *)
+      admit. (* TODO: should be fine *)
+      admit. (* TODO: should be fine *)
+      admit. (* TODO: should be fine *)
+      admit. (* TODO: should be fine *)
+      eapply aworklist_binds_split in Hbin as Hbin'; eauto.
+      destruct Hbin' as [Γ1' [Γ2' Hbin']]. subst.
+      erewrite split_depth_wl_aworklist_subst; eauto. lia. admit.
+      admit. TODO: should be fine *)
+    } 
+    assert (JgInst2: forall (Γ1 Γ2:aworklist) (X:typvar),
+              B = typ_var_f X ->
+              binds X abind_etvar_empty (awl_to_aenv Γ) ->
+              a_mono_typ (awl_to_aenv Γ) A ->
+              aworklist_subst Γ X A Γ1 Γ2 ->
+              (subst_tvar_in_aworklist A X Γ2 ⧺ Γ1) ⟶ᵃʷ⁎⋅ \/
+            ~ (subst_tvar_in_aworklist A X Γ2 ⧺ Γ1) ⟶ᵃʷ⁎⋅) by admit.
+    (* { intros E Γ1 Γ2 X Heq Hbin Hmono Hsub. subst.
+      eapply IHnw.
+      admit. (* safe: wf *)
+      - rewrite exp_size_wl_awl_app.
+        rewrite exp_size_wl_awl_app.
+        rewrite exp_size_wl_etvar_list.
+        erewrite exp_size_wl_subst_tvar_in_aworklist_mono; eauto. simpl.
+        eapply exp_size_wl_aworklist_subst in Hsub as Heq. lia.
+      - rewrite judge_size_wl_awl_app.
+        rewrite judge_size_wl_awl_app.
+        rewrite judge_size_wl_etvar_list.
+        erewrite judge_size_wl_subst_tvar_in_aworklist; eauto. simpl.
+        eapply judge_size_wl_aworklist_subst in Hsub as Heq. lia.
+      - admit.
+      - admit. 
+      - admit.
+      - admit.
+      - admit.
+      - admit.
+      - admit.
+    } *)
+    dependent destruction H.
+    * dependent destruction H0;
+        try solve [right; intro Hcontra;
+          dependent destruction Hcontra];
+        try solve [destruct Jg as [Jg | Jg]; eauto;
+          right; intro Hcontra; dependent destruction Hcontra;
+          eapply Jg; eauto].
+      -- right. intro Hcontra. dependent destruction Hcontra. unify_binds.
+      -- right. intro Hcontra. dependent destruction Hcontra. unify_binds.
+      -- destruct (a_wf_wl_aworklist_subst_dec Γ X typ_unit) as [[Γ1 [Γ2 Hsubst]] | Hsubst]; eauto.
+         ++ edestruct JgInst2 as [JgInst2' | JgInst2']; eauto.
             right. intro Hcontra. dependent destruction Hcontra.
-            apply JgArr; auto.
-        -- edestruct JgUnion1 as [JgUnion1' | JgUnion1']; eauto.
-           edestruct JgUnion2 as [JgUnion2' | JgUnion2']; eauto.
-           right. intro Hcontra. dependent destruction Hcontra.
-           eapply JgUnion1'; eauto. eapply JgUnion2'; eauto.
-        -- edestruct JgInter1 as [JgInter1' | JgInter1']; eauto.
-           right. intro Hcontra. dependent destruction Hcontra.
-           eapply JgInter1'; eauto.
-      * dependent destruction H1.
-        (* can use some tatics, while have to solve the binding problem first*) 
-        -- pick fresh X. inst_cofinites_with X.
-           edestruct JgAlll as [JgAlll' | JgAlll']; eauto.
-           ++ left. inst_cofinites_for a_wl_red__sub_alll; eauto.
-              intros X' Hnin.
-              apply a_wl_red_rename_tvar with (X:=X) (X':=X') in JgAlll'.
-              ** simpl in JgAlll'.
-                 unfold eq_dec in JgAlll'.
-                 destruct (EqDec_eq_of_X X X) in JgAlll'.
-                 --- rewrite rename_tvar_in_aworklist_fresh_eq in JgAlll'; auto.
-                     rewrite subst_tvar_in_typ_open_typ_wrt_typ_tvar2 in JgAlll'; auto.
-                 --- contradiction.
-              ** admit.
-              ** admit. (* wf *)
-              ** simpl. rewrite ftvar_in_typ_open_typ_wrt_typ_upper. auto.
-           ++ right. intro Hcontra. dependent destruction Hcontra.
-              pick fresh X1.
-              inst_cofinites_with X1.
-              apply a_wl_red_rename_tvar with (X:=X1) (X':=X) in H8; auto.
-              ** simpl in H8.
-                 unfold eq_dec in H8.
-                 destruct (EqDec_eq_of_X X1 X1) in H8.
-                 --- rewrite rename_tvar_in_aworklist_fresh_eq in H8; auto.
-                     rewrite subst_tvar_in_typ_open_typ_wrt_typ_tvar2 in H8; auto.
-                 --- contradiction.
-              ** admit. (* wf *)  
-              ** simpl. rewrite ftvar_in_typ_open_typ_wrt_typ_upper. auto.
-        -- pick fresh X. inst_cofinites_with X.
-           edestruct JgAlll as [JgAlll' | JgAlll']; eauto.
-           ++ left. inst_cofinites_for a_wl_red__sub_alll; eauto.
-              intros X' Hnin.
-              apply a_wl_red_rename_tvar with (X:=X) (X':=X') in JgAlll'.
-              ** simpl in JgAlll'.
-                 unfold eq_dec in JgAlll'.
-                 destruct (EqDec_eq_of_X X X) in JgAlll'.
-                 --- rewrite rename_tvar_in_aworklist_fresh_eq in JgAlll'; auto.
-                     rewrite subst_tvar_in_typ_open_typ_wrt_typ_tvar2 in JgAlll'; auto.
-                 --- contradiction.
-              ** admit.
-              ** admit. (* wf *)
-              ** simpl. rewrite ftvar_in_typ_open_typ_wrt_typ_upper. auto.
-           ++ right. intro Hcontra. dependent destruction Hcontra.
-              pick fresh X1.
-              inst_cofinites_with X1.
-              apply a_wl_red_rename_tvar with (X:=X1) (X':=X) in H8; auto.
-              ** simpl in H8.
-                 unfold eq_dec in H8.
-                 destruct (EqDec_eq_of_X X1 X1) in H8.
-                 --- rewrite rename_tvar_in_aworklist_fresh_eq in H8; auto.
-                     rewrite subst_tvar_in_typ_open_typ_wrt_typ_tvar2 in H8; auto.
-                 --- contradiction.
-              ** admit. (* wf *)  
-              ** simpl. rewrite ftvar_in_typ_open_typ_wrt_typ_upper. auto.
-        -- destruct Jg as [Jg | Jg]; eauto.
-           pick fresh X. inst_cofinites_with X.
-           edestruct JgAlll as [JgAlll' | JgAlll']; eauto.
-           ++ left. inst_cofinites_for a_wl_red__sub_alll; eauto.
-              intros X' Hnin.
-              apply a_wl_red_rename_tvar with (X:=X) (X':=X') in JgAlll'.
-              ** simpl in JgAlll'.
-                 unfold eq_dec in JgAlll'.
-                 destruct (EqDec_eq_of_X X X) in JgAlll'.
-                 --- rewrite rename_tvar_in_aworklist_fresh_eq in JgAlll'; auto.
-                     rewrite subst_tvar_in_typ_open_typ_wrt_typ_tvar2 in JgAlll'; auto.
-                 --- contradiction.
-              ** admit.
-              ** admit. (* wf *)
-              ** simpl. rewrite ftvar_in_typ_open_typ_wrt_typ_upper. auto.
-           ++ right. intro Hcontra. dependent destruction Hcontra; eauto.
-              pick fresh X1.
-              inst_cofinites_with X1.
-              apply a_wl_red_rename_tvar with (X:=X1) (X':=X) in H8; auto.
-              ** simpl in H8.
-                 unfold eq_dec in H8.
-                 destruct (EqDec_eq_of_X X1 X1) in H8.
-                 --- rewrite rename_tvar_in_aworklist_fresh_eq in H8; auto.
-                     rewrite subst_tvar_in_typ_open_typ_wrt_typ_tvar2 in H8; auto.
-                 --- contradiction.
-              ** admit. (* wf *)  
-              ** simpl. rewrite ftvar_in_typ_open_typ_wrt_typ_upper. auto.
-        -- pick fresh X1. inst_cofinites_with X1.
-           edestruct JgAlll as [JgAlll' | JgAlll']; eauto.
-           ++ left. inst_cofinites_for a_wl_red__sub_alll; eauto.
-              intros X' Hnin.
-              apply a_wl_red_rename_tvar with (X:=X1) (X':=X') in JgAlll'.
-              ** simpl in JgAlll'.
-                 destruct_eq_atom.
-                 rewrite rename_tvar_in_aworklist_fresh_eq in JgAlll'; auto.
-                 rewrite subst_tvar_in_typ_open_typ_wrt_typ_tvar2 in JgAlll'; auto.
-              ** admit.
-              ** admit. (* wf *)
-              ** simpl. rewrite ftvar_in_typ_open_typ_wrt_typ_upper. auto.
-           ++ right. intro Hcontra. dependent destruction Hcontra; try solve [dependent destruction H7].
-              pick fresh X1'.
-              inst_cofinites_with X1'.
-              apply a_wl_red_rename_tvar with (X:=X1') (X':=X1) in H9; auto.
-              ** simpl in H9.
-                 destruct_eq_atom.
-                 rewrite rename_tvar_in_aworklist_fresh_eq in H9; auto.
-                 rewrite subst_tvar_in_typ_open_typ_wrt_typ_tvar2 in H9; auto.
-              ** admit. (* wf *)  
-              ** simpl. rewrite ftvar_in_typ_open_typ_wrt_typ_upper. auto.
-        -- pick fresh X1. inst_cofinites_with X1.
-           edestruct JgAlll as [JgAlll' | JgAlll']; eauto.
-           ++ left. inst_cofinites_for a_wl_red__sub_alll; eauto.
-              intros X' Hnin.
-              apply a_wl_red_rename_tvar with (X:=X1) (X':=X') in JgAlll'.
-              ** simpl in JgAlll'.
-                 destruct_eq_atom.
-                 rewrite rename_tvar_in_aworklist_fresh_eq in JgAlll'; auto.
-                 rewrite subst_tvar_in_typ_open_typ_wrt_typ_tvar2 in JgAlll'; auto.
-              ** admit.
-              ** admit. (* wf *)
-              ** simpl. rewrite ftvar_in_typ_open_typ_wrt_typ_upper. auto.
-           ++ right. intro Hcontra. dependent destruction Hcontra; try solve [dependent destruction H7].
-              pick fresh X1'.
-              inst_cofinites_with X1'.
-              apply a_wl_red_rename_tvar with (X:=X1') (X':=X1) in H9; auto.
-              ** simpl in H9.
-                 destruct_eq_atom.
-                 rewrite rename_tvar_in_aworklist_fresh_eq in H9; auto.
-                 rewrite subst_tvar_in_typ_open_typ_wrt_typ_tvar2 in H9; auto.
-              ** admit. (* wf *)  
-              ** simpl. rewrite ftvar_in_typ_open_typ_wrt_typ_upper. auto.
-        -- pick fresh X1. inst_cofinites_with X1.
-           edestruct JgAlll as [JgAlll' | JgAlll']; eauto.
-           ++ left. inst_cofinites_for a_wl_red__sub_alll; eauto.
-              intros X' Hnin.
-              apply a_wl_red_rename_tvar with (X:=X1) (X':=X') in JgAlll'.
-              ** simpl in JgAlll'.
-                 destruct_eq_atom.
-                 rewrite rename_tvar_in_aworklist_fresh_eq in JgAlll'; auto.
-                 rewrite subst_tvar_in_typ_open_typ_wrt_typ_tvar2 in JgAlll'; auto.
-              ** admit.
-              ** admit. (* wf *)
-              ** simpl. rewrite ftvar_in_typ_open_typ_wrt_typ_upper. auto.
-           ++ right. intro Hcontra. dependent destruction Hcontra; try solve [dependent destruction H7].
-              pick fresh X1'.
-              inst_cofinites_with X1'.
-              apply a_wl_red_rename_tvar with (X:=X1') (X':=X1) in H9; auto.
-              ** simpl in H9.
-                 destruct_eq_atom.
-                 rewrite rename_tvar_in_aworklist_fresh_eq in H9; auto.
-                 rewrite subst_tvar_in_typ_open_typ_wrt_typ_tvar2 in H9; auto.
-              ** admit. (* wf *)  
-              ** simpl. rewrite ftvar_in_typ_open_typ_wrt_typ_upper. auto.
-        -- pick fresh X. inst_cofinites_with X.
-           edestruct JgAlll as [JgAlll' | JgAlll']; eauto.
-           admit. admit. admit. (* safe *) 
-           ++ left. inst_cofinites_for a_wl_red__sub_alll; eauto.
-              admit. admit. admit. (* safe *) 
-              intros X' Hnin.
-              apply a_wl_red_rename_tvar with (X:=X) (X':=X') in JgAlll'.
-              ** simpl in JgAlll'.
-                 unfold eq_dec in JgAlll'.
-                 destruct (EqDec_eq_of_X X X) in JgAlll'.
-                 --- rewrite rename_tvar_in_aworklist_fresh_eq in JgAlll'; auto.
-                     rewrite subst_tvar_in_typ_open_typ_wrt_typ_tvar2 in JgAlll'; auto.
-                     rewrite subst_tvar_in_typ_fresh_eq in JgAlll'; auto.
-                     rewrite subst_tvar_in_typ_fresh_eq in JgAlll'; auto.
-                 --- contradiction.
-              ** admit.
-              ** admit. (* wf *)
-              ** simpl. rewrite ftvar_in_typ_open_typ_wrt_typ_upper. auto.
-           ++ right. intro Hcontra. dependent destruction Hcontra; eauto.
-              pick fresh X1.
-              inst_cofinites_with X1.
-              apply a_wl_red_rename_tvar with (X:=X1) (X':=X) in H8; auto.
-              ** simpl in H8.
-                 unfold eq_dec in H8.
-                 destruct (EqDec_eq_of_X X1 X1) in H8.
-                 --- rewrite rename_tvar_in_aworklist_fresh_eq in H8; auto.
-                     rewrite subst_tvar_in_typ_open_typ_wrt_typ_tvar2 in H8; auto.
-                     rewrite subst_tvar_in_typ_fresh_eq in H8; auto.
-                     rewrite subst_tvar_in_typ_fresh_eq in H8; auto.
-                 --- contradiction.
-              ** admit. (* wf *)  
-              ** simpl. rewrite ftvar_in_typ_open_typ_wrt_typ_upper. auto.
-        -- dependent destruction H3. dependent destruction H5.
-           pick fresh X. inst_cofinites_with X.
-           assert (Heq: all_size A = all_size (A ᵗ^ₜ X)) by admit. (* safe *)
-           assert (Heq0: all_size A0 = all_size (A0 ᵗ^ₜ X)) by admit. (* safe *)
-           assert (Heq': iu_size A = iu_size (A ᵗ^ₜ X)) by admit. (* safe *)
-           assert (Heq0': iu_size A0 = iu_size (A0 ᵗ^ₜ X)) by admit. (* safe *)
-           assert (Heq'': weight A = weight (A ᵗ^ₜ X)) by admit. (* safe *)
-           assert (Heq0'': weight A0 = weight (A0 ᵗ^ₜ X)) by admit. (* safe *)
-           assert (JgAll: a_wl_red (aworklist_conswork (aworklist_constvar Γ X abind_stvar_empty) (work_sub  ( open_typ_wrt_typ A (typ_var_f X) )   ( open_typ_wrt_typ A0 (typ_var_f X) ) )) \/
-                        ~ a_wl_red (aworklist_conswork (aworklist_constvar Γ X abind_stvar_empty) (work_sub  ( open_typ_wrt_typ A (typ_var_f X) )   ( open_typ_wrt_typ A0 (typ_var_f X) ) ))).
-           { eapply IHnw with (m := (3 * n1 + all_size (A ᵗ^ₜ X)) * iu_size (A0 ᵗ^ₜ X) + (3 * n3 + all_size (A0 ᵗ^ₜ X)) * iu_size (A ᵗ^ₜ X) + n); eauto; simpl in *; try lia.
-             admit. (* safe: wf *)
-             eapply measp_wl_conswork; eauto; try lia. 
-             admit.
-             }
-           destruct JgAll as [JgAll | JgAll]; eauto.
-           ++ left. inst_cofinites_for a_wl_red__sub_all; eauto.
-              intros X' Hnin. 
-              apply a_wl_red_rename_tvar with (X:=X) (X':=X') in JgAll.
-              ** simpl in JgAll.
-                 unfold eq_dec in JgAll.
-                 destruct (EqDec_eq_of_X X X) in JgAll.
-                 --- rewrite rename_tvar_in_aworklist_fresh_eq in JgAll; auto.
-                     rewrite subst_tvar_in_typ_open_typ_wrt_typ_tvar2 in JgAll; auto.
-                     rewrite subst_tvar_in_typ_open_typ_wrt_typ_tvar2 in JgAll; auto.
-                 --- contradiction.
-              ** admit.
-              ** admit. (* wf *)
-              ** simpl.
-                 rewrite ftvar_in_typ_open_typ_wrt_typ_upper.
-                 rewrite ftvar_in_typ_open_typ_wrt_typ_upper. auto.
-           ++ right. intro Hcontra. dependent destruction Hcontra; try solve [dependent destruction H7].
-              pick fresh X1.
-              inst_cofinites_with X1.
-              apply a_wl_red_rename_tvar with (X:=X1) (X':=X) in H7; auto.
-              ** simpl in H7.
-                 unfold eq_dec in H7.
-                 destruct (EqDec_eq_of_X X1 X1) in H7.
-                 --- rewrite rename_tvar_in_aworklist_fresh_eq in H7; auto.
-                     rewrite subst_tvar_in_typ_open_typ_wrt_typ_tvar2 in H7; auto.
-                     rewrite subst_tvar_in_typ_open_typ_wrt_typ_tvar2 in H7; auto.
-                 --- contradiction.
-              ** admit. (* wf *)  
-              ** simpl. rewrite ftvar_in_typ_open_typ_wrt_typ_upper.
-                 rewrite ftvar_in_typ_open_typ_wrt_typ_upper. auto.
-        -- edestruct JgUnion1 as [JgUnion1' | JgUnion1']; eauto.
-           edestruct JgUnion2 as [JgUnion2' | JgUnion2']; eauto.
-           right. intro Hcontra. dependent destruction Hcontra.
-           ++ dependent destruction H7.
-           ++ eapply JgUnion1'; eauto.
-           ++ eapply JgUnion2'; eauto.
-        -- edestruct JgInter1 as [JgInter1' | JgInter1']; eauto.
-           right. intro Hcontra. dependent destruction Hcontra.
-           ++ dependent destruction H6.
-           ++ eapply JgInter1'; eauto.
-    * dependent destruction H1;
-        try solve [edestruct JgUnion3 as [JgUnion3' | JgUnion3']; eauto;
-                   right; intro Hcontra; dependent destruction Hcontra;
-                   eapply JgUnion3'; eauto; try dependent destruction H7].
-      -- edestruct JgUnion1 as [JgUnion1' | JgUnion1']; eauto.
-         edestruct JgUnion2 as [JgUnion2' | JgUnion2']; eauto.
-         edestruct JgUnion3 as [JgUnion3' | JgUnion3']; eauto.
-         right. intro Hcontra. dependent destruction Hcontra.
-         eapply JgUnion1'; eauto. eapply JgUnion2'; eauto. eapply JgUnion3'; eauto.
-      -- edestruct JgInter1 as [JgInter1' | JgInter1']; eauto.
-         edestruct JgUnion3 as [JgUnion3' | JgUnion3']; eauto.
-         right. intro Hcontra. dependent destruction Hcontra.
-         eapply JgInter1'; eauto. eapply JgUnion3'; eauto.
-    * dependent destruction H1;
-        edestruct JgInter2 as [JgInter2' | JgInter2']; eauto;
-        edestruct JgInter3 as [JgInter3' | JgInter3']; eauto;
-        try solve [right; intro Hcontra; dependent destruction Hcontra;
-          try solve [eapply JgInter2'; eauto]; try solve [eapply JgInter3'; eauto];
-          dependent destruction H7].
+            assert (Heq: Γ1 = Γ3 /\ Γ2 = Γ4).
+            { eapply aworklist_subst_det; eauto. }
+            destruct Heq as [Heq1 Heq2]. subst. eauto.
+         ++ right. intro Hcontra. dependent destruction Hcontra.
+            eapply Hsubst; eauto.
       -- edestruct JgUnion1 as [JgUnion1' | JgUnion1']; eauto.
          edestruct JgUnion2 as [JgUnion2' | JgUnion2']; eauto.
          right. intro Hcontra. dependent destruction Hcontra.
-         eapply JgInter2'; eauto. eapply JgInter3'; eauto.
          eapply JgUnion1'; eauto. eapply JgUnion2'; eauto.
       -- edestruct JgInter1 as [JgInter1' | JgInter1']; eauto.
          right. intro Hcontra. dependent destruction Hcontra.
-         eapply JgInter1'; eauto. eapply JgInter2'; eauto. eapply JgInter3'; eauto.
-  + simpl in *.
-    edestruct (apply_cont_dec c A) as [[w Happly] | Happly].
-    * eapply apply_cont_exp_size in Happly as Hes.
-      eapply apply_cont_judge_size in Happly as Hjs.
-      destruct (measp_wl_total (aworklist_conswork aW w)) as [m' Hms].
-      eapply a_wf_wl_apply_cont; eauto.
-      assert (JgApply: a_wl_red (aworklist_conswork aW w) \/
-                     ~ a_wl_red (aworklist_conswork aW w)).
-      { eapply IHnj with (m := m'); simpl; eauto; try lia.
-        eapply a_wf_wl_apply_cont; eauto. }
-      destruct JgApply as [JgApply | JgApply]; eauto.
-      right. intro Hcontra. dependent destruction Hcontra.
-      eapply apply_cont_det in Happly; eauto. subst. eapply JgApply; eauto.
+         eapply JgInter1'; eauto.
+    * dependent destruction H0;
+        try solve [right; intro Hcontra;
+          dependent destruction Hcontra];
+        try solve [destruct Jg as [Jg | Jg]; eauto;
+          right; intro Hcontra; dependent destruction Hcontra;
+          eapply Jg; eauto];
+        destruct Jg as [Jg | Jg]; eauto;
+        try solve [right; intro Hcontra; dependent destruction Hcontra;
+          eapply Jg; eauto; dependent destruction H1].
+      -- edestruct JgUnion1 as [JgUnion1' | JgUnion1']; eauto.
+         edestruct JgUnion2 as [JgUnion2' | JgUnion2']; eauto.
+         right. intro Hcontra. dependent destruction Hcontra.
+         eapply Jg; eauto. eapply JgUnion1'; eauto. eapply JgUnion2'; eauto.
+      -- edestruct JgInter1 as [JgInter1' | JgInter1']; eauto.
+         right. intro Hcontra. dependent destruction Hcontra.
+         eapply Jg; eauto. eapply JgInter1'; eauto.
+    * dependent destruction H0;
+        try solve [right; intro Hcontra;
+          dependent destruction Hcontra];
+        try solve [destruct Jg as [Jg | Jg]; eauto;
+          right; intro Hcontra; dependent destruction Hcontra;
+          eapply Jg; eauto];
+        try solve [right; intro Hcontra; dependent destruction Hcontra;
+          dependent destruction H1].
+      -- edestruct JgUnion1 as [JgUnion1' | JgUnion1']; eauto.
+         edestruct JgUnion2 as [JgUnion2' | JgUnion2']; eauto.
+         right. intro Hcontra. dependent destruction Hcontra.
+         eapply JgUnion1'; eauto. eapply JgUnion2'; eauto.
+      -- edestruct JgInter1 as [JgInter1' | JgInter1']; eauto.
+         right. intro Hcontra. dependent destruction Hcontra.
+         eapply JgInter1'; eauto.
+    * dependent destruction H0; try unify_binds;
+        try solve [destruct Jg as [Jg | Jg]; eauto;
+          right; intro Hcontra; dependent destruction Hcontra; try unify_binds;
+          eapply Jg; eauto].
+      -- destruct (eq_dec X X0) as [Heq | Hneq]; subst.
+         ++ destruct Jg as [Jg | Jg]; eauto.
+            right; intro Hcontra; dependent destruction Hcontra; try unify_binds.
+         ++ right. intro Hcontra. dependent destruction Hcontra; try unify_binds.
+      -- destruct (eq_dec X X0) as [Heq | Hneq]; subst; try unify_binds. 
+         destruct (a_wf_wl_aworklist_subst_dec Γ X0 (` X)) as [[Γ1 [Γ2 Hsubst]] | Hsubst]; eauto.
+         ++ edestruct JgInst2 as [JgInst2' | JgInst2']; eauto.
+            right. intro Hcontra. dependent destruction Hcontra; try unify_binds.
+            assert (Heq: Γ1 = Γ3 /\ Γ2 = Γ4).
+            { eapply aworklist_subst_det; eauto. }
+            destruct Heq as [Heq1 Heq2]. subst. eauto.
+         ++ right. intro Hcontra. dependent destruction Hcontra; try unify_binds.
+      -- edestruct JgUnion1 as [JgUnion1' | JgUnion1']; eauto.
+         edestruct JgUnion2 as [JgUnion2' | JgUnion2']; eauto.
+         right. intro Hcontra. dependent destruction Hcontra; try unify_binds.
+         eapply JgUnion1'; eauto. eapply JgUnion2'; eauto.
+      -- edestruct JgInter1 as [JgInter1' | JgInter1']; eauto.
+         right. intro Hcontra. dependent destruction Hcontra; try unify_binds.
+         eapply JgInter1'; eauto.
+    * dependent destruction H0; try unify_binds;
+        try solve [destruct Jg as [Jg | Jg]; eauto;
+          right; intro Hcontra; dependent destruction Hcontra; try unify_binds;
+          eapply Jg; eauto].
+      -- destruct (eq_dec X X0) as [Heq | Hneq]; subst.
+         ++ destruct Jg as [Jg | Jg]; eauto.
+            right; intro Hcontra; dependent destruction Hcontra; try unify_binds.
+         ++ right. intro Hcontra. dependent destruction Hcontra; try unify_binds.
+      -- right. intro Hcontra. dependent destruction Hcontra; try unify_binds.
+         dependent destruction H2; try unify_binds.
+      -- edestruct JgUnion1 as [JgUnion1' | JgUnion1']; eauto.
+         edestruct JgUnion2 as [JgUnion2' | JgUnion2']; eauto.
+         right. intro Hcontra. dependent destruction Hcontra; try unify_binds.
+         eapply JgUnion1'; eauto. eapply JgUnion2'; eauto.
+      -- edestruct JgInter1 as [JgInter1' | JgInter1']; eauto.
+         right. intro Hcontra. dependent destruction Hcontra; try unify_binds. eauto.
+    * dependent destruction H0.
+      -- destruct (a_wf_wl_aworklist_subst_dec Γ X typ_unit) as [[Γ1 [Γ2 Hsubst]] | Hsubst]; eauto.
+          ++ edestruct JgInst1 as [JgInst1' | JgInst1']; eauto.
+            right. intro Hcontra. dependent destruction Hcontra; try unify_binds.
+            assert (Heq: Γ1 = Γ3 /\ Γ2 = Γ4).
+            { eapply aworklist_subst_det; eauto. }
+            destruct Heq as [Heq1 Heq2]. subst. eauto.
+          ++ right. intro Hcontra. dependent destruction Hcontra; try unify_binds.
+      -- right; intro Hcontra; dependent destruction Hcontra; try unify_binds.
+         dependent destruction H1.
+      -- destruct Jg as [Jg | Jg]; eauto.
+         right; intro Hcontra; dependent destruction Hcontra; try unify_binds; eauto.
+         dependent destruction H1.
+      -- destruct (eq_dec X X0) as [Heq | Hneq]; subst; try unify_binds. 
+         destruct (a_wf_wl_aworklist_subst_dec Γ X (` X0)) as [[Γ1 [Γ2 Hsubst]] | Hsubst]; eauto.
+         ++ edestruct JgInst1 as [JgInst1' | JgInst1']; eauto.
+            right. intro Hcontra. dependent destruction Hcontra; try unify_binds.
+            assert (Heq: Γ1 = Γ3 /\ Γ2 = Γ4).
+            { eapply aworklist_subst_det; eauto. }
+            destruct Heq as [Heq1 Heq2]. subst. eauto.
+         ++ right. intro Hcontra. dependent destruction Hcontra; try unify_binds.
+      -- right. intro Hcontra. dependent destruction Hcontra; try unify_binds.
+         dependent destruction H2; try unify_binds.
+      -- destruct (eq_dec X X0) as [Heq | Hneq]; subst; try unify_binds.
+         ++ destruct Jg as [Jg | Jg]; eauto.
+            right; intro Hcontra; dependent destruction Hcontra;
+              try unify_binds; simpl in *; eauto.
+         ++ destruct (a_wf_wl_aworklist_subst_dec Γ X (` X0)) as [[Γ1 [Γ2 Hsubst]] | Hsubst]; eauto.
+            ** edestruct JgInst1 as [JgInst1' | JgInst1']; eauto.
+               destruct (a_wf_wl_aworklist_subst_dec Γ X0 (` X)) as [[Γ1' [Γ2' Hsubst']] | Hsubst']; eauto.
+               --- edestruct JgInst2 as [JgInst2' | JgInst2']; eauto.
+                   right. intro Hcontra. dependent destruction Hcontra; try unify_binds.
+                   +++ assert (Heq: Γ1' = Γ3 /\ Γ2' = Γ4).
+                       { eapply aworklist_subst_det; eauto. }
+                       destruct Heq as [Heq1 Heq2]. subst. eauto.
+                   +++ assert (Heq: Γ1 = Γ3 /\ Γ2 = Γ4).
+                       { eapply aworklist_subst_det; eauto. }
+                       destruct Heq as [Heq1 Heq2]. subst. eauto.
+               --- right. intro Hcontra. dependent destruction Hcontra; try unify_binds.
+                   assert (Heq: Γ1 = Γ3 /\ Γ2 = Γ4).
+                   { eapply aworklist_subst_det; eauto. }
+                   destruct Heq as [Heq1 Heq2]. subst. eauto.
+            ** destruct (a_wf_wl_aworklist_subst_dec Γ X0 (` X)) as [[Γ1' [Γ2' Hsubst']] | Hsubst']; eauto.
+               --- edestruct JgInst2 as [JgInst2' | JgInst2']; eauto.
+                   right. intro Hcontra. dependent destruction Hcontra; try unify_binds.
+                   assert (Heq: Γ1' = Γ1 /\ Γ2' = Γ2).
+                   { eapply aworklist_subst_det; eauto. }
+                   destruct Heq as [Heq1 Heq2]. subst. eauto.
+               --- right. intro Hcontra. dependent destruction Hcontra; try unify_binds.
+      -- destruct (a_mono_typ_dec Γ (typ_arrow A1 A2)); auto. apply a_wf_wl_a_wf_wwl; auto.
+         ++ assert (FV: X ∉ ftvar_in_typ (typ_arrow A1 A2) \/ not (X ∉ ftvar_in_typ (typ_arrow A1 A2))) by fsetdec.
+            destruct FV as [FV | FV]; try solve [right; intro Hcontra; dependent destruction Hcontra; try unify_binds].
+            destruct (a_wf_wl_aworklist_subst_dec Γ X (typ_arrow A1 A2)) as [[Γ1' [Γ2' Hsubst']] | Hsubst']; eauto.
+            ** edestruct JgInst1 as [JgInst1' | JgInst1']; eauto.
+               right. intro Hcontra. dependent destruction Hcontra; try unify_binds.
+               assert (Heq: Γ1' = Γ1 /\ Γ2' = Γ2).
+               { eapply aworklist_subst_det; eauto. }
+               destruct Heq as [Heq1 Heq2]. subst. eauto.
+            ** right. intro Hcontra. dependent destruction Hcontra; try unify_binds.
+         ++ pick fresh X1. pick fresh X2.
+            eapply awl_split_etvar in H as Hbin; eauto.
+            destruct Hbin as [Γ1 [Γ2 Hbin]]. subst.
+            assert (Hsubst: aworklist_subst (work_sub ` X (typ_arrow A1 A2) ⫤ᵃ X2 ~ᵃ ⬒ ;ᵃ X1 ~ᵃ ⬒ ;ᵃ Γ2 ⧺ X ~ᵃ ⬒ ;ᵃ Γ1) X
+                                            (typ_arrow ` X1 ` X2) (X1 ~ᵃ ⬒ ;ᵃ X2 ~ᵃ ⬒ ;ᵃ Γ1) (work_sub ` X (typ_arrow A1 A2) ⫤ᵃ Γ2)).
+            { eapply a_ws1__work_stay. eapply worklist_subst_fresh_etvar_total with (Γ1 := Γ1) (Γ2 := Γ2); eauto. }
+            assert (JgArr1: (work_sub ` X2 (subst_tvar_in_typ (typ_arrow ` X1 ` X2) X A2) ⫤ᵃ work_sub (subst_tvar_in_typ (typ_arrow ` X1 ` X2) X A1) ` X1 ⫤ᵃ subst_tvar_in_aworklist (typ_arrow ` X1 ` X2) X Γ2 ⧺ X1 ~ᵃ ⬒ ;ᵃ X2 ~ᵃ ⬒ ;ᵃ Γ1) ⟶ᵃʷ⁎⋅ \/
+                          ~ (work_sub ` X2 (subst_tvar_in_typ (typ_arrow ` X1 ` X2) X A2) ⫤ᵃ work_sub (subst_tvar_in_typ (typ_arrow ` X1 ` X2) X A1) ` X1 ⫤ᵃ subst_tvar_in_aworklist (typ_arrow ` X1 ` X2) X Γ2 ⧺ X1 ~ᵃ ⬒ ;ᵃ X2 ~ᵃ ⬒ ;ᵃ Γ1) ⟶ᵃʷ⁎⋅).
+            { eapply IHnm; simpl in *; eauto.
+              admit. admit. admit. admit. admit. admit. admit. admit.
+            }          
+            admit. (* TODO: renaming stuff *)
+      -- right. intro Hcontra. dependent destruction Hcontra; try unify_binds.
+         dependent destruction H3; try unify_binds.
+      -- edestruct JgUnion1 as [JgUnion1' | JgUnion1']; eauto.
+         edestruct JgUnion2 as [JgUnion2' | JgUnion2']; eauto.
+         right. intro Hcontra. dependent destruction Hcontra; try unify_binds.
+         dependent destruction H1. 
+         eapply JgUnion1'; eauto. eapply JgUnion2'; eauto.
+      -- edestruct JgInter1 as [JgInter1' | JgInter1']; eauto.
+         right. intro Hcontra. dependent destruction Hcontra; try unify_binds.
+         dependent destruction H1. eauto.
+    * dependent destruction H1;
+        try solve [right; intro Hcontra;
+          dependent destruction Hcontra];
+        try solve [destruct Jg as [Jg | Jg]; eauto;
+          right; intro Hcontra; dependent destruction Hcontra;
+          eapply Jg; eauto].
+      -- right. intro Hcontra. dependent destruction Hcontra; unify_binds.
+      -- right. intro Hcontra. dependent destruction Hcontra; unify_binds.
+      -- admit. (* arrow case *)
+      -- assert (JgArr: (work_sub A2 A3 ⫤ᵃ work_sub A0 A1 ⫤ᵃ Γ) ⟶ᵃʷ⁎⋅ \/
+                      ¬ (work_sub A2 A3 ⫤ᵃ work_sub A0 A1 ⫤ᵃ Γ) ⟶ᵃʷ⁎⋅).
+         { eapply IHnw; eauto.
+           simpl in *. unfold split_depth in *. simpl in *.
+           assert (split_depth_rec (⌊ Γ ⌋ᵃ) A2 1 * S (iu_size A3) +
+            split_depth_rec (⌊ Γ ⌋ᵃ) A3 1 * S (iu_size A2) +
+            (split_depth_rec (⌊ Γ ⌋ᵃ) A0 1 * S (iu_size A1) +
+            split_depth_rec (⌊ Γ ⌋ᵃ) A1 1 * S (iu_size A0) + 
+            split_depth_wl Γ) <= (split_depth_rec (⌊ Γ ⌋ᵃ) A1 1 + split_depth_rec (⌊ Γ ⌋ᵃ) A2 1) *
+            S (iu_size A0 + iu_size A3) +
+            (split_depth_rec (⌊ Γ ⌋ᵃ) A0 1 + split_depth_rec (⌊ Γ ⌋ᵃ) A3 1) *
+            S (iu_size A1 + iu_size A2) + split_depth_wl Γ) by lia.
+            admit.
+           simpl in *. lia. }
+         destruct JgArr as [JgArr | JgArr]; eauto.
+         right. intro Hcontra. dependent destruction Hcontra.
+         apply JgArr; auto.
+      -- edestruct JgUnion1 as [JgUnion1' | JgUnion1']; eauto.
+         edestruct JgUnion2 as [JgUnion2' | JgUnion2']; eauto.
+         right. intro Hcontra. dependent destruction Hcontra.
+         eapply JgUnion1'; eauto. eapply JgUnion2'; eauto.
+      -- edestruct JgInter1 as [JgInter1' | JgInter1']; eauto.
+         right. intro Hcontra. dependent destruction Hcontra.
+         eapply JgInter1'; eauto.
+    * dependent destruction H1.
+      (* can use some tatics, while have to solve the binding problem first*) 
+      -- pick fresh X. inst_cofinites_with X.
+         destruct JgAlll with (X:=X) (A1:=A) (L:=L) as [JgAlll' | JgAlll']; auto.
+         ++ left. inst_cofinites_for a_wl_red__sub_alll; eauto.
+            intros X' Hnin.
+            apply rename_tvar_in_a_wf_wwl_a_wl_red with (X:=X) (Y:=X') in JgAlll'; auto.
+            ** simpl in JgAlll'. destruct_eq_atom.
+               rewrite rename_tvar_in_aworklist_fresh_eq in JgAlll'; auto.
+               rewrite subst_tvar_in_typ_open_typ_wrt_typ_tvar2 in JgAlll'; auto.
+            ** apply a_wf_wl_a_wf_wwl.
+               apply a_wf_wl__conswork_sub; auto.
+               apply a_wf_typ_tvar_etvar with (Σ2 := nil). simpl. auto.
+         ++ right. intro Hcontra. dependent destruction Hcontra; auto.
+            pick fresh X1. inst_cofinites_with X1.
+            apply rename_tvar_in_a_wf_wwl_a_wl_red with (X:=X1) (Y:=X) in H4; auto.
+            ** simpl in H4. destruct_eq_atom.
+               rewrite rename_tvar_in_aworklist_fresh_eq in H4; auto.
+               rewrite subst_tvar_in_typ_open_typ_wrt_typ_tvar2 in H4; auto.
+            ** apply a_wf_wl_a_wf_wwl.
+               apply a_wf_wl__conswork_sub; auto. simpl.
+               apply a_wf_typ_tvar_etvar with (Σ2 := nil). simpl.
+               rewrite <- subst_tvar_in_typ_open_typ_wrt_typ_tvar2 with (X := X); auto.
+               apply a_wf_typ_rename_tvar_cons; auto.
+      -- pick fresh X. inst_cofinites_with X.
+         destruct JgAlll with (X:=X) (A1:=A) (L:=L) as [JgAlll' | JgAlll']; auto.
+         ++ left. inst_cofinites_for a_wl_red__sub_alll; eauto.
+            intros X' Hnin.
+            apply rename_tvar_in_a_wf_wwl_a_wl_red with (X:=X) (Y:=X') in JgAlll'; auto.
+            ** simpl in JgAlll'. destruct_eq_atom.
+               rewrite rename_tvar_in_aworklist_fresh_eq in JgAlll'; auto.
+               rewrite subst_tvar_in_typ_open_typ_wrt_typ_tvar2 in JgAlll'; auto.
+            ** apply a_wf_wl_a_wf_wwl.
+               apply a_wf_wl__conswork_sub; auto.
+               apply a_wf_typ_tvar_etvar with (Σ2 := nil). simpl. auto.
+         ++ right. intro Hcontra. dependent destruction Hcontra; auto.
+            pick fresh X1. inst_cofinites_with X1.
+            apply rename_tvar_in_a_wf_wwl_a_wl_red with (X:=X1) (Y:=X) in H4; auto.
+            ** simpl in H4. destruct_eq_atom.
+               rewrite rename_tvar_in_aworklist_fresh_eq in H4; auto.
+               rewrite subst_tvar_in_typ_open_typ_wrt_typ_tvar2 in H4; auto.
+            ** apply a_wf_wl_a_wf_wwl.
+               apply a_wf_wl__conswork_sub; auto. simpl.
+               apply a_wf_typ_tvar_etvar with (Σ2 := nil). simpl.
+               rewrite <- subst_tvar_in_typ_open_typ_wrt_typ_tvar2 with (X := X); auto.
+               apply a_wf_typ_rename_tvar_cons; auto.
+      -- pick fresh X. inst_cofinites_with X.
+         destruct JgAlll with (X:=X) (A1:=A) (L:=L) as [JgAlll' | JgAlll']; auto.
+         ++ left. inst_cofinites_for a_wl_red__sub_alll; eauto.
+            intros X' Hnin.
+            apply rename_tvar_in_a_wf_wwl_a_wl_red with (X:=X) (Y:=X') in JgAlll'; auto.
+            ** simpl in JgAlll'. destruct_eq_atom.
+               rewrite rename_tvar_in_aworklist_fresh_eq in JgAlll'; auto.
+               rewrite subst_tvar_in_typ_open_typ_wrt_typ_tvar2 in JgAlll'; auto.
+            ** apply a_wf_wl_a_wf_wwl.
+               apply a_wf_wl__conswork_sub; auto.
+               apply a_wf_typ_tvar_etvar with (Σ2 := nil). simpl. auto.
+         ++ right. intro Hcontra. dependent destruction Hcontra; auto.
+            pick fresh X1. inst_cofinites_with X1.
+            apply rename_tvar_in_a_wf_wwl_a_wl_red with (X:=X1) (Y:=X) in H4; auto.
+            ** simpl in H4. destruct_eq_atom.
+               rewrite rename_tvar_in_aworklist_fresh_eq in H4; auto.
+               rewrite subst_tvar_in_typ_open_typ_wrt_typ_tvar2 in H4; auto.
+            ** apply a_wf_wl_a_wf_wwl.
+               apply a_wf_wl__conswork_sub; auto. simpl.
+               apply a_wf_typ_tvar_etvar with (Σ2 := nil). simpl.
+               rewrite <- subst_tvar_in_typ_open_typ_wrt_typ_tvar2 with (X := X); auto.
+               apply a_wf_typ_rename_tvar_cons; auto.
+      -- pick fresh X1. inst_cofinites_with X1.
+         destruct JgAlll with (X:=X1) (A1:=A) (L:=L) as [JgAlll' | JgAlll']; auto.
+         ++ left. inst_cofinites_for a_wl_red__sub_alll; eauto.
+            intros X' Hnin.
+            apply rename_tvar_in_a_wf_wwl_a_wl_red with (X:=X1) (Y:=X') in JgAlll'; auto.
+            ** simpl in JgAlll'. destruct_eq_atom.
+               rewrite rename_tvar_in_aworklist_fresh_eq in JgAlll'; auto.
+               rewrite subst_tvar_in_typ_open_typ_wrt_typ_tvar2 in JgAlll'; auto.
+            ** apply a_wf_wl_a_wf_wwl.
+               apply a_wf_wl__conswork_sub; auto.
+               apply a_wf_typ_tvar_etvar with (Σ2 := nil). simpl. auto.
+               simpl. auto.
+         ++ right. intro Hcontra. dependent destruction Hcontra; try solve [dependent destruction H3].
+            pick fresh X1'. inst_cofinites_with X1'.
+            apply rename_tvar_in_a_wf_wwl_a_wl_red with (X:=X1') (Y:=X1) in H5; auto.
+            ** simpl in H5. destruct_eq_atom.
+               rewrite rename_tvar_in_aworklist_fresh_eq in H5; auto.
+               rewrite subst_tvar_in_typ_open_typ_wrt_typ_tvar2 in H5; auto.
+            ** apply a_wf_wl_a_wf_wwl.
+               apply a_wf_wl__conswork_sub; auto. simpl.
+               apply a_wf_typ_tvar_etvar with (Σ2 := nil). simpl.
+               rewrite <- subst_tvar_in_typ_open_typ_wrt_typ_tvar2 with (X := X1); auto.
+               apply a_wf_typ_rename_tvar_cons; auto.
+               simpl. auto.
+      -- pick fresh X1. inst_cofinites_with X1.
+         destruct JgAlll with (X:=X1) (A1:=A) (L:=L) as [JgAlll' | JgAlll']; auto.
+         ++ left. inst_cofinites_for a_wl_red__sub_alll; eauto.
+            intros X' Hnin.
+            apply rename_tvar_in_a_wf_wwl_a_wl_red with (X:=X1) (Y:=X') in JgAlll'; auto.
+            ** simpl in JgAlll'. destruct_eq_atom.
+               rewrite rename_tvar_in_aworklist_fresh_eq in JgAlll'; auto.
+               rewrite subst_tvar_in_typ_open_typ_wrt_typ_tvar2 in JgAlll'; auto.
+            ** apply a_wf_wl_a_wf_wwl.
+               apply a_wf_wl__conswork_sub; auto.
+               apply a_wf_typ_tvar_etvar with (Σ2 := nil). simpl. auto.
+               simpl. auto.
+         ++ right. intro Hcontra. dependent destruction Hcontra; try solve [dependent destruction H3].
+            pick fresh X1'. inst_cofinites_with X1'.
+            apply rename_tvar_in_a_wf_wwl_a_wl_red with (X:=X1') (Y:=X1) in H5; auto.
+            ** simpl in H5. destruct_eq_atom.
+               rewrite rename_tvar_in_aworklist_fresh_eq in H5; auto.
+               rewrite subst_tvar_in_typ_open_typ_wrt_typ_tvar2 in H5; auto.
+            ** apply a_wf_wl_a_wf_wwl.
+               apply a_wf_wl__conswork_sub; auto. simpl.
+               apply a_wf_typ_tvar_etvar with (Σ2 := nil). simpl.
+               rewrite <- subst_tvar_in_typ_open_typ_wrt_typ_tvar2 with (X := X1); auto.
+               apply a_wf_typ_rename_tvar_cons; auto.
+               simpl. auto.
+      -- pick fresh X1. inst_cofinites_with X1.
+         destruct JgAlll with (X:=X1) (A1:=A) (L:=L) as [JgAlll' | JgAlll']; auto.
+         ++ left. inst_cofinites_for a_wl_red__sub_alll; eauto.
+            intros X' Hnin.
+            apply rename_tvar_in_a_wf_wwl_a_wl_red with (X:=X1) (Y:=X') in JgAlll'; auto.
+            ** simpl in JgAlll'. destruct_eq_atom.
+               rewrite rename_tvar_in_aworklist_fresh_eq in JgAlll'; auto.
+               rewrite subst_tvar_in_typ_open_typ_wrt_typ_tvar2 in JgAlll'; auto.
+            ** apply a_wf_wl_a_wf_wwl.
+               apply a_wf_wl__conswork_sub; auto.
+               apply a_wf_typ_tvar_etvar with (Σ2 := nil). simpl. auto.
+               simpl. auto.
+         ++ right. intro Hcontra. dependent destruction Hcontra; try solve [dependent destruction H3].
+            pick fresh X1'. inst_cofinites_with X1'.
+            apply rename_tvar_in_a_wf_wwl_a_wl_red with (X:=X1') (Y:=X1) in H5; auto.
+            ** simpl in H5. destruct_eq_atom.
+               rewrite rename_tvar_in_aworklist_fresh_eq in H5; auto.
+               rewrite subst_tvar_in_typ_open_typ_wrt_typ_tvar2 in H5; auto.
+            ** apply a_wf_wl_a_wf_wwl.
+               apply a_wf_wl__conswork_sub; auto. simpl.
+               apply a_wf_typ_tvar_etvar with (Σ2 := nil). simpl.
+               rewrite <- subst_tvar_in_typ_open_typ_wrt_typ_tvar2 with (X := X1); auto.
+               apply a_wf_typ_rename_tvar_cons; auto.
+               simpl. auto.
+      -- pick fresh X. inst_cofinites_with X.
+         destruct JgAlll with (X:=X) (A1:=A) (L:=L) as [JgAlll' | JgAlll']; eauto.
+         ++ left. inst_cofinites_for a_wl_red__sub_alll; eauto.
+            intros X' Hnin.
+            apply rename_tvar_in_a_wf_wwl_a_wl_red with (X:=X) (Y:=X') in JgAlll'; auto.
+            ** simpl in JgAlll'. destruct_eq_atom.
+               rewrite rename_tvar_in_aworklist_fresh_eq in JgAlll'; auto.
+               rewrite subst_tvar_in_typ_open_typ_wrt_typ_tvar2 in JgAlll'; auto.
+               rewrite subst_tvar_in_typ_fresh_eq in JgAlll'; auto.
+               rewrite subst_tvar_in_typ_fresh_eq in JgAlll'; auto.
+            ** apply a_wf_wl_a_wf_wwl.
+               apply a_wf_wl__conswork_sub; auto.
+               apply a_wf_typ_tvar_etvar with (Σ2 := nil). simpl. auto.
+               apply a_wf_typ_weaken_cons; auto.
+         ++ right. intro Hcontra. dependent destruction Hcontra; auto.
+            pick fresh X1. inst_cofinites_with X1.
+            apply rename_tvar_in_a_wf_wwl_a_wl_red with (X:=X1) (Y:=X) in H4; auto.
+            ** simpl in H4. destruct_eq_atom.
+               rewrite rename_tvar_in_aworklist_fresh_eq in H4; auto.
+               rewrite subst_tvar_in_typ_open_typ_wrt_typ_tvar2 in H4; auto.
+               rewrite subst_tvar_in_typ_fresh_eq in H4; auto.
+               rewrite subst_tvar_in_typ_fresh_eq in H4; auto.
+            ** apply a_wf_wl_a_wf_wwl.
+               apply a_wf_wl__conswork_sub; auto. simpl.
+               apply a_wf_typ_tvar_etvar with (Σ2 := nil). simpl.
+               rewrite <- subst_tvar_in_typ_open_typ_wrt_typ_tvar2 with (X := X); auto.
+               apply a_wf_typ_rename_tvar_cons; auto.
+               apply a_wf_typ_weaken_cons; auto.
+      --  pick fresh X. inst_cofinites_with X.
+          assert (JgAll: (work_sub (A ᵗ^ₜ X) (A0 ᵗ^ₜ X) ⫤ᵃ X ~ᵃ ■ ;ᵃ Γ) ⟶ᵃʷ⁎⋅ \/
+                       ¬ (work_sub (A ᵗ^ₜ X) (A0 ᵗ^ₜ X) ⫤ᵃ X ~ᵃ ■ ;ᵃ Γ) ⟶ᵃʷ⁎⋅).
+          { eapply IHnw; eauto; simpl in *; try lia.
+            admit. (* safe: wf *) 
+            admit. admit. }
+          destruct JgAll as [JgAll | JgAll]; eauto.
+          ++ left. inst_cofinites_for a_wl_red__sub_all; eauto.
+             intros X' Hnin. 
+             apply rename_tvar_in_a_wf_wwl_a_wl_red with (X:=X) (Y:=X') in JgAll; auto.
+             ** simpl in JgAll. destruct_eq_atom.
+                rewrite rename_tvar_in_aworklist_fresh_eq in JgAll; auto.
+                rewrite subst_tvar_in_typ_open_typ_wrt_typ_tvar2 in JgAll; auto.
+                rewrite subst_tvar_in_typ_open_typ_wrt_typ_tvar2 in JgAll; auto.
+            ** apply a_wf_wl_a_wf_wwl.
+               apply a_wf_wl__conswork_sub; auto. simpl.
+               apply a_wf_typ_tvar_stvar with (Σ2 := nil). simpl. auto.
+               apply a_wf_typ_tvar_stvar with (Σ2 := nil). simpl. auto.
+          ++ right. intro Hcontra. dependent destruction Hcontra; try solve [dependent destruction H3].
+             pick fresh X1. inst_cofinites_with X1.
+             apply rename_tvar_in_a_wf_wwl_a_wl_red with (X:=X1) (Y:=X) in H3; auto.
+            ** simpl in H3. destruct_eq_atom.
+               rewrite rename_tvar_in_aworklist_fresh_eq in H3; auto.
+               rewrite subst_tvar_in_typ_open_typ_wrt_typ_tvar2 in H3; auto.
+               rewrite subst_tvar_in_typ_open_typ_wrt_typ_tvar2 in H3; auto.
+            ** apply a_wf_wl_a_wf_wwl.
+               apply a_wf_wl__conswork_sub; auto. simpl.
+               apply a_wf_typ_tvar_stvar with (Σ2 := nil). simpl.
+               rewrite <- subst_tvar_in_typ_open_typ_wrt_typ_tvar2 with (X := X); auto.
+               apply a_wf_typ_rename_tvar_cons; auto.
+               apply a_wf_typ_tvar_stvar with (Σ2 := nil). simpl.
+               rewrite <- subst_tvar_in_typ_open_typ_wrt_typ_tvar2 with (X := X); auto.
+               apply a_wf_typ_rename_tvar_cons; auto.
+      -- edestruct JgUnion1 as [JgUnion1' | JgUnion1']; eauto.
+         edestruct JgUnion2 as [JgUnion2' | JgUnion2']; eauto.
+         right. intro Hcontra. dependent destruction Hcontra.
+         ++ dependent destruction H3.
+         ++ eapply JgUnion1'; eauto.
+         ++ eapply JgUnion2'; eauto.
+      -- edestruct JgInter1 as [JgInter1' | JgInter1']; eauto.
+         right. intro Hcontra. dependent destruction Hcontra.
+         ++ dependent destruction H2.
+         ++ eapply JgInter1'; eauto.
+  * dependent destruction H1;
+      try solve [edestruct JgUnion3 as [JgUnion3' | JgUnion3']; eauto;
+                  right; intro Hcontra; dependent destruction Hcontra;
+                  eapply JgUnion3'; eauto; try dependent destruction H3].
+    -- edestruct JgUnion1 as [JgUnion1' | JgUnion1']; eauto.
+       edestruct JgUnion2 as [JgUnion2' | JgUnion2']; eauto.
+       edestruct JgUnion3 as [JgUnion3' | JgUnion3']; eauto.
+       right. intro Hcontra. dependent destruction Hcontra.
+       eapply JgUnion1'; eauto. eapply JgUnion2'; eauto. eapply JgUnion3'; eauto.
+    -- edestruct JgInter1 as [JgInter1' | JgInter1']; eauto.
+       edestruct JgUnion3 as [JgUnion3' | JgUnion3']; eauto.
+       right. intro Hcontra. dependent destruction Hcontra.
+       eapply JgInter1'; eauto. eapply JgUnion3'; eauto.
+  * dependent destruction H1;
+      edestruct JgInter2 as [JgInter2' | JgInter2']; eauto;
+      edestruct JgInter3 as [JgInter3' | JgInter3']; eauto;
+      try solve [right; intro Hcontra; dependent destruction Hcontra;
+        try solve [eapply JgInter2'; eauto]; try solve [eapply JgInter3'; eauto];
+        dependent destruction H3].
+    -- edestruct JgUnion1 as [JgUnion1' | JgUnion1']; eauto.
+       edestruct JgUnion2 as [JgUnion2' | JgUnion2']; eauto.
+       right. intro Hcontra. dependent destruction Hcontra.
+       eapply JgInter2'; eauto. eapply JgInter3'; eauto.
+       eapply JgUnion1'; eauto. eapply JgUnion2'; eauto.
+    -- edestruct JgInter1 as [JgInter1' | JgInter1']; eauto.
+       right. intro Hcontra. dependent destruction Hcontra.
+       eapply JgInter1'; eauto. eapply JgInter2'; eauto. eapply JgInter3'; eauto.
 Admitted.
